<?xml version="1.0"?>
<rdf:RDF xmlns="http://www.ease-crc.org/ont/SUTURO#"
     xml:base="http://www.ease-crc.org/ont/SUTURO"
     xmlns:dc="http://purl.org/dc/elements/1.1/"
     xmlns:owl="http://www.w3.org/2002/07/owl#"
     xmlns:rdf="http://www.w3.org/1999/02/22-rdf-syntax-ns#"
     xmlns:xml="http://www.w3.org/XML/1998/namespace"
     xmlns:xsd="http://www.w3.org/2001/XMLSchema#"
     xmlns:SOMA="http://www.ease-crc.org/ont/SOMA.owl#"
     xmlns:rdfs="http://www.w3.org/2000/01/rdf-schema#"
     xmlns:SUTURO="http://www.ease-crc.org/ont/SUTURO.owl#">
    <owl:Ontology rdf:about="http://www.ease-crc.org/ont/SUTURO.owl">
        <owl:imports rdf:resource="http://www.ease-crc.org/ont/SOMA-HOME.owl"/>
        <owl:imports rdf:resource="http://www.ease-crc.org/ont/SOMA.owl"/>
        <owl:imports rdf:resource="package://knowrob/owl/URDF.owl"/>
    </owl:Ontology>
    


    <!-- 
    ///////////////////////////////////////////////////////////////////////////////////////
    //
    // Annotation properties
    //
    ///////////////////////////////////////////////////////////////////////////////////////
     -->

    


    <!-- http://www.ease-crc.org/ont/SUTURO.owl#perceptionId -->

    <owl:AnnotationProperty rdf:about="http://www.ease-crc.org/ont/SUTURO.owl#perceptionId">
        <rdfs:comment>Used to re-identify the same object by the Perception Subgroup if, for example, the name or IRI is changed. Corresponds to the ID in the  annotations/label mapping of their image datasets.</rdfs:comment>
        <rdfs:isDefinedBy rdf:resource="http://www.ease-crc.org/ont/SUTURO.owl"/>
    </owl:AnnotationProperty>
    


    <!-- http://www.ease-crc.org/ont/SUTURO.owl#perceptionName -->

    <owl:AnnotationProperty rdf:about="http://www.ease-crc.org/ont/SUTURO.owl#perceptionName">
        <rdfs:isDefinedBy rdf:resource="http://www.ease-crc.org/ont/SUTURO.owl"/>
    </owl:AnnotationProperty>
    


    <!-- 
    ///////////////////////////////////////////////////////////////////////////////////////
    //
    // Object Properties
    //
    ///////////////////////////////////////////////////////////////////////////////////////
     -->

    


    <!-- http://www.ease-crc.org/ont/SOMA.owl#hasDisposition -->

    <owl:ObjectProperty rdf:about="http://www.ease-crc.org/ont/SOMA.owl#hasDisposition"/>
    


    <!-- http://www.ease-crc.org/ont/SOMA.owl#hasPhysicalComponent -->

    <owl:ObjectProperty rdf:about="http://www.ease-crc.org/ont/SOMA.owl#hasPhysicalComponent"/>
    


    <!-- http://www.ease-crc.org/ont/SUTURO.owl#hasDestinationLocation -->

    <owl:ObjectProperty rdf:about="http://www.ease-crc.org/ont/SUTURO.owl#hasDestinationLocation">
        <rdfs:subPropertyOf rdf:resource="http://www.ease-crc.org/ont/SUTURO.owl#hasPredefinedLocation"/>
    </owl:ObjectProperty>
    


    <!-- http://www.ease-crc.org/ont/SUTURO.owl#hasOriginLocation -->

    <owl:ObjectProperty rdf:about="http://www.ease-crc.org/ont/SUTURO.owl#hasOriginLocation">
        <rdfs:subPropertyOf rdf:resource="http://www.ease-crc.org/ont/SUTURO.owl#hasPredefinedLocation"/>
    </owl:ObjectProperty>
    


    <!-- http://www.ease-crc.org/ont/SUTURO.owl#hasPredefinedLocation -->

    <owl:ObjectProperty rdf:about="http://www.ease-crc.org/ont/SUTURO.owl#hasPredefinedLocation">
        <rdfs:subPropertyOf rdf:resource="http://www.ontologydesignpatterns.org/ont/dul/DUL.owl#associatedWith"/>
    </owl:ObjectProperty>
    


    <!-- http://www.ease-crc.org/ont/SUTURO.owl#isEntryTo -->

    <owl:ObjectProperty rdf:about="http://www.ease-crc.org/ont/SUTURO.owl#isEntryTo">
        <rdfs:subPropertyOf rdf:resource="http://www.ontologydesignpatterns.org/ont/dul/DUL.owl#hasLocation"/>
        <rdfs:domain rdf:resource="http://www.ease-crc.org/ont/SOMA.owl#Location"/>
        <rdfs:range rdf:resource="http://www.ease-crc.org/ont/SOMA.owl#Room"/>
        <rdfs:comment>A spatial relation holding between a room and a location on the border of the room that should be used for entering the room.</rdfs:comment>
        <rdfs:label>is entry to</rdfs:label>
    </owl:ObjectProperty>
    


    <!-- http://www.ease-crc.org/ont/SUTURO.owl#isExitFrom -->

    <owl:ObjectProperty rdf:about="http://www.ease-crc.org/ont/SUTURO.owl#isExitFrom">
        <rdfs:subPropertyOf rdf:resource="http://www.ontologydesignpatterns.org/ont/dul/DUL.owl#hasLocation"/>
        <rdfs:domain rdf:resource="http://www.ease-crc.org/ont/SOMA.owl#Location"/>
        <rdfs:range rdf:resource="http://www.ease-crc.org/ont/SOMA.owl#Room"/>
        <rdfs:comment>A spatial relation holding between a room and a location on the border of the room that should be used for exiting the room.</rdfs:comment>
        <rdfs:label>is exit from</rdfs:label>
    </owl:ObjectProperty>
    


    <!-- http://www.ease-crc.org/ont/SUTURO.owl#isInRoom -->

    <owl:ObjectProperty rdf:about="http://www.ease-crc.org/ont/SUTURO.owl#isInRoom">
        <rdfs:subPropertyOf rdf:resource="http://www.ease-crc.org/ont/SUTURO.owl#hasPredefinedLocation"/>
    </owl:ObjectProperty>
    


    <!-- http://www.ontologydesignpatterns.org/ont/dul/DUL.owl#associatedWith -->

    <owl:ObjectProperty rdf:about="http://www.ontologydesignpatterns.org/ont/dul/DUL.owl#associatedWith"/>
    


    <!-- http://www.ontologydesignpatterns.org/ont/dul/DUL.owl#hasLocation -->

    <owl:ObjectProperty rdf:about="http://www.ontologydesignpatterns.org/ont/dul/DUL.owl#hasLocation"/>
    


    <!-- 
    ///////////////////////////////////////////////////////////////////////////////////////
    //
    // Data properties
    //
    ///////////////////////////////////////////////////////////////////////////////////////
     -->

    


    <!-- http://www.ease-crc.org/ont/SOMA.owl#hasNameString -->

    <owl:DatatypeProperty rdf:about="http://www.ease-crc.org/ont/SOMA.owl#hasNameString"/>
    


    <!-- http://www.ease-crc.org/ont/SOMA.owl#hasPositionData -->

    <owl:DatatypeProperty rdf:about="http://www.ease-crc.org/ont/SOMA.owl#hasPositionData"/>
    


    <!-- http://www.ease-crc.org/ont/SUTURO.owl#handled -->

    <owl:DatatypeProperty rdf:about="http://www.ease-crc.org/ont/SUTURO.owl#handled">
        <rdfs:subPropertyOf rdf:resource="http://www.ontologydesignpatterns.org/ont/dul/DUL.owl#hasDataValue"/>
        <rdfs:domain rdf:resource="http://www.ontologydesignpatterns.org/ont/dul/DUL.owl#Entity"/>
        <rdfs:range rdf:resource="http://www.w3.org/2001/XMLSchema#boolean"/>
    </owl:DatatypeProperty>
    


    <!-- http://www.ease-crc.org/ont/SUTURO.owl#hasConfidenceValue -->

    <owl:DatatypeProperty rdf:about="http://www.ease-crc.org/ont/SUTURO.owl#hasConfidenceValue">
        <rdfs:subPropertyOf rdf:resource="http://www.ontologydesignpatterns.org/ont/dul/DUL.owl#hasDataValue"/>
        <rdfs:domain rdf:resource="http://www.ontologydesignpatterns.org/ont/dul/DUL.owl#Entity"/>
        <rdfs:range rdf:resource="http://www.w3.org/2001/XMLSchema#float"/>
    </owl:DatatypeProperty>
    


    <!-- http://www.ease-crc.org/ont/SUTURO.owl#hasDataSource -->

    <owl:DatatypeProperty rdf:about="http://www.ease-crc.org/ont/SUTURO.owl#hasDataSource">
        <rdfs:subPropertyOf rdf:resource="http://www.ontologydesignpatterns.org/ont/dul/DUL.owl#hasDataValue"/>
        <rdfs:domain rdf:resource="http://www.ontologydesignpatterns.org/ont/dul/DUL.owl#Entity"/>
        <rdfs:range rdf:resource="http://www.w3.org/2001/XMLSchema#string"/>
        <rdfs:comment xml:lang="en">The source of information for this entity can vary. For instance, tables are derived from the semantic map, whereas the objects perceived are obtained from Perception.</rdfs:comment>
    </owl:DatatypeProperty>
    


    <!-- http://www.ease-crc.org/ont/SUTURO.owl#hasGraspPose -->

    <owl:DatatypeProperty rdf:about="http://www.ease-crc.org/ont/SUTURO.owl#hasGraspPose">
        <rdfs:subPropertyOf rdf:resource="http://www.ontologydesignpatterns.org/ont/dul/DUL.owl#hasDataValue"/>
        <rdfs:comment>The pose an object shall be grabbed from such as &quot;above&quot; or &quot;side&quot;.</rdfs:comment>
        <rdfs:isDefinedBy rdf:resource="http://www.ease-crc.org/ont/SUTURO.owl"/>
    </owl:DatatypeProperty>
    


    <!-- http://www.ease-crc.org/ont/SUTURO.owl#hasHandleState -->

    <owl:DatatypeProperty rdf:about="http://www.ease-crc.org/ont/SUTURO.owl#hasHandleState">
        <rdfs:subPropertyOf rdf:resource="http://www.ontologydesignpatterns.org/ont/dul/DUL.owl#hasDataValue"/>
        <rdfs:domain rdf:resource="http://www.ontologydesignpatterns.org/ont/dul/DUL.owl#Entity"/>
        <rdfs:range rdf:resource="http://www.w3.org/2001/XMLSchema#boolean"/>
    </owl:DatatypeProperty>
    


    <!-- http://www.ease-crc.org/ont/SUTURO.owl#hasPosition -->

    <owl:DatatypeProperty rdf:about="http://www.ease-crc.org/ont/SUTURO.owl#hasPosition">
        <rdfs:subPropertyOf rdf:resource="http://www.ontologydesignpatterns.org/ont/dul/DUL.owl#hasDataValue"/>
        <rdfs:isDefinedBy rdf:resource="http://www.ease-crc.org/ont/SUTURO.owl"/>
    </owl:DatatypeProperty>
    


    <!-- http://www.ease-crc.org/ont/SUTURO.owl#hasPredefinedName -->

    <owl:DatatypeProperty rdf:about="http://www.ease-crc.org/ont/SUTURO.owl#hasPredefinedName">
        <rdfs:subPropertyOf rdf:resource="http://www.ease-crc.org/ont/SOMA.owl#hasNameString"/>
        <rdfs:comment>A predefined name refers to a name or label that is predetermined or established beforehand. It is typically assigned or chosen from a predefined set of names, often based on specific criteria or guidelines.</rdfs:comment>
        <rdfs:isDefinedBy rdf:resource="http://www.ease-crc.org/ont/SUTURO.owl"/>
    </owl:DatatypeProperty>
    


    <!-- http://www.ease-crc.org/ont/SUTURO.owl#hasRobocupName -->

    <owl:DatatypeProperty rdf:about="http://www.ease-crc.org/ont/SUTURO.owl#hasRobocupName">
        <rdfs:subPropertyOf rdf:resource="http://www.ease-crc.org/ont/SOMA.owl#hasNameString"/>
        <rdfs:comment>The robocup name of a furniture instance.

TODO: make this more descriptive and generalized.</rdfs:comment>
    </owl:DatatypeProperty>
    


    <!-- http://www.ontologydesignpatterns.org/ont/dul/DUL.owl#hasDataValue -->

    <owl:DatatypeProperty rdf:about="http://www.ontologydesignpatterns.org/ont/dul/DUL.owl#hasDataValue"/>
    


    <!-- 
    ///////////////////////////////////////////////////////////////////////////////////////
    //
    // Classes
    //
    ///////////////////////////////////////////////////////////////////////////////////////
     -->

    


    <!-- http://knowrob.org/kb/urdf.owl#Robot -->

    <owl:Class rdf:about="http://knowrob.org/kb/urdf.owl#Robot"/>
    


    <!-- http://www.ease-crc.org/ont/SOMA.owl#Appliance -->

    <owl:Class rdf:about="http://www.ease-crc.org/ont/SOMA.owl#Appliance"/>
    


    <!-- http://www.ease-crc.org/ont/SOMA.owl#BakedGood -->

    <owl:Class rdf:about="http://www.ease-crc.org/ont/SOMA.owl#BakedGood">
        <rdfs:subClassOf>
            <owl:Restriction>
                <owl:onProperty rdf:resource="http://www.ease-crc.org/ont/SUTURO.owl#hasPredefinedName"/>
                <owl:hasValue>baked good</owl:hasValue>
            </owl:Restriction>
        </rdfs:subClassOf>
        <rdfs:comment>Baked goods are food items made by cooking or baking ingredients such as flour, sugar, eggs, and butter, resulting in a wide variety of products like bread, pastries, cakes, and cookies. They are typically characterized by their fluffy or crispy texture, and they are enjoyed as snacks or desserts.</rdfs:comment>
    </owl:Class>
    


    <!-- http://www.ease-crc.org/ont/SOMA.owl#Blade -->

    <owl:Class rdf:about="http://www.ease-crc.org/ont/SOMA.owl#Blade"/>
    


    <!-- http://www.ease-crc.org/ont/SOMA.owl#Bottle -->

    <owl:Class rdf:about="http://www.ease-crc.org/ont/SOMA.owl#Bottle">
        <rdfs:subClassOf>
            <owl:Restriction>
                <owl:onProperty rdf:resource="http://www.ease-crc.org/ont/SUTURO.owl#hasPredefinedName"/>
                <owl:hasValue>bottle</owl:hasValue>
            </owl:Restriction>
        </rdfs:subClassOf>
        <SUTURO:perceptionId rdf:datatype="http://www.w3.org/2001/XMLSchema#int">42</SUTURO:perceptionId>
    </owl:Class>
    


    <!-- http://www.ease-crc.org/ont/SOMA.owl#Bowl -->

    <owl:Class rdf:about="http://www.ease-crc.org/ont/SOMA.owl#Bowl">
        <rdfs:subClassOf rdf:resource="http://www.ease-crc.org/ont/SUTURO.owl#RoboCupDishes"/>
        <rdfs:subClassOf>
            <owl:Restriction>
                <owl:onProperty rdf:resource="http://www.ease-crc.org/ont/SOMA.owl#hasDisposition"/>
                <owl:allValuesFrom rdf:resource="http://www.ease-crc.org/ont/SUTURO.owl#Fragility"/>
            </owl:Restriction>
        </rdfs:subClassOf>
        <rdfs:subClassOf>
            <owl:Restriction>
                <owl:onProperty rdf:resource="http://www.ease-crc.org/ont/SOMA.owl#hasPositionData"/>
                <owl:hasValue>Text</owl:hasValue>
            </owl:Restriction>
        </rdfs:subClassOf>
        <rdfs:subClassOf>
            <owl:Restriction>
                <owl:onProperty rdf:resource="http://www.ease-crc.org/ont/SUTURO.owl#hasGraspPose"/>
                <owl:hasValue>above</owl:hasValue>
            </owl:Restriction>
        </rdfs:subClassOf>
        <rdfs:subClassOf>
            <owl:Restriction>
                <owl:onProperty rdf:resource="http://www.ease-crc.org/ont/SUTURO.owl#hasPredefinedName"/>
                <owl:hasValue>bowl</owl:hasValue>
            </owl:Restriction>
        </rdfs:subClassOf>
        <SUTURO:perceptionId rdf:datatype="http://www.w3.org/2001/XMLSchema#int">29</SUTURO:perceptionId>
    </owl:Class>
    


    <!-- http://www.ease-crc.org/ont/SOMA.owl#Box -->

    <owl:Class rdf:about="http://www.ease-crc.org/ont/SOMA.owl#Box"/>
    


    <!-- http://www.ease-crc.org/ont/SOMA.owl#Bread -->

    <owl:Class rdf:about="http://www.ease-crc.org/ont/SOMA.owl#Bread">
        <rdfs:subClassOf>
            <owl:Restriction>
                <owl:onProperty rdf:resource="http://www.ease-crc.org/ont/SUTURO.owl#hasPredefinedName"/>
                <owl:hasValue>bread</owl:hasValue>
            </owl:Restriction>
        </rdfs:subClassOf>
        <rdfs:comment>Bread is a staple food made from a dough of flour, water, and yeast or other leavening agents, which is then baked. It is known for its characteristic crust and soft interior, and it comes in various shapes and sizes, serving as a versatile food item for sandwiches, toasts, or enjoyed on its own. In European cuisine, pancakes refer to thin and flat cakes made from a batter of flour, eggs, and milk or buttermilk. They are usually larger and thinner than American-style pancakes and are commonly enjoyed with sweet or savory fillings, such as jam, Nutella, cheese, or vegetables.</rdfs:comment>
    </owl:Class>
    


    <!-- http://www.ease-crc.org/ont/SOMA.owl#BreakfastPlate -->

    <owl:Class rdf:about="http://www.ease-crc.org/ont/SOMA.owl#BreakfastPlate">
        <rdfs:subClassOf>
            <owl:Restriction>
                <owl:onProperty rdf:resource="http://www.ease-crc.org/ont/SUTURO.owl#hasPredefinedName"/>
                <owl:hasValue>breakfast plate</owl:hasValue>
            </owl:Restriction>
        </rdfs:subClassOf>
    </owl:Class>
    


    <!-- http://www.ease-crc.org/ont/SOMA.owl#CerealBox -->

    <owl:Class rdf:about="http://www.ease-crc.org/ont/SOMA.owl#CerealBox">
        <rdfs:subClassOf rdf:resource="http://www.ease-crc.org/ont/SUTURO.owl#RoboCupSnacks"/>
        <rdfs:subClassOf>
            <owl:Restriction>
                <owl:onProperty rdf:resource="http://www.ease-crc.org/ont/SUTURO.owl#hasPredefinedName"/>
                <owl:hasValue>cereal box</owl:hasValue>
            </owl:Restriction>
        </rdfs:subClassOf>
        <SUTURO:perceptionId rdf:datatype="http://www.w3.org/2001/XMLSchema#int">55</SUTURO:perceptionId>
    </owl:Class>
    


    <!-- http://www.ease-crc.org/ont/SOMA.owl#Cup -->

    <owl:Class rdf:about="http://www.ease-crc.org/ont/SOMA.owl#Cup">
        <rdfs:subClassOf rdf:resource="http://www.ease-crc.org/ont/SUTURO.owl#RoboCupDishes"/>
        <rdfs:subClassOf>
            <owl:Restriction>
                <owl:onProperty rdf:resource="http://www.ease-crc.org/ont/SUTURO.owl#hasPredefinedName"/>
                <owl:hasValue>cup</owl:hasValue>
            </owl:Restriction>
        </rdfs:subClassOf>
        <SUTURO:perceptionId rdf:datatype="http://www.w3.org/2001/XMLSchema#int">53</SUTURO:perceptionId>
    </owl:Class>
    


    <!-- http://www.ease-crc.org/ont/SOMA.owl#Cupboard -->

    <owl:Class rdf:about="http://www.ease-crc.org/ont/SOMA.owl#Cupboard">
        <rdfs:subClassOf>
            <owl:Restriction>
                <owl:onProperty rdf:resource="http://www.ease-crc.org/ont/SUTURO.owl#hasPredefinedName"/>
                <owl:hasValue>cupboard</owl:hasValue>
            </owl:Restriction>
        </rdfs:subClassOf>
        <SUTURO:perceptionId rdf:datatype="http://www.w3.org/2001/XMLSchema#int">3</SUTURO:perceptionId>
        <rdfs:comment>A cupboard is a piece of furniture used for storage, typically in the kitchen or dining room, and often used for storing dishes, glassware, and food items. It can come in various shapes and sizes, ranging from small wall-mounted cabinets to larger standalone units with multiple shelves and compartments.</rdfs:comment>
    </owl:Class>
    


    <!-- http://www.ease-crc.org/ont/SOMA.owl#Cutlery -->

    <owl:Class rdf:about="http://www.ease-crc.org/ont/SOMA.owl#Cutlery">
        <rdfs:subClassOf rdf:resource="http://www.ease-crc.org/ont/SUTURO.owl#HouseholdHardware"/>
        <rdfs:subClassOf>
            <owl:Restriction>
                <owl:onProperty rdf:resource="http://www.ease-crc.org/ont/SUTURO.owl#isInRoom"/>
                <owl:allValuesFrom rdf:resource="http://www.ease-crc.org/ont/SOMA.owl#Kitchen"/>
            </owl:Restriction>
        </rdfs:subClassOf>
        <rdfs:subClassOf>
            <owl:Restriction>
                <owl:onProperty rdf:resource="http://www.ease-crc.org/ont/SUTURO.owl#hasGraspPose"/>
                <owl:hasValue>above</owl:hasValue>
            </owl:Restriction>
        </rdfs:subClassOf>
        <rdfs:subClassOf>
            <owl:Restriction>
                <owl:onProperty rdf:resource="http://www.ease-crc.org/ont/SUTURO.owl#hasPredefinedName"/>
                <owl:hasValue>cutlery</owl:hasValue>
            </owl:Restriction>
        </rdfs:subClassOf>
        <rdfs:comment>Cutlery refers to utensils used for eating or serving food such as forks, knives, spoons, and serving spoons.</rdfs:comment>
    </owl:Class>
    


    <!-- http://www.ease-crc.org/ont/SOMA.owl#CuttingTool -->

    <owl:Class rdf:about="http://www.ease-crc.org/ont/SOMA.owl#CuttingTool">
        <rdfs:comment>A cutting tool is an instrument or machine used for cutting, shaping, or removing material.</rdfs:comment>
    </owl:Class>
    


    <!-- http://www.ease-crc.org/ont/SOMA.owl#Deposition -->

    <owl:Class rdf:about="http://www.ease-crc.org/ont/SOMA.owl#Deposition"/>
    


    <!-- http://www.ease-crc.org/ont/SOMA.owl#DesignedChair -->

    <owl:Class rdf:about="http://www.ease-crc.org/ont/SOMA.owl#DesignedChair">
        <SUTURO:perceptionId rdf:datatype="http://www.w3.org/2001/XMLSchema#integer">2</SUTURO:perceptionId>
    </owl:Class>
    


    <!-- http://www.ease-crc.org/ont/SOMA.owl#DesignedComponent -->

    <owl:Class rdf:about="http://www.ease-crc.org/ont/SOMA.owl#DesignedComponent"/>
    


    <!-- http://www.ease-crc.org/ont/SOMA.owl#DesignedContainer -->

    <owl:Class rdf:about="http://www.ease-crc.org/ont/SOMA.owl#DesignedContainer"/>
    


    <!-- http://www.ease-crc.org/ont/SOMA.owl#DesignedFurniture -->

    <owl:Class rdf:about="http://www.ease-crc.org/ont/SOMA.owl#DesignedFurniture"/>
    


    <!-- http://www.ease-crc.org/ont/SOMA.owl#DesignedHandle -->

    <owl:Class rdf:about="http://www.ease-crc.org/ont/SOMA.owl#DesignedHandle">
        <SUTURO:perceptionId rdf:datatype="http://www.w3.org/2001/XMLSchema#int">15</SUTURO:perceptionId>
    </owl:Class>
    


    <!-- http://www.ease-crc.org/ont/SOMA.owl#DesignedTool -->

    <owl:Class rdf:about="http://www.ease-crc.org/ont/SOMA.owl#DesignedTool"/>
    


    <!-- http://www.ease-crc.org/ont/SOMA.owl#DinnerPlate -->

    <owl:Class rdf:about="http://www.ease-crc.org/ont/SOMA.owl#DinnerPlate">
        <rdfs:subClassOf>
            <owl:Restriction>
                <owl:onProperty rdf:resource="http://www.ease-crc.org/ont/SUTURO.owl#hasPredefinedName"/>
                <owl:hasValue>dinner plate</owl:hasValue>
            </owl:Restriction>
        </rdfs:subClassOf>
    </owl:Class>
    


    <!-- http://www.ease-crc.org/ont/SOMA.owl#Dish -->

    <owl:Class rdf:about="http://www.ease-crc.org/ont/SOMA.owl#Dish">
        <rdfs:subClassOf>
            <owl:Restriction>
                <owl:onProperty rdf:resource="http://www.ease-crc.org/ont/SUTURO.owl#hasPredefinedName"/>
                <owl:hasValue>dish</owl:hasValue>
            </owl:Restriction>
        </rdfs:subClassOf>
        <rdfs:comment>A dish is a prepared food item that is usually cooked and served on a plate, bowl, or platter.</rdfs:comment>
    </owl:Class>
    


    <!-- http://www.ease-crc.org/ont/SOMA.owl#Dishwasher -->

    <owl:Class rdf:about="http://www.ease-crc.org/ont/SOMA.owl#Dishwasher">
        <rdfs:subClassOf>
            <owl:Restriction>
                <owl:onProperty rdf:resource="http://www.ease-crc.org/ont/SUTURO.owl#hasPredefinedName"/>
                <owl:hasValue>dishwasher</owl:hasValue>
            </owl:Restriction>
        </rdfs:subClassOf>
        <SUTURO:perceptionId rdf:datatype="http://www.w3.org/2001/XMLSchema#int">22</SUTURO:perceptionId>
    </owl:Class>
    


    <!-- http://www.ease-crc.org/ont/SOMA.owl#DishwasherTab -->

    <owl:Class rdf:about="http://www.ease-crc.org/ont/SOMA.owl#DishwasherTab">
        <rdfs:subClassOf rdf:resource="http://www.ease-crc.org/ont/SUTURO.owl#RoboCupCleaningSupplies"/>
        <rdfs:subClassOf>
            <owl:Restriction>
                <owl:onProperty rdf:resource="http://www.ease-crc.org/ont/SUTURO.owl#hasPredefinedName"/>
                <owl:hasValue>dishwasher tab</owl:hasValue>
            </owl:Restriction>
        </rdfs:subClassOf>
        <SUTURO:perceptionId rdf:datatype="http://www.w3.org/2001/XMLSchema#int">49</SUTURO:perceptionId>
        <rdfs:isDefinedBy rdf:resource="http://www.ease-crc.org/ont/SUTURO.owl"/>
    </owl:Class>
    


    <!-- http://www.ease-crc.org/ont/SOMA.owl#Disposition -->

    <owl:Class rdf:about="http://www.ease-crc.org/ont/SOMA.owl#Disposition"/>
    


    <!-- http://www.ease-crc.org/ont/SOMA.owl#Door -->

    <owl:Class rdf:about="http://www.ease-crc.org/ont/SOMA.owl#Door">
        <rdfs:subClassOf>
            <owl:Restriction>
                <owl:onProperty rdf:resource="http://www.ease-crc.org/ont/SUTURO.owl#hasPredefinedName"/>
                <owl:hasValue>door</owl:hasValue>
            </owl:Restriction>
        </rdfs:subClassOf>
        <SUTURO:perceptionId rdf:datatype="http://www.w3.org/2001/XMLSchema#int">20</SUTURO:perceptionId>
    </owl:Class>
    


    <!-- http://www.ease-crc.org/ont/SOMA.owl#Drawer -->

    <owl:Class rdf:about="http://www.ease-crc.org/ont/SOMA.owl#Drawer">
        <rdfs:subClassOf>
            <owl:Restriction>
                <owl:onProperty rdf:resource="http://www.ease-crc.org/ont/SUTURO.owl#hasPredefinedName"/>
                <owl:hasValue>drawer</owl:hasValue>
            </owl:Restriction>
        </rdfs:subClassOf>
        <SUTURO:perceptionId rdf:datatype="http://www.w3.org/2001/XMLSchema#int">60</SUTURO:perceptionId>
    </owl:Class>
    


    <!-- http://www.ease-crc.org/ont/SOMA.owl#Fluid -->

    <owl:Class rdf:about="http://www.ease-crc.org/ont/SOMA.owl#Fluid"/>
    


    <!-- http://www.ease-crc.org/ont/SOMA.owl#Fork -->

    <owl:Class rdf:about="http://www.ease-crc.org/ont/SOMA.owl#Fork">
        <rdfs:subClassOf rdf:resource="http://www.ease-crc.org/ont/SUTURO.owl#RoboCupDishes"/>
        <rdfs:subClassOf>
            <owl:Restriction>
                <owl:onProperty rdf:resource="http://www.ease-crc.org/ont/SUTURO.owl#hasPredefinedName"/>
                <owl:hasValue>fork</owl:hasValue>
            </owl:Restriction>
        </rdfs:subClassOf>
        <SUTURO:perceptionId rdf:datatype="http://www.w3.org/2001/XMLSchema#int">5</SUTURO:perceptionId>
    </owl:Class>
    


    <!-- http://www.ease-crc.org/ont/SOMA.owl#Glass -->

    <owl:Class rdf:about="http://www.ease-crc.org/ont/SOMA.owl#Glass">
        <rdfs:subClassOf>
            <owl:Restriction>
                <owl:onProperty rdf:resource="http://www.ease-crc.org/ont/SOMA.owl#hasDisposition"/>
                <owl:allValuesFrom rdf:resource="http://www.ease-crc.org/ont/SUTURO.owl#Fragility"/>
            </owl:Restriction>
        </rdfs:subClassOf>
        <rdfs:subClassOf>
            <owl:Restriction>
                <owl:onProperty rdf:resource="http://www.ease-crc.org/ont/SUTURO.owl#hasPredefinedName"/>
                <owl:hasValue>glass</owl:hasValue>
            </owl:Restriction>
        </rdfs:subClassOf>
        <SUTURO:perceptionId rdf:datatype="http://www.w3.org/2001/XMLSchema#int">30</SUTURO:perceptionId>
    </owl:Class>
    


    <!-- http://www.ease-crc.org/ont/SOMA.owl#Intrinsic -->

    <owl:Class rdf:about="http://www.ease-crc.org/ont/SOMA.owl#Intrinsic"/>
    


    <!-- http://www.ease-crc.org/ont/SOMA.owl#Jar -->

    <owl:Class rdf:about="http://www.ease-crc.org/ont/SOMA.owl#Jar"/>
    


    <!-- http://www.ease-crc.org/ont/SOMA.owl#Kitchen -->

    <owl:Class rdf:about="http://www.ease-crc.org/ont/SOMA.owl#Kitchen">
        <rdfs:subClassOf>
            <owl:Restriction>
                <owl:onProperty rdf:resource="http://www.ease-crc.org/ont/SUTURO.owl#hasPredefinedName"/>
                <owl:hasValue>kitchen</owl:hasValue>
            </owl:Restriction>
        </rdfs:subClassOf>
        <rdfs:comment>A kitchen is a dedicated space in a home or establishment used for cooking, food preparation, and sometimes dining. It typically contains appliances such as a stove, refrigerator, and sink, as well as storage for cookware, utensils, and ingredients.</rdfs:comment>
    </owl:Class>
    


    <!-- http://www.ease-crc.org/ont/SOMA.owl#KitchenCabinet -->

    <owl:Class rdf:about="http://www.ease-crc.org/ont/SOMA.owl#KitchenCabinet">
        <rdfs:subClassOf>
            <owl:Restriction>
                <owl:onProperty rdf:resource="http://www.ease-crc.org/ont/SUTURO.owl#hasPredefinedName"/>
                <owl:hasValue>kitchen cabinet</owl:hasValue>
            </owl:Restriction>
        </rdfs:subClassOf>
        <SUTURO:perceptionId rdf:datatype="http://www.w3.org/2001/XMLSchema#decimal">9</SUTURO:perceptionId>
    </owl:Class>
    


    <!-- http://www.ease-crc.org/ont/SOMA.owl#KitchenKnife -->

    <owl:Class rdf:about="http://www.ease-crc.org/ont/SOMA.owl#KitchenKnife">
        <rdfs:subClassOf>
            <owl:Restriction>
                <owl:onProperty rdf:resource="http://www.ease-crc.org/ont/SUTURO.owl#hasPredefinedName"/>
                <owl:hasValue>kitchen knife</owl:hasValue>
            </owl:Restriction>
        </rdfs:subClassOf>
    </owl:Class>
    


    <!-- http://www.ease-crc.org/ont/SOMA.owl#Knife -->

    <owl:Class rdf:about="http://www.ease-crc.org/ont/SOMA.owl#Knife">
        <rdfs:subClassOf rdf:resource="http://www.ease-crc.org/ont/SOMA.owl#Cutlery"/>
        <rdfs:subClassOf rdf:resource="http://www.ease-crc.org/ont/SUTURO.owl#RoboCupDishes"/>
        <rdfs:subClassOf>
            <owl:Restriction>
                <owl:onProperty rdf:resource="http://www.ease-crc.org/ont/SUTURO.owl#hasPosition"/>
                <owl:hasValue>right</owl:hasValue>
            </owl:Restriction>
        </rdfs:subClassOf>
        <rdfs:subClassOf>
            <owl:Restriction>
                <owl:onProperty rdf:resource="http://www.ease-crc.org/ont/SUTURO.owl#hasPredefinedName"/>
                <owl:hasValue>knife</owl:hasValue>
            </owl:Restriction>
        </rdfs:subClassOf>
        <SUTURO:perceptionId rdf:datatype="http://www.w3.org/2001/XMLSchema#int">50</SUTURO:perceptionId>
    </owl:Class>
    


    <!-- http://www.ease-crc.org/ont/SOMA.owl#Lid -->

    <owl:Class rdf:about="http://www.ease-crc.org/ont/SOMA.owl#Lid"/>
    


    <!-- http://www.ease-crc.org/ont/SOMA.owl#Location -->

    <owl:Class rdf:about="http://www.ease-crc.org/ont/SOMA.owl#Location"/>
    


    <!-- http://www.ease-crc.org/ont/SOMA.owl#MilkBottle -->

    <owl:Class rdf:about="http://www.ease-crc.org/ont/SOMA.owl#MilkBottle">
        <rdfs:subClassOf rdf:resource="http://www.ease-crc.org/ont/SUTURO.owl#Milk"/>
        <rdfs:subClassOf rdf:resource="http://www.ease-crc.org/ont/SUTURO.owl#RoboCupDrinks"/>
        <rdfs:subClassOf>
            <owl:Restriction>
                <owl:onProperty rdf:resource="http://www.ease-crc.org/ont/SUTURO.owl#hasPredefinedName"/>
                <owl:hasValue>milk bottle</owl:hasValue>
            </owl:Restriction>
        </rdfs:subClassOf>
        <SUTURO:perceptionId rdf:datatype="http://www.w3.org/2001/XMLSchema#int">85</SUTURO:perceptionId>
    </owl:Class>
    


    <!-- http://www.ease-crc.org/ont/SOMA.owl#MilkPack -->

    <owl:Class rdf:about="http://www.ease-crc.org/ont/SOMA.owl#MilkPack">
        <rdfs:subClassOf>
            <owl:Restriction>
                <owl:onProperty rdf:resource="http://www.ease-crc.org/ont/SUTURO.owl#hasPredefinedName"/>
                <owl:hasValue>milk pack</owl:hasValue>
            </owl:Restriction>
        </rdfs:subClassOf>
        <SUTURO:perceptionId rdf:datatype="http://www.w3.org/2001/XMLSchema#int">63</SUTURO:perceptionId>
    </owl:Class>
    


    <!-- http://www.ease-crc.org/ont/SOMA.owl#Pack -->

    <owl:Class rdf:about="http://www.ease-crc.org/ont/SOMA.owl#Pack"/>
    


    <!-- http://www.ease-crc.org/ont/SOMA.owl#Pan -->

    <owl:Class rdf:about="http://www.ease-crc.org/ont/SOMA.owl#Pan"/>
    


    <!-- http://www.ease-crc.org/ont/SOMA.owl#Pancake -->

    <owl:Class rdf:about="http://www.ease-crc.org/ont/SOMA.owl#Pancake">
        <rdfs:subClassOf>
            <owl:Restriction>
                <owl:onProperty rdf:resource="http://www.ease-crc.org/ont/SUTURO.owl#hasPredefinedName"/>
                <owl:hasValue>pancake</owl:hasValue>
            </owl:Restriction>
        </rdfs:subClassOf>
        <rdfs:comment>Pancakes are a type of flat, round, and fluffy breakfast food made from a batter of flour, eggs, milk, and a leavening agent, typically baking powder or baking soda. They are cooked on a griddle or frying pan and are often served with toppings such as syrup, fruit, or whipped cream, making them a popular choice for a delicious morning meal.</rdfs:comment>
    </owl:Class>
    


    <!-- http://www.ease-crc.org/ont/SOMA.owl#PastaBowl -->

    <owl:Class rdf:about="http://www.ease-crc.org/ont/SOMA.owl#PastaBowl">
        <rdfs:subClassOf>
            <owl:Restriction>
                <owl:onProperty rdf:resource="http://www.ease-crc.org/ont/SUTURO.owl#hasPredefinedName"/>
                <owl:hasValue>pasta bowl</owl:hasValue>
            </owl:Restriction>
        </rdfs:subClassOf>
    </owl:Class>
    


    <!-- http://www.ease-crc.org/ont/SOMA.owl#Plate -->

    <owl:Class rdf:about="http://www.ease-crc.org/ont/SOMA.owl#Plate">
        <rdfs:subClassOf rdf:resource="http://www.ease-crc.org/ont/SUTURO.owl#RoboCupDishes"/>
        <rdfs:subClassOf>
            <owl:Restriction>
                <owl:onProperty rdf:resource="http://www.ease-crc.org/ont/SOMA.owl#hasDisposition"/>
                <owl:allValuesFrom rdf:resource="http://www.ease-crc.org/ont/SUTURO.owl#Fragility"/>
            </owl:Restriction>
        </rdfs:subClassOf>
        <rdfs:subClassOf>
            <owl:Restriction>
                <owl:onProperty rdf:resource="http://www.ease-crc.org/ont/SUTURO.owl#hasGraspPose"/>
                <owl:hasValue>side</owl:hasValue>
            </owl:Restriction>
        </rdfs:subClassOf>
        <rdfs:subClassOf>
            <owl:Restriction>
                <owl:onProperty rdf:resource="http://www.ease-crc.org/ont/SUTURO.owl#hasPredefinedName"/>
                <owl:hasValue>plate</owl:hasValue>
            </owl:Restriction>
        </rdfs:subClassOf>
        <SUTURO:perceptionId rdf:datatype="http://www.w3.org/2001/XMLSchema#int">52</SUTURO:perceptionId>
    </owl:Class>
    


    <!-- http://www.ease-crc.org/ont/SOMA.owl#Pot -->

    <owl:Class rdf:about="http://www.ease-crc.org/ont/SOMA.owl#Pot">
        <rdfs:subClassOf>
            <owl:Restriction>
                <owl:onProperty rdf:resource="http://www.ease-crc.org/ont/SUTURO.owl#hasPredefinedName"/>
                <owl:hasValue>pot</owl:hasValue>
            </owl:Restriction>
        </rdfs:subClassOf>
        <SUTURO:perceptionId rdf:datatype="http://www.w3.org/2001/XMLSchema#int">16</SUTURO:perceptionId>
        <rdfs:comment>Pot is a container, typically made of ceramic or clay, used for cooking, serving, or storing food. It comes in various shapes, sizes, and designs and is a common household item found in many cultures around the world.</rdfs:comment>
    </owl:Class>
    


    <!-- http://www.ease-crc.org/ont/SOMA.owl#Preference -->

    <owl:Class rdf:about="http://www.ease-crc.org/ont/SOMA.owl#Preference"/>
    


    <!-- http://www.ease-crc.org/ont/SOMA.owl#Rack -->

    <owl:Class rdf:about="http://www.ease-crc.org/ont/SOMA.owl#Rack"/>
    


    <!-- http://www.ease-crc.org/ont/SOMA.owl#Refrigerator -->

    <owl:Class rdf:about="http://www.ease-crc.org/ont/SOMA.owl#Refrigerator"/>
    


    <!-- http://www.ease-crc.org/ont/SOMA.owl#Room -->

    <owl:Class rdf:about="http://www.ease-crc.org/ont/SOMA.owl#Room"/>
    


    <!-- http://www.ease-crc.org/ont/SOMA.owl#SaladBowl -->

    <owl:Class rdf:about="http://www.ease-crc.org/ont/SOMA.owl#SaladBowl">
        <rdfs:subClassOf>
            <owl:Restriction>
                <owl:onProperty rdf:resource="http://www.ease-crc.org/ont/SUTURO.owl#hasPredefinedName"/>
                <owl:hasValue>salad bowl</owl:hasValue>
            </owl:Restriction>
        </rdfs:subClassOf>
    </owl:Class>
    


    <!-- http://www.ease-crc.org/ont/SOMA.owl#SaltShaker -->

    <owl:Class rdf:about="http://www.ease-crc.org/ont/SOMA.owl#SaltShaker">
        <rdfs:subClassOf>
            <owl:Restriction>
                <owl:onProperty rdf:resource="http://www.ease-crc.org/ont/SUTURO.owl#hasPredefinedName"/>
                <owl:hasValue>salt shaker</owl:hasValue>
            </owl:Restriction>
        </rdfs:subClassOf>
        <SUTURO:perceptionId rdf:datatype="http://www.w3.org/2001/XMLSchema#int">34</SUTURO:perceptionId>
    </owl:Class>
    


    <!-- http://www.ease-crc.org/ont/SOMA.owl#Shaker -->

    <owl:Class rdf:about="http://www.ease-crc.org/ont/SOMA.owl#Shaker"/>
    


    <!-- http://www.ease-crc.org/ont/SOMA.owl#Sink -->

    <owl:Class rdf:about="http://www.ease-crc.org/ont/SOMA.owl#Sink">
        <rdfs:subClassOf>
            <owl:Restriction>
                <owl:onProperty rdf:resource="http://www.ease-crc.org/ont/SUTURO.owl#hasPredefinedName"/>
                <owl:hasValue>sink</owl:hasValue>
            </owl:Restriction>
        </rdfs:subClassOf>
    </owl:Class>
    


    <!-- http://www.ease-crc.org/ont/SOMA.owl#Sofa -->

    <owl:Class rdf:about="http://www.ease-crc.org/ont/SOMA.owl#Sofa">
        <rdfs:subClassOf>
            <owl:Restriction>
                <owl:onProperty rdf:resource="http://www.ease-crc.org/ont/SUTURO.owl#hasPredefinedName"/>
                <owl:hasValue>sofa</owl:hasValue>
            </owl:Restriction>
        </rdfs:subClassOf>
    </owl:Class>
    


    <!-- http://www.ease-crc.org/ont/SOMA.owl#Spatula -->

    <owl:Class rdf:about="http://www.ease-crc.org/ont/SOMA.owl#Spatula">
        <rdfs:subClassOf>
            <owl:Restriction>
                <owl:onProperty rdf:resource="http://www.ease-crc.org/ont/SUTURO.owl#hasPredefinedName"/>
                <owl:hasValue>spatula</owl:hasValue>
            </owl:Restriction>
        </rdfs:subClassOf>
        <SUTURO:perceptionId rdf:datatype="http://www.w3.org/2001/XMLSchema#int">6</SUTURO:perceptionId>
        <rdfs:comment>A spatula is a flat, broad kitchen tool with a long handle used for flipping and lifting food items, such as pancakes, eggs, or burgers, while cooking.</rdfs:comment>
    </owl:Class>
    


    <!-- http://www.ease-crc.org/ont/SOMA.owl#Spoon -->

    <owl:Class rdf:about="http://www.ease-crc.org/ont/SOMA.owl#Spoon">
        <rdfs:subClassOf rdf:resource="http://www.ease-crc.org/ont/SUTURO.owl#RoboCupDishes"/>
        <rdfs:subClassOf>
            <owl:Restriction>
                <owl:onProperty rdf:resource="http://www.ease-crc.org/ont/SUTURO.owl#hasGraspPose"/>
                <owl:hasValue>above</owl:hasValue>
            </owl:Restriction>
        </rdfs:subClassOf>
        <rdfs:subClassOf>
            <owl:Restriction>
                <owl:onProperty rdf:resource="http://www.ease-crc.org/ont/SUTURO.owl#hasPredefinedName"/>
                <owl:hasValue>spoon</owl:hasValue>
            </owl:Restriction>
        </rdfs:subClassOf>
        <SUTURO:perceptionId rdf:datatype="http://www.w3.org/2001/XMLSchema#int">40</SUTURO:perceptionId>
    </owl:Class>
    


    <!-- http://www.ease-crc.org/ont/SOMA.owl#Table -->

    <owl:Class rdf:about="http://www.ease-crc.org/ont/SOMA.owl#Table">
        <rdfs:subClassOf>
            <owl:Restriction>
                <owl:onProperty rdf:resource="http://www.ease-crc.org/ont/SOMA.owl#hasDisposition"/>
                <owl:allValuesFrom rdf:resource="http://www.ease-crc.org/ont/SOMA.owl#Deposition"/>
            </owl:Restriction>
        </rdfs:subClassOf>
        <rdfs:subClassOf>
            <owl:Restriction>
                <owl:onProperty rdf:resource="http://www.ease-crc.org/ont/SUTURO.owl#hasPredefinedName"/>
                <owl:hasValue>table</owl:hasValue>
            </owl:Restriction>
        </rdfs:subClassOf>
        <SUTURO:perceptionId rdf:datatype="http://www.w3.org/2001/XMLSchema#int">28</SUTURO:perceptionId>
        <rdfs:comment>A table is a data structure that organizes information into rows and columns, forming a grid. Tables are widely used in databases and spreadsheets, where each row represents a data record and each column represents a data attribute.</rdfs:comment>
    </owl:Class>
    


    <!-- http://www.ease-crc.org/ont/SOMA.owl#TrashContainer -->

    <owl:Class rdf:about="http://www.ease-crc.org/ont/SOMA.owl#TrashContainer"/>
    


    <!-- http://www.ease-crc.org/ont/SOMA.owl#WaterGlass -->

    <owl:Class rdf:about="http://www.ease-crc.org/ont/SOMA.owl#WaterGlass">
        <rdfs:subClassOf>
            <owl:Restriction>
                <owl:onProperty rdf:resource="http://www.ease-crc.org/ont/SUTURO.owl#hasPredefinedName"/>
                <owl:hasValue>water glass</owl:hasValue>
            </owl:Restriction>
        </rdfs:subClassOf>
    </owl:Class>
    


    <!-- http://www.ease-crc.org/ont/SOMA.owl#WineBottle -->

    <owl:Class rdf:about="http://www.ease-crc.org/ont/SOMA.owl#WineBottle">
        <rdfs:subClassOf rdf:resource="http://www.ease-crc.org/ont/SUTURO.owl#RoboCupDrinks"/>
        <rdfs:subClassOf>
            <owl:Restriction>
                <owl:onProperty rdf:resource="http://www.ease-crc.org/ont/SUTURO.owl#hasPredefinedName"/>
                <owl:hasValue>wine bottle</owl:hasValue>
            </owl:Restriction>
        </rdfs:subClassOf>
        <SUTURO:perceptionId rdf:datatype="http://www.w3.org/2001/XMLSchema#int">81</SUTURO:perceptionId>
    </owl:Class>
    


    <!-- http://www.ease-crc.org/ont/SOMA.owl#WineGlass -->

    <owl:Class rdf:about="http://www.ease-crc.org/ont/SOMA.owl#WineGlass">
        <rdfs:subClassOf>
            <owl:Restriction>
                <owl:onProperty rdf:resource="http://www.ease-crc.org/ont/SUTURO.owl#hasPredefinedName"/>
                <owl:hasValue>wine glass</owl:hasValue>
            </owl:Restriction>
        </rdfs:subClassOf>
        <SUTURO:perceptionId rdf:datatype="http://www.w3.org/2001/XMLSchema#int">24</SUTURO:perceptionId>
    </owl:Class>
    


    <!-- http://www.ease-crc.org/ont/SUTURO.owl#AbrasiveSponge -->

    <owl:Class rdf:about="http://www.ease-crc.org/ont/SUTURO.owl#AbrasiveSponge">
        <rdfs:subClassOf rdf:resource="http://www.ease-crc.org/ont/SUTURO.owl#RoboCupCleaningSupplies"/>
        <rdfs:subClassOf rdf:resource="http://www.ease-crc.org/ont/SUTURO.owl#Sponge"/>
        <rdfs:subClassOf>
            <owl:Restriction>
                <owl:onProperty rdf:resource="http://www.ease-crc.org/ont/SUTURO.owl#hasPredefinedName"/>
                <owl:hasValue>abrasive sponge</owl:hasValue>
            </owl:Restriction>
        </rdfs:subClassOf>
        <SUTURO:perceptionId rdf:datatype="http://www.w3.org/2001/XMLSchema#int">46</SUTURO:perceptionId>
        <rdfs:comment>An abrasive sponge is a cleaning tool designed to scrub away tough dirt and grime from surfaces using its rough, abrasive surface. It is typically made from materials such as nylon, polyester, or natural fibers, and is commonly used in the kitchen and bathroom for cleaning dishes, pots, pans, and other surfaces.</rdfs:comment>
        <rdfs:isDefinedBy rdf:resource="http://www.ease-crc.org/ont/SUTURO.owl"/>
    </owl:Class>
    


    <!-- http://www.ease-crc.org/ont/SUTURO.owl#AdjustableWrench -->

    <owl:Class rdf:about="http://www.ease-crc.org/ont/SUTURO.owl#AdjustableWrench">
        <rdfs:subClassOf rdf:resource="http://www.ease-crc.org/ont/SUTURO.owl#Wrench"/>
        <rdfs:comment>An adjustable wrench is a hand-held tool with a movable jaw that can be adjusted to fit nuts, bolts, and other objects of different sizes, used for turning or tightening them.</rdfs:comment>
        <rdfs:isDefinedBy rdf:resource="http://www.ease-crc.org/ont/SUTURO.owl"/>
    </owl:Class>
    


    <!-- http://www.ease-crc.org/ont/SUTURO.owl#Apple -->

    <owl:Class rdf:about="http://www.ease-crc.org/ont/SUTURO.owl#Apple">
        <rdfs:subClassOf rdf:resource="http://www.ease-crc.org/ont/SUTURO.owl#Fruit"/>
        <rdfs:subClassOf rdf:resource="http://www.ease-crc.org/ont/SUTURO.owl#RoboCupFruits"/>
        <rdfs:subClassOf>
            <owl:Restriction>
                <owl:onProperty rdf:resource="http://www.ease-crc.org/ont/SUTURO.owl#hasPredefinedName"/>
                <owl:hasValue>apple</owl:hasValue>
            </owl:Restriction>
        </rdfs:subClassOf>
        <SUTURO:perceptionId rdf:datatype="http://www.w3.org/2001/XMLSchema#int">66</SUTURO:perceptionId>
        <rdfs:comment>An apple is a round or oval-shaped fruit with a red, green, or yellow skin, a crisp, juicy flesh, and a core with seeds in the center.</rdfs:comment>
        <rdfs:isDefinedBy rdf:resource="http://www.ease-crc.org/ont/SUTURO.owl"/>
    </owl:Class>
    


    <!-- http://www.ease-crc.org/ont/SUTURO.owl#AppleJuice -->

    <owl:Class rdf:about="http://www.ease-crc.org/ont/SUTURO.owl#AppleJuice">
        <rdfs:subClassOf rdf:resource="http://www.ease-crc.org/ont/SUTURO.owl#Juice"/>
        <rdfs:subClassOf>
            <owl:Restriction>
                <owl:onProperty rdf:resource="http://www.ease-crc.org/ont/SUTURO.owl#hasPredefinedName"/>
                <owl:hasValue>apple juice</owl:hasValue>
            </owl:Restriction>
        </rdfs:subClassOf>
        <rdfs:comment>Apple juice is a beverage made by pressing or extracting the natural liquid from apples, a sweet and crunchy fruit. It is often consumed as a refreshing drink.</rdfs:comment>
        <rdfs:isDefinedBy rdf:resource="http://www.ease-crc.org/ont/SUTURO.owl"/>
    </owl:Class>
    


    <!-- http://www.ease-crc.org/ont/SUTURO.owl#Arena -->

    <owl:Class rdf:about="http://www.ease-crc.org/ont/SUTURO.owl#Arena">
        <rdfs:subClassOf rdf:resource="http://www.ease-crc.org/ont/SOMA.owl#Room"/>
        <rdfs:subClassOf>
            <owl:Restriction>
                <owl:onProperty rdf:resource="http://www.ease-crc.org/ont/SUTURO.owl#hasPredefinedName"/>
                <owl:hasValue>arena</owl:hasValue>
            </owl:Restriction>
        </rdfs:subClassOf>
        <rdfs:comment>The whole arena where the robot is normally allowed to move.</rdfs:comment>
    </owl:Class>
    


    <!-- http://www.ease-crc.org/ont/SUTURO.owl#Bag -->

    <owl:Class rdf:about="http://www.ease-crc.org/ont/SUTURO.owl#Bag">
        <rdfs:subClassOf rdf:resource="http://www.ease-crc.org/ont/SOMA.owl#DesignedContainer"/>
        <rdfs:subClassOf>
            <owl:Restriction>
                <owl:onProperty rdf:resource="http://www.ease-crc.org/ont/SUTURO.owl#hasPredefinedName"/>
                <owl:hasValue>bag</owl:hasValue>
            </owl:Restriction>
        </rdfs:subClassOf>
        <SUTURO:perceptionId rdf:datatype="http://www.w3.org/2001/XMLSchema#int">69</SUTURO:perceptionId>
        <rdfs:comment>A bag is a container made of flexible or rigid materials, such as cloth, paper, or plastic, used to store or transport objects. It often has an opening at the top and can be closed with a zipper, button, or other fastening mechanism. Bags come in a variety of shapes and sizes and are used for a wide range of purposes, from carrying groceries and books to holding personal belongings when traveling.</rdfs:comment>
        <rdfs:isDefinedBy rdf:resource="http://www.ease-crc.org/ont/SUTURO.owl"/>
    </owl:Class>
    


    <!-- http://www.ease-crc.org/ont/SUTURO.owl#Balcony -->

    <owl:Class rdf:about="http://www.ease-crc.org/ont/SUTURO.owl#Balcony">
        <rdfs:subClassOf rdf:resource="http://www.ease-crc.org/ont/SOMA.owl#Room"/>
        <rdfs:subClassOf>
            <owl:Restriction>
                <owl:onProperty rdf:resource="http://www.ease-crc.org/ont/SUTURO.owl#hasPredefinedName"/>
                <owl:hasValue>balcony</owl:hasValue>
            </owl:Restriction>
        </rdfs:subClassOf>
        <rdfs:isDefinedBy rdf:resource="http://www.ease-crc.org/ont/SUTURO.owl"/>
    </owl:Class>
    


    <!-- http://www.ease-crc.org/ont/SUTURO.owl#Ball -->

    <owl:Class rdf:about="http://www.ease-crc.org/ont/SUTURO.owl#Ball">
        <rdfs:subClassOf rdf:resource="http://www.ease-crc.org/ont/SOMA.owl#DesignedTool"/>
        <rdfs:comment>A ball is a spherical object typically used in sports, games, or as a toy, made from various materials and usually bounced, thrown, or kicked.</rdfs:comment>
        <rdfs:isDefinedBy rdf:resource="http://www.ease-crc.org/ont/SUTURO.owl"/>
    </owl:Class>
    


    <!-- http://www.ease-crc.org/ont/SUTURO.owl#Banana -->

    <owl:Class rdf:about="http://www.ease-crc.org/ont/SUTURO.owl#Banana">
        <rdfs:subClassOf rdf:resource="http://www.ease-crc.org/ont/SUTURO.owl#Fruit"/>
        <rdfs:subClassOf rdf:resource="http://www.ease-crc.org/ont/SUTURO.owl#RoboCupFruits"/>
        <rdfs:subClassOf>
            <owl:Restriction>
                <owl:onProperty rdf:resource="http://www.ease-crc.org/ont/SUTURO.owl#hasPredefinedName"/>
                <owl:hasValue>banana</owl:hasValue>
            </owl:Restriction>
        </rdfs:subClassOf>
        <SUTURO:perceptionId rdf:datatype="http://www.w3.org/2001/XMLSchema#int">77</SUTURO:perceptionId>
        <rdfs:comment>A banana is a long, curved fruit with a yellow skin that is easy to peel, a soft, sweet flesh, and small seeds inside.</rdfs:comment>
        <rdfs:isDefinedBy rdf:resource="http://www.ease-crc.org/ont/SUTURO.owl"/>
    </owl:Class>
    


    <!-- http://www.ease-crc.org/ont/SUTURO.owl#Baseball -->

    <owl:Class rdf:about="http://www.ease-crc.org/ont/SUTURO.owl#Baseball">
        <rdfs:subClassOf rdf:resource="http://www.ease-crc.org/ont/SUTURO.owl#Ball"/>
        <rdfs:subClassOf rdf:resource="http://www.ease-crc.org/ont/SUTURO.owl#RoboCupToys"/>
        <rdfs:subClassOf>
            <owl:Restriction>
                <owl:onProperty rdf:resource="http://www.ease-crc.org/ont/SUTURO.owl#hasPredefinedName"/>
                <owl:hasValue>baseball</owl:hasValue>
            </owl:Restriction>
        </rdfs:subClassOf>
        <SUTURO:perceptionId rdf:datatype="http://www.w3.org/2001/XMLSchema#int">12</SUTURO:perceptionId>
        <rdfs:comment>A baseball is a ball used in the sport of baseball, made of cork or rubber, and covered with leather or synthetic materials, and is roughly the size of an adult&apos;s fist.</rdfs:comment>
        <rdfs:isDefinedBy rdf:resource="http://www.ease-crc.org/ont/SUTURO.owl"/>
    </owl:Class>
    


    <!-- http://www.ease-crc.org/ont/SUTURO.owl#Bathroom -->

    <owl:Class rdf:about="http://www.ease-crc.org/ont/SUTURO.owl#Bathroom">
        <rdfs:subClassOf rdf:resource="http://www.ease-crc.org/ont/SOMA.owl#Room"/>
        <rdfs:subClassOf>
            <owl:Restriction>
                <owl:onProperty rdf:resource="http://www.ease-crc.org/ont/SUTURO.owl#hasPredefinedName"/>
                <owl:hasValue>bathroom</owl:hasValue>
            </owl:Restriction>
        </rdfs:subClassOf>
        <rdfs:isDefinedBy rdf:resource="http://www.ease-crc.org/ont/SUTURO.owl"/>
    </owl:Class>
    


    <!-- http://www.ease-crc.org/ont/SUTURO.owl#Bed -->

    <owl:Class rdf:about="http://www.ease-crc.org/ont/SUTURO.owl#Bed">
        <rdfs:subClassOf rdf:resource="http://www.ease-crc.org/ont/SOMA.owl#DesignedFurniture"/>
        <rdfs:subClassOf>
            <owl:Restriction>
                <owl:onProperty rdf:resource="http://www.ease-crc.org/ont/SUTURO.owl#hasPredefinedName"/>
                <owl:hasValue>bed</owl:hasValue>
            </owl:Restriction>
        </rdfs:subClassOf>
        <rdfs:comment>A bed is a piece of furniture for sleeping or resting on that typically includes a mattress and a frame.</rdfs:comment>
        <rdfs:isDefinedBy rdf:resource="http://www.ease-crc.org/ont/SUTURO.owl"/>
    </owl:Class>
    


    <!-- http://www.ease-crc.org/ont/SUTURO.owl#Bedroom -->

    <owl:Class rdf:about="http://www.ease-crc.org/ont/SUTURO.owl#Bedroom">
        <rdfs:subClassOf rdf:resource="http://www.ease-crc.org/ont/SOMA.owl#Room"/>
        <rdfs:subClassOf>
            <owl:Restriction>
                <owl:onProperty rdf:resource="http://www.ease-crc.org/ont/SUTURO.owl#hasPredefinedName"/>
                <owl:hasValue>bedroom</owl:hasValue>
            </owl:Restriction>
        </rdfs:subClassOf>
        <rdfs:comment>A bedroom is a private space within a dwelling primarily used for sleeping and relaxation. It typically contains a bed, storage for personal belongings, and may include additional furniture such as a dresser or nightstand.</rdfs:comment>
        <rdfs:isDefinedBy rdf:resource="http://www.ease-crc.org/ont/SUTURO.owl"/>
    </owl:Class>
    


    <!-- http://www.ease-crc.org/ont/SUTURO.owl#Beer -->

    <owl:Class rdf:about="http://www.ease-crc.org/ont/SUTURO.owl#Beer">
        <rdfs:subClassOf rdf:resource="http://www.ease-crc.org/ont/SUTURO.owl#Drink"/>
        <rdfs:subClassOf>
            <owl:Restriction>
                <owl:onProperty rdf:resource="http://www.ease-crc.org/ont/SUTURO.owl#hasPredefinedName"/>
                <owl:hasValue>beer</owl:hasValue>
            </owl:Restriction>
        </rdfs:subClassOf>
        <rdfs:isDefinedBy rdf:resource="http://www.ease-crc.org/ont/SUTURO.owl"/>
    </owl:Class>
    


    <!-- http://www.ease-crc.org/ont/SUTURO.owl#Bib -->

    <owl:Class rdf:about="http://www.ease-crc.org/ont/SUTURO.owl#Bib">
        <rdfs:subClassOf rdf:resource="http://www.ease-crc.org/ont/SUTURO.owl#DesignedFabric"/>
        <rdfs:subClassOf>
            <owl:Restriction>
                <owl:onProperty rdf:resource="http://www.ease-crc.org/ont/SUTURO.owl#hasPredefinedName"/>
                <owl:hasValue>bib</owl:hasValue>
            </owl:Restriction>
        </rdfs:subClassOf>
        <rdfs:isDefinedBy rdf:resource="http://www.ease-crc.org/ont/SUTURO.owl"/>
    </owl:Class>
    


    <!-- http://www.ease-crc.org/ont/SUTURO.owl#BlankCreditCard -->

    <owl:Class rdf:about="http://www.ease-crc.org/ont/SUTURO.owl#BlankCreditCard">
        <rdfs:subClassOf rdf:resource="http://www.ease-crc.org/ont/SUTURO.owl#CreditCard"/>
        <rdfs:subClassOf>
            <owl:Restriction>
                <owl:onProperty rdf:resource="http://www.ease-crc.org/ont/SUTURO.owl#hasPredefinedName"/>
                <owl:hasValue>blank credit card</owl:hasValue>
            </owl:Restriction>
        </rdfs:subClassOf>
        <rdfs:comment>A blank credit card is a standard-size rectangular piece of plastic with no personal or financial information embossed or encoded on it, used as a blank template for creating customized credit, debit, or ID cards.</rdfs:comment>
        <rdfs:isDefinedBy rdf:resource="http://www.ease-crc.org/ont/SUTURO.owl"/>
    </owl:Class>
    


    <!-- http://www.ease-crc.org/ont/SUTURO.owl#BleachCleanserBottle -->

    <owl:Class rdf:about="http://www.ease-crc.org/ont/SUTURO.owl#BleachCleanserBottle">
        <rdfs:subClassOf rdf:resource="http://www.ease-crc.org/ont/SUTURO.owl#CleanserBottle"/>
        <rdfs:subClassOf rdf:resource="http://www.ease-crc.org/ont/SUTURO.owl#RoboCupCleaningSupplies"/>
        <rdfs:subClassOf>
            <owl:Restriction>
                <owl:onProperty rdf:resource="http://www.ease-crc.org/ont/SUTURO.owl#hasPredefinedName"/>
                <owl:hasValue>bleach</owl:hasValue>
            </owl:Restriction>
        </rdfs:subClassOf>
        <rdfs:subClassOf>
            <owl:Restriction>
                <owl:onProperty rdf:resource="http://www.ease-crc.org/ont/SUTURO.owl#hasPredefinedName"/>
                <owl:hasValue>bleach cleanser bottle</owl:hasValue>
            </owl:Restriction>
        </rdfs:subClassOf>
        <SUTURO:perceptionId rdf:datatype="http://www.w3.org/2001/XMLSchema#int">8</SUTURO:perceptionId>
        <rdfs:comment>A bleach cleanser bottle is a container designed to hold a cleaning solution that contains bleach, a powerful disinfectant and stain remover. It typically has a nozzle or cap that dispenses the solution in a controlled manner to effectively clean and sanitize surfaces.</rdfs:comment>
        <rdfs:isDefinedBy rdf:resource="http://www.ease-crc.org/ont/SUTURO.owl"/>
    </owl:Class>
    


    <!-- http://www.ease-crc.org/ont/SUTURO.owl#Block -->

    <owl:Class rdf:about="http://www.ease-crc.org/ont/SUTURO.owl#Block">
        <rdfs:subClassOf rdf:resource="http://www.ease-crc.org/ont/SOMA.owl#DesignedComponent"/>
        <rdfs:comment>A block is a solid piece of hard material, such as wood, stone or metal, that is used as a construction material, as a support or to hold other objects.</rdfs:comment>
        <rdfs:isDefinedBy rdf:resource="http://www.ease-crc.org/ont/SUTURO.owl"/>
    </owl:Class>
    


    <!-- http://www.ease-crc.org/ont/SUTURO.owl#Blouse -->

    <owl:Class rdf:about="http://www.ease-crc.org/ont/SUTURO.owl#Blouse">
        <rdfs:subClassOf rdf:resource="http://www.ease-crc.org/ont/SUTURO.owl#Clothing"/>
        <rdfs:subClassOf>
            <owl:Restriction>
                <owl:onProperty rdf:resource="http://www.ease-crc.org/ont/SUTURO.owl#hasPredefinedName"/>
                <owl:hasValue>blouse</owl:hasValue>
            </owl:Restriction>
        </rdfs:subClassOf>
        <rdfs:isDefinedBy rdf:resource="http://www.ease-crc.org/ont/SUTURO.owl"/>
    </owl:Class>
    


    <!-- http://www.ease-crc.org/ont/SUTURO.owl#BlueJeans -->

    <owl:Class rdf:about="http://www.ease-crc.org/ont/SUTURO.owl#BlueJeans">
        <rdfs:subClassOf rdf:resource="http://www.ease-crc.org/ont/SUTURO.owl#Clothing"/>
        <rdfs:subClassOf>
            <owl:Restriction>
                <owl:onProperty rdf:resource="http://www.ease-crc.org/ont/SUTURO.owl#hasPredefinedName"/>
                <owl:hasValue>blue jeans</owl:hasValue>
            </owl:Restriction>
        </rdfs:subClassOf>
        <rdfs:isDefinedBy rdf:resource="http://www.ease-crc.org/ont/SUTURO.owl"/>
    </owl:Class>
    


    <!-- http://www.ease-crc.org/ont/SUTURO.owl#Bolt -->

    <owl:Class rdf:about="http://www.ease-crc.org/ont/SUTURO.owl#Bolt">
        <rdfs:subClassOf rdf:resource="http://www.ease-crc.org/ont/SUTURO.owl#Fastener"/>
        <rdfs:subClassOf rdf:resource="http://www.ease-crc.org/ont/SUTURO.owl#MetalHardware"/>
        <rdfs:subClassOf>
            <owl:Restriction>
                <owl:onProperty rdf:resource="http://www.ease-crc.org/ont/SUTURO.owl#hasPredefinedName"/>
                <owl:hasValue>bolt</owl:hasValue>
            </owl:Restriction>
        </rdfs:subClassOf>
        <rdfs:comment>A bolt is a cylindrical or cone-shaped metal fastener with a threaded end used for securing two objects together, often requiring a nut and washer to hold it in place.</rdfs:comment>
        <rdfs:isDefinedBy rdf:resource="http://www.ease-crc.org/ont/SUTURO.owl"/>
    </owl:Class>
    


    <!-- http://www.ease-crc.org/ont/SUTURO.owl#Book -->

    <owl:Class rdf:about="http://www.ease-crc.org/ont/SUTURO.owl#Book">
        <rdfs:subClassOf rdf:resource="http://www.ease-crc.org/ont/SUTURO.owl#PrintedMatter"/>
        <rdfs:comment>A book is a written or printed work consisting of pages bound together, typically containing a story, information, or other forms of expression.</rdfs:comment>
        <rdfs:isDefinedBy rdf:resource="http://www.ease-crc.org/ont/SUTURO.owl"/>
    </owl:Class>
    


    <!-- http://www.ease-crc.org/ont/SUTURO.owl#Bookcase -->

    <owl:Class rdf:about="http://www.ease-crc.org/ont/SUTURO.owl#Bookcase">
        <rdfs:subClassOf rdf:resource="http://www.ease-crc.org/ont/SUTURO.owl#ShelfUnit"/>
        <rdfs:subClassOf>
            <owl:Restriction>
                <owl:onProperty rdf:resource="http://www.ease-crc.org/ont/SUTURO.owl#hasPredefinedName"/>
                <owl:hasValue>book case</owl:hasValue>
            </owl:Restriction>
        </rdfs:subClassOf>
        <rdfs:comment>A bookcase is a piece of furniture with horizontal shelves used to store books.</rdfs:comment>
        <rdfs:isDefinedBy rdf:resource="http://www.ease-crc.org/ont/SUTURO.owl"/>
    </owl:Class>
    


    <!-- http://www.ease-crc.org/ont/SUTURO.owl#BoxLid -->

    <owl:Class rdf:about="http://www.ease-crc.org/ont/SUTURO.owl#BoxLid">
        <rdfs:subClassOf rdf:resource="http://www.ease-crc.org/ont/SOMA.owl#Lid"/>
        <rdfs:comment>A box lid is a removable cover that fits over the top of a box, providing protection and keeping the contents secure.</rdfs:comment>
        <rdfs:isDefinedBy rdf:resource="http://www.ease-crc.org/ont/SUTURO.owl"/>
    </owl:Class>
    


    <!-- http://www.ease-crc.org/ont/SUTURO.owl#Brand -->

    <owl:Class rdf:about="http://www.ease-crc.org/ont/SUTURO.owl#Brand">
        <rdfs:subClassOf rdf:resource="http://www.ontologydesignpatterns.org/ont/dul/DUL.owl#SocialObject"/>
        <rdfs:comment>A brand is a is a name, term, design, symbol or any other feature that identifies and distinguishes a company, product or service from other companies or products in the same market. It is the unique identity that represents the company and its reputation, and can influence consumer behavior and loyalty.</rdfs:comment>
        <rdfs:isDefinedBy rdf:resource="http://www.ease-crc.org/ont/SUTURO.owl"/>
    </owl:Class>
    


    <!-- http://www.ease-crc.org/ont/SUTURO.owl#Can -->

    <owl:Class rdf:about="http://www.ease-crc.org/ont/SUTURO.owl#Can">
        <rdfs:subClassOf rdf:resource="http://www.ease-crc.org/ont/SOMA.owl#DesignedContainer"/>
        <rdfs:subClassOf>
            <owl:Restriction>
                <owl:onProperty rdf:resource="http://www.ease-crc.org/ont/SUTURO.owl#hasPredefinedName"/>
                <owl:hasValue>can</owl:hasValue>
            </owl:Restriction>
        </rdfs:subClassOf>
        <rdfs:comment>A can is a cylindrical container usually made of metal or aluminum, used for storing food, beverages, or other products.</rdfs:comment>
        <rdfs:isDefinedBy rdf:resource="http://www.ease-crc.org/ont/SUTURO.owl"/>
    </owl:Class>
    


    <!-- http://www.ease-crc.org/ont/SUTURO.owl#Candle -->

    <owl:Class rdf:about="http://www.ease-crc.org/ont/SUTURO.owl#Candle">
        <rdfs:subClassOf rdf:resource="http://www.ease-crc.org/ont/SOMA.owl#DesignedComponent"/>
        <rdfs:subClassOf rdf:resource="http://www.ease-crc.org/ont/SUTURO.owl#Decorations"/>
        <rdfs:subClassOf>
            <owl:Restriction>
                <owl:onProperty rdf:resource="http://www.ease-crc.org/ont/SUTURO.owl#hasPredefinedName"/>
                <owl:hasValue>candle</owl:hasValue>
            </owl:Restriction>
        </rdfs:subClassOf>
        <SUTURO:perceptionId rdf:datatype="http://www.w3.org/2001/XMLSchema#decimal">127</SUTURO:perceptionId>
        <rdfs:isDefinedBy rdf:resource="http://www.ease-crc.org/ont/SUTURO.owl"/>
    </owl:Class>
    


    <!-- http://www.ease-crc.org/ont/SUTURO.owl#Candy -->

    <owl:Class rdf:about="http://www.ease-crc.org/ont/SUTURO.owl#Candy">
        <rdfs:subClassOf rdf:resource="http://www.ease-crc.org/ont/SUTURO.owl#RoboCupSnacks"/>
        <rdfs:subClassOf rdf:resource="http://www.ease-crc.org/ont/SUTURO.owl#Sweets"/>
        <rdfs:subClassOf>
            <owl:Restriction>
                <owl:onProperty rdf:resource="http://www.ease-crc.org/ont/SUTURO.owl#hasPredefinedName"/>
                <owl:hasValue>candy</owl:hasValue>
            </owl:Restriction>
        </rdfs:subClassOf>
        <SUTURO:perceptionId rdf:datatype="http://www.w3.org/2001/XMLSchema#decimal">123</SUTURO:perceptionId>
        <rdfs:isDefinedBy rdf:resource="http://www.ease-crc.org/ont/SUTURO.owl"/>
    </owl:Class>
    


    <!-- http://www.ease-crc.org/ont/SUTURO.owl#Cereal -->

    <owl:Class rdf:about="http://www.ease-crc.org/ont/SUTURO.owl#Cereal">
        <rdfs:subClassOf rdf:resource="http://www.ease-crc.org/ont/SUTURO.owl#ProcessedFood"/>
        <rdfs:subClassOf>
            <owl:Restriction>
                <owl:onProperty rdf:resource="http://www.ease-crc.org/ont/SUTURO.owl#hasPredefinedName"/>
                <owl:hasValue>cereal</owl:hasValue>
            </owl:Restriction>
        </rdfs:subClassOf>
        <rdfs:comment>Cereal is a type of food made from processed grains that is typically eaten for breakfast.</rdfs:comment>
        <rdfs:isDefinedBy rdf:resource="http://www.ease-crc.org/ont/SUTURO.owl"/>
    </owl:Class>
    


    <!-- http://www.ease-crc.org/ont/SUTURO.owl#CerealBowl -->

    <owl:Class rdf:about="http://www.ease-crc.org/ont/SUTURO.owl#CerealBowl">
        <rdfs:subClassOf rdf:resource="http://www.ease-crc.org/ont/SOMA.owl#Bowl"/>
        <rdfs:subClassOf>
            <owl:Restriction>
                <owl:onProperty rdf:resource="http://www.ease-crc.org/ont/SUTURO.owl#hasPredefinedName"/>
                <owl:hasValue>cereal bowl</owl:hasValue>
            </owl:Restriction>
        </rdfs:subClassOf>
        <rdfs:comment>A cereal bowl is a deep dish used for serving breakfast cereal with milk.</rdfs:comment>
        <rdfs:isDefinedBy rdf:resource="http://www.ease-crc.org/ont/SUTURO.owl"/>
    </owl:Class>
    


    <!-- http://www.ease-crc.org/ont/SUTURO.owl#CerealBoxRoboCup -->

    <owl:Class rdf:about="http://www.ease-crc.org/ont/SUTURO.owl#CerealBoxRoboCup">
        <rdfs:subClassOf rdf:resource="http://www.ease-crc.org/ont/SOMA.owl#CerealBox"/>
        <rdfs:subClassOf rdf:resource="http://www.ease-crc.org/ont/SUTURO.owl#RoboCupSnacks"/>
        <rdfs:subClassOf>
            <owl:Restriction>
                <owl:onProperty rdf:resource="http://www.ease-crc.org/ont/SUTURO.owl#hasPredefinedName"/>
                <owl:hasValue>cereal box robocup</owl:hasValue>
            </owl:Restriction>
        </rdfs:subClassOf>
        <SUTURO:perceptionId rdf:datatype="http://www.w3.org/2001/XMLSchema#int">89</SUTURO:perceptionId>
        <rdfs:comment>The cereal box(es) used at RoboCup 2023 Bordeaux</rdfs:comment>
        <rdfs:isDefinedBy rdf:resource="http://www.ease-crc.org/ont/SUTURO.owl"/>
    </owl:Class>
    


    <!-- http://www.ease-crc.org/ont/SUTURO.owl#Chain -->

    <owl:Class rdf:about="http://www.ease-crc.org/ont/SUTURO.owl#Chain">
        <rdfs:subClassOf rdf:resource="http://www.ease-crc.org/ont/SUTURO.owl#Fastener"/>
        <rdfs:comment>A chain is a series of metal links or rings, typically made of steel or other metals, connected together to form a flexible, strong, and durable tool for lifting, towing, securing, or transmitting power.</rdfs:comment>
        <rdfs:isDefinedBy rdf:resource="http://www.ease-crc.org/ont/SUTURO.owl"/>
    </owl:Class>
    


    <!-- http://www.ease-crc.org/ont/SUTURO.owl#Chair -->

    <owl:Class rdf:about="http://www.ease-crc.org/ont/SUTURO.owl#Chair">
        <rdfs:subClassOf rdf:resource="http://www.ease-crc.org/ont/SOMA.owl#DesignedChair"/>
        <rdfs:subClassOf>
            <owl:Restriction>
                <owl:onProperty rdf:resource="http://www.ease-crc.org/ont/SUTURO.owl#hasPredefinedName"/>
                <owl:hasValue>chair</owl:hasValue>
            </owl:Restriction>
        </rdfs:subClassOf>
        <rdfs:isDefinedBy rdf:resource="http://www.ease-crc.org/ont/SUTURO.owl"/>
    </owl:Class>
    


    <!-- http://www.ease-crc.org/ont/SUTURO.owl#CheezIt -->

    <owl:Class rdf:about="http://www.ease-crc.org/ont/SUTURO.owl#CheezIt">
        <rdfs:subClassOf rdf:resource="http://www.ease-crc.org/ont/SUTURO.owl#ProcessedFood"/>
        <rdfs:subClassOf>
            <owl:Restriction>
                <owl:onProperty rdf:resource="http://www.ease-crc.org/ont/SUTURO.owl#hasPredefinedName"/>
                <owl:hasValue>cheezit</owl:hasValue>
            </owl:Restriction>
        </rdfs:subClassOf>
        <rdfs:isDefinedBy rdf:resource="http://www.ease-crc.org/ont/SUTURO.owl"/>
    </owl:Class>
    


    <!-- http://www.ease-crc.org/ont/SUTURO.owl#CheezItCrackerBox -->

    <owl:Class rdf:about="http://www.ease-crc.org/ont/SUTURO.owl#CheezItCrackerBox">
        <rdfs:subClassOf rdf:resource="http://www.ease-crc.org/ont/SUTURO.owl#CrackerBox"/>
        <rdfs:subClassOf>
            <owl:Restriction>
                <owl:onProperty rdf:resource="http://www.ease-crc.org/ont/SUTURO.owl#hasPredefinedName"/>
                <owl:hasValue>cheezit cracker box</owl:hasValue>
            </owl:Restriction>
        </rdfs:subClassOf>
        <rdfs:comment>A box containing, or at least intended to contain, Cheeze-It brand crackers. A cracker is a flat, dry-baked pastry, usually made from flour.</rdfs:comment>
        <rdfs:isDefinedBy rdf:resource="http://www.ease-crc.org/ont/SUTURO.owl"/>
    </owl:Class>
    


    <!-- http://www.ease-crc.org/ont/SUTURO.owl#Chili -->

    <owl:Class rdf:about="http://www.ease-crc.org/ont/SUTURO.owl#Chili">
        <rdfs:subClassOf rdf:resource="http://www.ease-crc.org/ont/SUTURO.owl#ProcessedFood"/>
        <rdfs:subClassOf>
            <owl:Restriction>
                <owl:onProperty rdf:resource="http://www.ease-crc.org/ont/SUTURO.owl#hasPredefinedName"/>
                <owl:hasValue>chili</owl:hasValue>
            </owl:Restriction>
        </rdfs:subClassOf>
        <rdfs:isDefinedBy rdf:resource="http://www.ease-crc.org/ont/SUTURO.owl"/>
    </owl:Class>
    


    <!-- http://www.ease-crc.org/ont/SUTURO.owl#ChiliConCarne -->

    <owl:Class rdf:about="http://www.ease-crc.org/ont/SUTURO.owl#ChiliConCarne">
        <rdfs:subClassOf rdf:resource="http://www.ease-crc.org/ont/SUTURO.owl#Chili"/>
        <rdfs:subClassOf>
            <owl:Restriction>
                <owl:onProperty rdf:resource="http://www.ease-crc.org/ont/SUTURO.owl#hasPredefinedName"/>
                <owl:hasValue>chili con carne</owl:hasValue>
            </owl:Restriction>
        </rdfs:subClassOf>
        <rdfs:isDefinedBy rdf:resource="http://www.ease-crc.org/ont/SUTURO.owl"/>
    </owl:Class>
    


    <!-- http://www.ease-crc.org/ont/SUTURO.owl#ChiliSinCarne -->

    <owl:Class rdf:about="http://www.ease-crc.org/ont/SUTURO.owl#ChiliSinCarne">
        <rdfs:subClassOf rdf:resource="http://www.ease-crc.org/ont/SUTURO.owl#Chili"/>
        <rdfs:subClassOf>
            <owl:Restriction>
                <owl:onProperty rdf:resource="http://www.ease-crc.org/ont/SUTURO.owl#hasPredefinedName"/>
                <owl:hasValue>chili sin carne</owl:hasValue>
            </owl:Restriction>
        </rdfs:subClassOf>
        <rdfs:isDefinedBy rdf:resource="http://www.ease-crc.org/ont/SUTURO.owl"/>
    </owl:Class>
    


    <!-- http://www.ease-crc.org/ont/SUTURO.owl#ChipsCan -->

    <owl:Class rdf:about="http://www.ease-crc.org/ont/SUTURO.owl#ChipsCan">
        <rdfs:subClassOf rdf:resource="http://www.ease-crc.org/ont/SUTURO.owl#Can"/>
        <rdfs:subClassOf>
            <owl:Restriction>
                <owl:onProperty rdf:resource="http://www.ease-crc.org/ont/SUTURO.owl#hasPredefinedName"/>
                <owl:hasValue>chips can</owl:hasValue>
            </owl:Restriction>
        </rdfs:subClassOf>
        <rdfs:comment>Chips can refers to a cylindrical container that holds potato chips.</rdfs:comment>
        <rdfs:isDefinedBy rdf:resource="http://www.ease-crc.org/ont/SUTURO.owl"/>
    </owl:Class>
    


    <!-- http://www.ease-crc.org/ont/SUTURO.owl#ChocolateJello -->

    <owl:Class rdf:about="http://www.ease-crc.org/ont/SUTURO.owl#ChocolateJello">
        <rdfs:subClassOf rdf:resource="http://www.ease-crc.org/ont/SUTURO.owl#Jello"/>
        <rdfs:subClassOf>
            <owl:Restriction>
                <owl:onProperty rdf:resource="http://www.ease-crc.org/ont/SUTURO.owl#hasPredefinedName"/>
                <owl:hasValue>chocolate jello</owl:hasValue>
            </owl:Restriction>
        </rdfs:subClassOf>
        <rdfs:isDefinedBy rdf:resource="http://www.ease-crc.org/ont/SUTURO.owl"/>
    </owl:Class>
    


    <!-- http://www.ease-crc.org/ont/SUTURO.owl#Clamp -->

    <owl:Class rdf:about="http://www.ease-crc.org/ont/SUTURO.owl#Clamp">
        <rdfs:subClassOf rdf:resource="http://www.ease-crc.org/ont/SUTURO.owl#ForceConcentratingTool"/>
        <rdfs:subClassOf>
            <owl:Restriction>
                <owl:onProperty rdf:resource="http://www.ease-crc.org/ont/SOMA.owl#hasPhysicalComponent"/>
                <owl:someValuesFrom rdf:resource="http://www.ease-crc.org/ont/SOMA.owl#DesignedHandle"/>
            </owl:Restriction>
        </rdfs:subClassOf>
        <rdfs:subClassOf>
            <owl:Restriction>
                <owl:onProperty rdf:resource="http://www.ease-crc.org/ont/SUTURO.owl#hasPredefinedName"/>
                <owl:hasValue>clamp</owl:hasValue>
            </owl:Restriction>
        </rdfs:subClassOf>
        <SUTURO:perceptionId rdf:datatype="http://www.w3.org/2001/XMLSchema#decimal">103</SUTURO:perceptionId>
        <rdfs:comment>A clamp is a mechanical device with two jaws that can be adjusted to hold an object in place, used for woodworking, metalworking, and other types of manual work.</rdfs:comment>
        <rdfs:isDefinedBy rdf:resource="http://www.ease-crc.org/ont/SUTURO.owl"/>
    </owl:Class>
    


    <!-- http://www.ease-crc.org/ont/SUTURO.owl#CleaningProduct -->

    <owl:Class rdf:about="http://www.ease-crc.org/ont/SUTURO.owl#CleaningProduct">
        <rdfs:subClassOf rdf:resource="http://www.ontologydesignpatterns.org/ont/dul/DUL.owl#DesignedSubstance"/>
        <rdfs:isDefinedBy rdf:resource="http://www.ease-crc.org/ont/SUTURO.owl"/>
    </owl:Class>
    


    <!-- http://www.ease-crc.org/ont/SUTURO.owl#CleaningTool -->

    <owl:Class rdf:about="http://www.ease-crc.org/ont/SUTURO.owl#CleaningTool">
        <rdfs:subClassOf rdf:resource="http://www.ease-crc.org/ont/SOMA.owl#DesignedTool"/>
        <rdfs:comment>A cleaning tool is an instrument used for cleaning or scrubbing surfaces.</rdfs:comment>
        <rdfs:isDefinedBy rdf:resource="http://www.ease-crc.org/ont/SUTURO.owl"/>
    </owl:Class>
    


    <!-- http://www.ease-crc.org/ont/SUTURO.owl#Cleanser -->

    <owl:Class rdf:about="http://www.ease-crc.org/ont/SUTURO.owl#Cleanser">
        <rdfs:subClassOf rdf:resource="http://www.ease-crc.org/ont/SUTURO.owl#CleaningProduct"/>
        <rdfs:subClassOf>
            <owl:Restriction>
                <owl:onProperty rdf:resource="http://www.ease-crc.org/ont/SUTURO.owl#hasPredefinedName"/>
                <owl:hasValue>cleanser</owl:hasValue>
            </owl:Restriction>
        </rdfs:subClassOf>
        <rdfs:isDefinedBy rdf:resource="http://www.ease-crc.org/ont/SUTURO.owl"/>
    </owl:Class>
    


    <!-- http://www.ease-crc.org/ont/SUTURO.owl#CleanserBottle -->

    <owl:Class rdf:about="http://www.ease-crc.org/ont/SUTURO.owl#CleanserBottle">
        <rdfs:subClassOf rdf:resource="http://www.ease-crc.org/ont/SOMA.owl#Bottle"/>
        <rdfs:subClassOf>
            <owl:Restriction>
                <owl:onProperty rdf:resource="http://www.ease-crc.org/ont/SUTURO.owl#hasPredefinedName"/>
                <owl:hasValue>cleanser bottle</owl:hasValue>
            </owl:Restriction>
        </rdfs:subClassOf>
        <rdfs:comment>A container typically made of plastic or glass that holds cleaning products such as liquid soap, bleach, or other household chemicals.</rdfs:comment>
        <rdfs:isDefinedBy rdf:resource="http://www.ease-crc.org/ont/SUTURO.owl"/>
    </owl:Class>
    


    <!-- http://www.ease-crc.org/ont/SUTURO.owl#ClearBox -->

    <owl:Class rdf:about="http://www.ease-crc.org/ont/SUTURO.owl#ClearBox">
        <rdfs:subClassOf rdf:resource="http://www.ease-crc.org/ont/SOMA.owl#Box"/>
        <rdfs:subClassOf>
            <owl:Restriction>
                <owl:onProperty rdf:resource="http://www.ease-crc.org/ont/SUTURO.owl#hasPredefinedName"/>
                <owl:hasValue>clear box</owl:hasValue>
            </owl:Restriction>
        </rdfs:subClassOf>
        <rdfs:comment>A clear box is a transparent container made of plastic, glass, or other clear materials, designed to hold and display objects while keeping them visible and protected.</rdfs:comment>
        <rdfs:isDefinedBy rdf:resource="http://www.ease-crc.org/ont/SUTURO.owl"/>
    </owl:Class>
    


    <!-- http://www.ease-crc.org/ont/SUTURO.owl#Clothing -->

    <owl:Class rdf:about="http://www.ease-crc.org/ont/SUTURO.owl#Clothing">
        <rdfs:subClassOf rdf:resource="http://www.ease-crc.org/ont/SUTURO.owl#DesignedFabric"/>
        <rdfs:isDefinedBy rdf:resource="http://www.ease-crc.org/ont/SUTURO.owl"/>
    </owl:Class>
    


    <!-- http://www.ease-crc.org/ont/SUTURO.owl#Coat -->

    <owl:Class rdf:about="http://www.ease-crc.org/ont/SUTURO.owl#Coat">
        <rdfs:subClassOf rdf:resource="http://www.ease-crc.org/ont/SUTURO.owl#Clothing"/>
        <rdfs:subClassOf>
            <owl:Restriction>
                <owl:onProperty rdf:resource="http://www.ease-crc.org/ont/SUTURO.owl#hasPredefinedName"/>
                <owl:hasValue>coat</owl:hasValue>
            </owl:Restriction>
        </rdfs:subClassOf>
        <rdfs:isDefinedBy rdf:resource="http://www.ease-crc.org/ont/SUTURO.owl"/>
    </owl:Class>
    


    <!-- http://www.ease-crc.org/ont/SUTURO.owl#CoatRack -->

    <owl:Class rdf:about="http://www.ease-crc.org/ont/SUTURO.owl#CoatRack">
        <rdfs:subClassOf rdf:resource="http://www.ease-crc.org/ont/SOMA.owl#Rack"/>
        <rdfs:subClassOf rdf:resource="http://www.ease-crc.org/ont/SUTURO.owl#Rack"/>
        <rdfs:subClassOf>
            <owl:Restriction>
                <owl:onProperty rdf:resource="http://www.ease-crc.org/ont/SUTURO.owl#hasPredefinedName"/>
                <owl:hasValue>coat rack</owl:hasValue>
            </owl:Restriction>
        </rdfs:subClassOf>
        <rdfs:comment>A coat rack is a free-standing or wall-mounted piece of furniture that is designed to hold coats, hats, scarves, and other outerwear.</rdfs:comment>
        <rdfs:isDefinedBy rdf:resource="http://www.ease-crc.org/ont/SUTURO.owl"/>
    </owl:Class>
    


    <!-- http://www.ease-crc.org/ont/SUTURO.owl#CocoaBox -->

    <owl:Class rdf:about="http://www.ease-crc.org/ont/SUTURO.owl#CocoaBox">
        <rdfs:subClassOf rdf:resource="http://www.ease-crc.org/ont/SOMA.owl#Box"/>
        <rdfs:subClassOf>
            <owl:Restriction>
                <owl:onProperty rdf:resource="http://www.ease-crc.org/ont/SUTURO.owl#hasPredefinedName"/>
                <owl:hasValue>cocoa box</owl:hasValue>
            </owl:Restriction>
        </rdfs:subClassOf>
        <rdfs:comment>A cocoa box is a container, usually made of cardboard, metal, or plastic, designed to store and dispense cocoa powder. It often features a resealable lid or cap to maintain the freshness of the cocoa and prevent moisture from entering, and is valued for its ease of storage and use in household kitchens.</rdfs:comment>
        <rdfs:isDefinedBy rdf:resource="http://www.ease-crc.org/ont/SUTURO.owl"/>
    </owl:Class>
    


    <!-- http://www.ease-crc.org/ont/SUTURO.owl#Coffee -->

    <owl:Class rdf:about="http://www.ease-crc.org/ont/SUTURO.owl#Coffee">
        <rdfs:subClassOf rdf:resource="http://www.ease-crc.org/ont/SUTURO.owl#Drink"/>
        <rdfs:subClassOf>
            <owl:Restriction>
                <owl:onProperty rdf:resource="http://www.ease-crc.org/ont/SUTURO.owl#hasPredefinedName"/>
                <owl:hasValue>coffee</owl:hasValue>
            </owl:Restriction>
        </rdfs:subClassOf>
        <rdfs:comment>Coffee is a beverage made by brewing roasted coffee beans, which come from the fruit of the Coffea plant. It is a popular drink worldwide, known for its stimulating effects due to its caffeine content, and can be served hot or cold in a variety of preparations.</rdfs:comment>
        <rdfs:isDefinedBy rdf:resource="http://www.ease-crc.org/ont/SUTURO.owl"/>
    </owl:Class>
    


    <!-- http://www.ease-crc.org/ont/SUTURO.owl#CoffeeCan -->

    <owl:Class rdf:about="http://www.ease-crc.org/ont/SUTURO.owl#CoffeeCan">
        <rdfs:subClassOf rdf:resource="http://www.ease-crc.org/ont/SUTURO.owl#Can"/>
        <rdfs:subClassOf rdf:resource="http://www.ease-crc.org/ont/SUTURO.owl#RoboCupFood"/>
        <rdfs:subClassOf>
            <owl:Restriction>
                <owl:onProperty rdf:resource="http://www.ease-crc.org/ont/SUTURO.owl#hasPredefinedName"/>
                <owl:hasValue>coffee can</owl:hasValue>
            </owl:Restriction>
        </rdfs:subClassOf>
        <SUTURO:perceptionId rdf:datatype="http://www.w3.org/2001/XMLSchema#int">62</SUTURO:perceptionId>
        <rdfs:comment>A coffee can is a cylindrical container typically made of metal or plastic, used for storing and transporting coffee or other dry goods.</rdfs:comment>
        <rdfs:isDefinedBy rdf:resource="http://www.ease-crc.org/ont/SUTURO.owl"/>
    </owl:Class>
    


    <!-- http://www.ease-crc.org/ont/SUTURO.owl#CoffeeGrounds -->

    <owl:Class rdf:about="http://www.ease-crc.org/ont/SUTURO.owl#CoffeeGrounds">
        <rdfs:subClassOf rdf:resource="http://www.ontologydesignpatterns.org/ont/dul/DUL.owl#DesignedSubstance"/>
        <rdfs:subClassOf>
            <owl:Restriction>
                <owl:onProperty rdf:resource="http://www.ease-crc.org/ont/SUTURO.owl#hasPredefinedName"/>
                <owl:hasValue>coffee grounds</owl:hasValue>
            </owl:Restriction>
        </rdfs:subClassOf>
        <rdfs:isDefinedBy rdf:resource="http://www.ease-crc.org/ont/SUTURO.owl"/>
    </owl:Class>
    


    <!-- http://www.ease-crc.org/ont/SUTURO.owl#CoffeePack -->

    <owl:Class rdf:about="http://www.ease-crc.org/ont/SUTURO.owl#CoffeePack">
        <rdfs:subClassOf rdf:resource="http://www.ease-crc.org/ont/SOMA.owl#Pack"/>
        <rdfs:subClassOf>
            <owl:Restriction>
                <owl:onProperty rdf:resource="http://www.ease-crc.org/ont/SUTURO.owl#hasPredefinedName"/>
                <owl:hasValue>coffee pack</owl:hasValue>
            </owl:Restriction>
        </rdfs:subClassOf>
        <SUTURO:perceptionId rdf:datatype="http://www.w3.org/2001/XMLSchema#int">31</SUTURO:perceptionId>
        <rdfs:comment>A coffee pack typically refers to a package containing ground coffee or coffee beans used for making coffee, usually in a drip coffee maker, espresso machine, or French press. The packaging is designed to keep the coffee fresh and flavorful, and often includes information on the type of roast, flavor profile, and origin of the coffee.</rdfs:comment>
        <rdfs:isDefinedBy rdf:resource="http://www.ease-crc.org/ont/SUTURO.owl"/>
    </owl:Class>
    


    <!-- http://www.ease-crc.org/ont/SUTURO.owl#Cola -->

    <owl:Class rdf:about="http://www.ease-crc.org/ont/SUTURO.owl#Cola">
        <rdfs:subClassOf rdf:resource="http://www.ease-crc.org/ont/SUTURO.owl#Drink"/>
        <rdfs:subClassOf rdf:resource="http://www.ease-crc.org/ont/SUTURO.owl#RoboCupDrinks"/>
        <rdfs:subClassOf>
            <owl:Restriction>
                <owl:onProperty rdf:resource="http://www.ease-crc.org/ont/SUTURO.owl#hasPredefinedName"/>
                <owl:hasValue>cola</owl:hasValue>
            </owl:Restriction>
        </rdfs:subClassOf>
        <rdfs:isDefinedBy rdf:resource="http://www.ease-crc.org/ont/SUTURO.owl"/>
    </owl:Class>
    


    <!-- http://www.ease-crc.org/ont/SUTURO.owl#ColaBottle -->

    <owl:Class rdf:about="http://www.ease-crc.org/ont/SUTURO.owl#ColaBottle">
        <rdfs:subClassOf rdf:resource="http://www.ease-crc.org/ont/SUTURO.owl#Cola"/>
        <rdfs:subClassOf rdf:resource="http://www.ease-crc.org/ont/SUTURO.owl#RoboCupDrinks"/>
        <rdfs:subClassOf>
            <owl:Restriction>
                <owl:onProperty rdf:resource="http://www.ease-crc.org/ont/SUTURO.owl#hasPredefinedName"/>
                <owl:hasValue>big coke</owl:hasValue>
            </owl:Restriction>
        </rdfs:subClassOf>
        <SUTURO:perceptionId rdf:datatype="http://www.w3.org/2001/XMLSchema#decimal">114</SUTURO:perceptionId>
        <rdfs:isDefinedBy rdf:resource="http://www.ease-crc.org/ont/SUTURO.owl"/>
    </owl:Class>
    


    <!-- http://www.ease-crc.org/ont/SUTURO.owl#ColaCan -->

    <owl:Class rdf:about="http://www.ease-crc.org/ont/SUTURO.owl#ColaCan">
        <rdfs:subClassOf rdf:resource="http://www.ease-crc.org/ont/SUTURO.owl#Can"/>
        <rdfs:subClassOf rdf:resource="http://www.ease-crc.org/ont/SUTURO.owl#Cola"/>
        <rdfs:subClassOf rdf:resource="http://www.ease-crc.org/ont/SUTURO.owl#RoboCupDrinks"/>
        <rdfs:subClassOf>
            <owl:Restriction>
                <owl:onProperty rdf:resource="http://www.ease-crc.org/ont/SUTURO.owl#hasPredefinedName"/>
                <owl:hasValue>coke</owl:hasValue>
            </owl:Restriction>
        </rdfs:subClassOf>
        <rdfs:subClassOf>
            <owl:Restriction>
                <owl:onProperty rdf:resource="http://www.ease-crc.org/ont/SUTURO.owl#hasPredefinedName"/>
                <owl:hasValue>cola can</owl:hasValue>
            </owl:Restriction>
        </rdfs:subClassOf>
        <SUTURO:perceptionId rdf:datatype="http://www.w3.org/2001/XMLSchema#int">83</SUTURO:perceptionId>
        <rdfs:comment>A cola can is a small, cylindrical container, often made of aluminum, used for holding and distributing carbonated soft drinks, particularly cola. It features a pull-tab or stay-on-tab at the top for easy opening and consumption, and is popular for its portability and recyclability.</rdfs:comment>
        <rdfs:isDefinedBy rdf:resource="http://www.ease-crc.org/ont/SUTURO.owl"/>
    </owl:Class>
    


    <!-- http://www.ease-crc.org/ont/SUTURO.owl#ColoredWoodBlock -->

    <owl:Class rdf:about="http://www.ease-crc.org/ont/SUTURO.owl#ColoredWoodBlock">
        <rdfs:subClassOf rdf:resource="http://www.ease-crc.org/ont/SUTURO.owl#WoodBlock"/>
        <rdfs:subClassOf>
            <owl:Restriction>
                <owl:onProperty rdf:resource="http://www.ease-crc.org/ont/SUTURO.owl#hasPredefinedName"/>
                <owl:hasValue>colored wood block</owl:hasValue>
            </owl:Restriction>
        </rdfs:subClassOf>
        <rdfs:comment>Colored wood blocks are toys that consist of various sized wooden blocks that are painted in different colors and shapes for children to play with.</rdfs:comment>
        <rdfs:isDefinedBy rdf:resource="http://www.ease-crc.org/ont/SUTURO.owl"/>
    </owl:Class>
    


    <!-- http://www.ease-crc.org/ont/SUTURO.owl#Condiment -->

    <owl:Class rdf:about="http://www.ease-crc.org/ont/SUTURO.owl#Condiment">
        <rdfs:subClassOf rdf:resource="http://www.ease-crc.org/ont/SUTURO.owl#ProcessedFood"/>
        <rdfs:subClassOf>
            <owl:Restriction>
                <owl:onProperty rdf:resource="http://www.ease-crc.org/ont/SUTURO.owl#hasPredefinedName"/>
                <owl:hasValue>condiment</owl:hasValue>
            </owl:Restriction>
        </rdfs:subClassOf>
        <rdfs:comment>A condiment is a food item, typically a sauce or seasoning, that is used to enhance the flavor of other foods. Examples of condiments include ketchup, mustard, mayonnaise, soy sauce, and hot sauce.</rdfs:comment>
    </owl:Class>
    


    <!-- http://www.ease-crc.org/ont/SUTURO.owl#Cookie -->

    <owl:Class rdf:about="http://www.ease-crc.org/ont/SUTURO.owl#Cookie">
        <rdfs:subClassOf rdf:resource="http://www.ease-crc.org/ont/SUTURO.owl#Sweets"/>
        <rdfs:subClassOf>
            <owl:Restriction>
                <owl:onProperty rdf:resource="http://www.ease-crc.org/ont/SUTURO.owl#hasPredefinedName"/>
                <owl:hasValue>cookie</owl:hasValue>
            </owl:Restriction>
        </rdfs:subClassOf>
        <rdfs:comment>Cookies are baked sweet treats that are typically small, flat, and round in shape, and can be crispy, chewy, or soft. They are made from a dough that typically contains flour, sugar, eggs, and butter or oil, and can be flavored with ingredients such as chocolate chips, nuts, or spices.</rdfs:comment>
        <rdfs:isDefinedBy rdf:resource="http://www.ease-crc.org/ont/SUTURO.owl"/>
    </owl:Class>
    


    <!-- http://www.ease-crc.org/ont/SUTURO.owl#CookieBox -->

    <owl:Class rdf:about="http://www.ease-crc.org/ont/SUTURO.owl#CookieBox">
        <rdfs:subClassOf rdf:resource="http://www.ease-crc.org/ont/SOMA.owl#Box"/>
        <rdfs:subClassOf>
            <owl:Restriction>
                <owl:onProperty rdf:resource="http://www.ease-crc.org/ont/SUTURO.owl#hasPredefinedName"/>
                <owl:hasValue>cookie box</owl:hasValue>
            </owl:Restriction>
        </rdfs:subClassOf>
        <rdfs:comment>A cookie box is a container made of cardboard or other materials that is used to store and transport cookies. It usually has a lid that can be opened and closed for easy access to the cookies inside.</rdfs:comment>
        <rdfs:isDefinedBy rdf:resource="http://www.ease-crc.org/ont/SUTURO.owl"/>
    </owl:Class>
    


    <!-- http://www.ease-crc.org/ont/SUTURO.owl#CookieMix -->

    <owl:Class rdf:about="http://www.ease-crc.org/ont/SUTURO.owl#CookieMix">
        <rdfs:subClassOf rdf:resource="http://www.ease-crc.org/ont/SUTURO.owl#Sweets"/>
        <rdfs:subClassOf>
            <owl:Restriction>
                <owl:onProperty rdf:resource="http://www.ease-crc.org/ont/SUTURO.owl#hasPredefinedName"/>
                <owl:hasValue>cookie mix</owl:hasValue>
            </owl:Restriction>
        </rdfs:subClassOf>
        <rdfs:comment>A cookie mix is a pre-made dry mix that typically contains flour, sugar, baking powder or soda, and sometimes additional flavorings or ingredients such as chocolate chips, nuts, or dried fruit. It is used to make cookie dough quickly and easily by adding liquid ingredients such as eggs, butter, or oil, and can be baked into a variety of cookie shapes and flavors.</rdfs:comment>
        <rdfs:isDefinedBy rdf:resource="http://www.ease-crc.org/ont/SUTURO.owl"/>
    </owl:Class>
    


    <!-- http://www.ease-crc.org/ont/SUTURO.owl#Cornflakes -->

    <owl:Class rdf:about="http://www.ease-crc.org/ont/SUTURO.owl#Cornflakes">
        <rdfs:subClassOf rdf:resource="http://www.ease-crc.org/ont/SUTURO.owl#Cereal"/>
        <rdfs:subClassOf rdf:resource="http://www.ease-crc.org/ont/SUTURO.owl#RoboCupFood"/>
        <rdfs:subClassOf>
            <owl:Restriction>
                <owl:onProperty rdf:resource="http://www.ease-crc.org/ont/SUTURO.owl#hasPredefinedName"/>
                <owl:hasValue>cornflakes</owl:hasValue>
            </owl:Restriction>
        </rdfs:subClassOf>
        <SUTURO:perceptionId rdf:datatype="http://www.w3.org/2001/XMLSchema#decimal">116</SUTURO:perceptionId>
        <rdfs:isDefinedBy rdf:resource="http://www.ease-crc.org/ont/SUTURO.owl"/>
    </owl:Class>
    


    <!-- http://www.ease-crc.org/ont/SUTURO.owl#CornyBox -->

    <owl:Class rdf:about="http://www.ease-crc.org/ont/SUTURO.owl#CornyBox">
        <rdfs:subClassOf rdf:resource="http://www.ease-crc.org/ont/SOMA.owl#Box"/>
        <rdfs:subClassOf rdf:resource="http://www.ease-crc.org/ont/SUTURO.owl#RoboCupSnacks"/>
        <rdfs:subClassOf>
            <owl:Restriction>
                <owl:onProperty rdf:resource="http://www.ease-crc.org/ont/SUTURO.owl#hasPredefinedName"/>
                <owl:hasValue>corny box</owl:hasValue>
            </owl:Restriction>
        </rdfs:subClassOf>
        <SUTURO:perceptionId rdf:datatype="http://www.w3.org/2001/XMLSchema#decimal">106</SUTURO:perceptionId>
        <rdfs:comment>A box that contains cereal bars named &quot;corny&quot;</rdfs:comment>
        <rdfs:isDefinedBy rdf:resource="http://www.ease-crc.org/ont/SOMA-HOME.owl"/>
    </owl:Class>
    


    <!-- http://www.ease-crc.org/ont/SUTURO.owl#Couch -->

    <owl:Class rdf:about="http://www.ease-crc.org/ont/SUTURO.owl#Couch">
        <rdfs:subClassOf rdf:resource="http://www.ease-crc.org/ont/SOMA.owl#DesignedFurniture"/>
        <rdfs:subClassOf>
            <owl:Restriction>
                <owl:onProperty rdf:resource="http://www.ease-crc.org/ont/SUTURO.owl#hasPredefinedName"/>
                <owl:hasValue>couch</owl:hasValue>
            </owl:Restriction>
        </rdfs:subClassOf>
        <rdfs:isDefinedBy rdf:resource="http://www.ease-crc.org/ont/SUTURO.owl"/>
    </owl:Class>
    


    <!-- http://www.ease-crc.org/ont/SUTURO.owl#CouchTable -->

    <owl:Class rdf:about="http://www.ease-crc.org/ont/SUTURO.owl#CouchTable">
        <rdfs:subClassOf rdf:resource="http://www.ease-crc.org/ont/SOMA.owl#Table"/>
        <rdfs:subClassOf>
            <owl:Restriction>
                <owl:onProperty rdf:resource="http://www.ease-crc.org/ont/SUTURO.owl#hasPredefinedName"/>
                <owl:hasValue>couch table</owl:hasValue>
            </owl:Restriction>
        </rdfs:subClassOf>
        <rdfs:comment rdf:resource="http://www.ease-crc.org/ont/SUTURO.owl"/>
    </owl:Class>
    


    <!-- http://www.ease-crc.org/ont/SUTURO.owl#CrackerBox -->

    <owl:Class rdf:about="http://www.ease-crc.org/ont/SUTURO.owl#CrackerBox">
        <rdfs:subClassOf rdf:resource="http://www.ease-crc.org/ont/SOMA.owl#Box"/>
        <rdfs:subClassOf rdf:resource="http://www.ease-crc.org/ont/SUTURO.owl#RoboCupSnacks"/>
        <rdfs:subClassOf>
            <owl:Restriction>
                <owl:onProperty rdf:resource="http://www.ease-crc.org/ont/SUTURO.owl#hasPredefinedName"/>
                <owl:hasValue>cracker box</owl:hasValue>
            </owl:Restriction>
        </rdfs:subClassOf>
        <SUTURO:perceptionId rdf:datatype="http://www.w3.org/2001/XMLSchema#int">10</SUTURO:perceptionId>
        <rdfs:comment>A box containing, or at least intended to contain, crackers. A cracker is a flat, dry-baked pastry, usually made from flour.</rdfs:comment>
        <rdfs:isDefinedBy rdf:resource="http://www.ease-crc.org/ont/SUTURO.owl"/>
    </owl:Class>
    


    <!-- http://www.ease-crc.org/ont/SUTURO.owl#CreditCard -->

    <owl:Class rdf:about="http://www.ease-crc.org/ont/SUTURO.owl#CreditCard">
        <rdfs:subClassOf rdf:resource="http://www.ease-crc.org/ont/SOMA.owl#DesignedTool"/>
        <rdfs:subClassOf>
            <owl:Restriction>
                <owl:onProperty rdf:resource="http://www.ease-crc.org/ont/SUTURO.owl#hasPredefinedName"/>
                <owl:hasValue>credit card</owl:hasValue>
            </owl:Restriction>
        </rdfs:subClassOf>
        <rdfs:comment>A credit card is a standard-size rectangular piece of plastic. It is a payment card that allows the cardholder to borrow funds from a financial institution to make purchases and pay them back with interest over time.</rdfs:comment>
        <rdfs:isDefinedBy rdf:resource="http://www.ease-crc.org/ont/SUTURO.owl"/>
    </owl:Class>
    


    <!-- http://www.ease-crc.org/ont/SUTURO.owl#CrispsBag -->

    <owl:Class rdf:about="http://www.ease-crc.org/ont/SUTURO.owl#CrispsBag">
        <rdfs:subClassOf rdf:resource="http://www.ease-crc.org/ont/SUTURO.owl#Bag"/>
        <rdfs:subClassOf rdf:resource="http://www.ease-crc.org/ont/SUTURO.owl#RoboCupSnacks"/>
        <rdfs:subClassOf>
            <owl:Restriction>
                <owl:onProperty rdf:resource="http://www.ease-crc.org/ont/SUTURO.owl#hasPredefinedName"/>
                <owl:hasValue>crips</owl:hasValue>
            </owl:Restriction>
        </rdfs:subClassOf>
        <SUTURO:perceptionId rdf:datatype="http://www.w3.org/2001/XMLSchema#decimal">122</SUTURO:perceptionId>
        <rdfs:isDefinedBy rdf:resource="http://www.ease-crc.org/ont/SUTURO.owl"/>
    </owl:Class>
    


    <!-- http://www.ease-crc.org/ont/SUTURO.owl#CupBlue -->

    <owl:Class rdf:about="http://www.ease-crc.org/ont/SUTURO.owl#CupBlue">
        <rdfs:subClassOf rdf:resource="http://www.ease-crc.org/ont/SOMA.owl#Cup"/>
        <SUTURO:perceptionId rdf:datatype="http://www.w3.org/2001/XMLSchema#decimal">94</SUTURO:perceptionId>
        <rdfs:isDefinedBy rdf:resource="http://www.ease-crc.org/ont/SUTURO.owl"/>
    </owl:Class>
    


    <!-- http://www.ease-crc.org/ont/SUTURO.owl#CupGreen -->

    <owl:Class rdf:about="http://www.ease-crc.org/ont/SUTURO.owl#CupGreen">
        <rdfs:subClassOf rdf:resource="http://www.ease-crc.org/ont/SOMA.owl#Cup"/>
        <SUTURO:perceptionId rdf:datatype="http://www.w3.org/2001/XMLSchema#decimal">95</SUTURO:perceptionId>
        <rdfs:isDefinedBy rdf:resource="http://www.ease-crc.org/ont/SUTURO.owl"/>
    </owl:Class>
    


    <!-- http://www.ease-crc.org/ont/SUTURO.owl#CupSmall -->

    <owl:Class rdf:about="http://www.ease-crc.org/ont/SUTURO.owl#CupSmall">
        <rdfs:subClassOf rdf:resource="http://www.ease-crc.org/ont/SOMA.owl#Cup"/>
        <SUTURO:perceptionId rdf:datatype="http://www.w3.org/2001/XMLSchema#decimal">101</SUTURO:perceptionId>
        <rdfs:isDefinedBy rdf:resource="http://www.ease-crc.org/ont/SUTURO.owl"/>
    </owl:Class>
    


    <!-- http://www.ease-crc.org/ont/SUTURO.owl#Curry -->

    <owl:Class rdf:about="http://www.ease-crc.org/ont/SUTURO.owl#Curry">
        <rdfs:subClassOf rdf:resource="http://www.ease-crc.org/ont/SUTURO.owl#ProcessedFood"/>
        <rdfs:subClassOf rdf:resource="http://www.ease-crc.org/ont/SUTURO.owl#RoboCupFood"/>
        <rdfs:subClassOf>
            <owl:Restriction>
                <owl:onProperty rdf:resource="http://www.ease-crc.org/ont/SUTURO.owl#hasPredefinedName"/>
                <owl:hasValue>curry</owl:hasValue>
            </owl:Restriction>
        </rdfs:subClassOf>
        <SUTURO:perceptionId rdf:datatype="http://www.w3.org/2001/XMLSchema#decimal">117</SUTURO:perceptionId>
        <rdfs:isDefinedBy rdf:resource="http://www.ease-crc.org/ont/SUTURO.owl"/>
    </owl:Class>
    


    <!-- http://www.ease-crc.org/ont/SUTURO.owl#Customer -->

    <owl:Class rdf:about="http://www.ease-crc.org/ont/SUTURO.owl#Customer">
        <rdfs:subClassOf rdf:resource="http://www.ontologydesignpatterns.org/ont/dul/DUL.owl#NaturalPerson"/>
        <rdfs:comment>A customer is a person, whose name we know.</rdfs:comment>
        <rdfs:isDefinedBy rdf:resource="http://www.ease-crc.org/ont/SUTURO.owl"/>
    </owl:Class>
    


    <!-- http://www.ease-crc.org/ont/SUTURO.owl#Customer_ID -->

    <owl:Class rdf:about="http://www.ease-crc.org/ont/SUTURO.owl#Customer_ID">
        <rdfs:subClassOf rdf:resource="http://www.ease-crc.org/ont/SUTURO.owl#Customer"/>
        <rdfs:comment>An id for every customer we meet.</rdfs:comment>
        <rdfs:isDefinedBy rdf:resource="http://www.ease-crc.org/ont/SUTURO.owl"/>
    </owl:Class>
    


    <!-- http://www.ease-crc.org/ont/SUTURO.owl#CuttingBoard -->

    <owl:Class rdf:about="http://www.ease-crc.org/ont/SUTURO.owl#CuttingBoard">
        <rdfs:subClassOf rdf:resource="http://www.ease-crc.org/ont/SOMA.owl#CuttingTool"/>
        <rdfs:subClassOf>
            <owl:Restriction>
                <owl:onProperty rdf:resource="http://www.ease-crc.org/ont/SUTURO.owl#hasPredefinedName"/>
                <owl:hasValue>cutting board</owl:hasValue>
            </owl:Restriction>
        </rdfs:subClassOf>
        <rdfs:isDefinedBy rdf:resource="http://www.ease-crc.org/ont/SUTURO.owl"/>
    </owl:Class>
    


    <!-- http://www.ease-crc.org/ont/SUTURO.owl#Decorations -->

    <owl:Class rdf:about="http://www.ease-crc.org/ont/SUTURO.owl#Decorations">
        <rdfs:subClassOf rdf:resource="http://www.ease-crc.org/ont/SUTURO.owl#RoboCup2023Categories"/>
    </owl:Class>
    


    <!-- http://www.ease-crc.org/ont/SUTURO.owl#DesignedFabric -->

    <owl:Class rdf:about="http://www.ease-crc.org/ont/SUTURO.owl#DesignedFabric">
        <rdfs:subClassOf rdf:resource="http://www.ontologydesignpatterns.org/ont/dul/DUL.owl#DesignedArtifact"/>
        <rdfs:comment>Fabric is a flexible, woven material consisting of a network of natural or artificial fibers, often used for making clothing and other textile products.</rdfs:comment>
        <rdfs:isDefinedBy rdf:resource="http://www.ease-crc.org/ont/SUTURO.owl"/>
        <rdfs:label>Designed fabric</rdfs:label>
    </owl:Class>
    


    <!-- http://www.ease-crc.org/ont/SUTURO.owl#Dice -->

    <owl:Class rdf:about="http://www.ease-crc.org/ont/SUTURO.owl#Dice">
        <rdfs:subClassOf rdf:resource="http://www.ease-crc.org/ont/SUTURO.owl#Toy"/>
        <rdfs:subClassOf>
            <owl:Restriction>
                <owl:onProperty rdf:resource="http://www.ease-crc.org/ont/SUTURO.owl#hasPredefinedName"/>
                <owl:hasValue>dice</owl:hasValue>
            </owl:Restriction>
        </rdfs:subClassOf>
        <SUTURO:perceptionId rdf:datatype="http://www.w3.org/2001/XMLSchema#int">54</SUTURO:perceptionId>
        <rdfs:comment>Dice are small, cube-shaped objects with markings on each face, typically used in games of chance and gambling, to generate random numbers, or for other recreational purposes.</rdfs:comment>
        <rdfs:isDefinedBy rdf:resource="http://www.ease-crc.org/ont/SUTURO.owl"/>
    </owl:Class>
    


    <!-- http://www.ease-crc.org/ont/SUTURO.owl#DiningRoom -->

    <owl:Class rdf:about="http://www.ease-crc.org/ont/SUTURO.owl#DiningRoom">
        <rdfs:subClassOf rdf:resource="http://www.ease-crc.org/ont/SOMA.owl#Room"/>
        <rdfs:subClassOf>
            <owl:Restriction>
                <owl:onProperty rdf:resource="http://www.ease-crc.org/ont/SUTURO.owl#hasPredefinedName"/>
                <owl:hasValue>dining room</owl:hasValue>
            </owl:Restriction>
        </rdfs:subClassOf>
        <rdfs:isDefinedBy rdf:resource="http://www.ease-crc.org/ont/SUTURO.owl"/>
    </owl:Class>
    


    <!-- http://www.ease-crc.org/ont/SUTURO.owl#DiningTable -->

    <owl:Class rdf:about="http://www.ease-crc.org/ont/SUTURO.owl#DiningTable">
        <rdfs:subClassOf rdf:resource="http://www.ease-crc.org/ont/SOMA.owl#Table"/>
        <rdfs:subClassOf>
            <owl:Restriction>
                <owl:onProperty rdf:resource="http://www.ease-crc.org/ont/SUTURO.owl#hasPredefinedName"/>
                <owl:hasValue>dining table</owl:hasValue>
            </owl:Restriction>
        </rdfs:subClassOf>
        <rdfs:comment>A table mainly used for dining. Often placed inside of a living room.</rdfs:comment>
        <rdfs:isDefinedBy rdf:resource="http://www.ease-crc.org/ont/SUTURO.owl"/>
    </owl:Class>
    


    <!-- http://www.ease-crc.org/ont/SUTURO.owl#DishwasherTray -->

    <owl:Class rdf:about="http://www.ease-crc.org/ont/SUTURO.owl#DishwasherTray">
        <rdfs:subClassOf rdf:resource="http://www.ease-crc.org/ont/SOMA.owl#Drawer"/>
        <rdfs:subClassOf>
            <owl:Restriction>
                <owl:onProperty rdf:resource="http://www.ease-crc.org/ont/SUTURO.owl#hasPredefinedName"/>
                <owl:hasValue>dishwasher tray</owl:hasValue>
            </owl:Restriction>
        </rdfs:subClassOf>
        <rdfs:comment>A dishwasher tray is a removable component in a dishwasher that holds dishes, glasses, and utensils during the washing cycle. It is designed with compartments and prongs to securely position and separate items for efficient cleaning.</rdfs:comment>
        <rdfs:isDefinedBy rdf:resource="http://www.ease-crc.org/ont/SUTURO.owl"/>
    </owl:Class>
    


    <!-- http://www.ease-crc.org/ont/SUTURO.owl#DominoSugarBox -->

    <owl:Class rdf:about="http://www.ease-crc.org/ont/SUTURO.owl#DominoSugarBox">
        <rdfs:subClassOf rdf:resource="http://www.ease-crc.org/ont/SUTURO.owl#SugarBox"/>
        <rdfs:subClassOf>
            <owl:Restriction>
                <owl:onProperty rdf:resource="http://www.ease-crc.org/ont/SUTURO.owl#hasPredefinedName"/>
                <owl:hasValue>domino sugar box</owl:hasValue>
            </owl:Restriction>
        </rdfs:subClassOf>
        <rdfs:comment>A box containing, or at least usually intended to contain, Domino brand sugar.</rdfs:comment>
        <rdfs:isDefinedBy rdf:resource="http://www.ease-crc.org/ont/SUTURO.owl"/>
    </owl:Class>
    


    <!-- http://www.ease-crc.org/ont/SUTURO.owl#Dress -->

    <owl:Class rdf:about="http://www.ease-crc.org/ont/SUTURO.owl#Dress">
        <rdfs:subClassOf rdf:resource="http://www.ease-crc.org/ont/SUTURO.owl#Clothing"/>
        <rdfs:subClassOf>
            <owl:Restriction>
                <owl:onProperty rdf:resource="http://www.ease-crc.org/ont/SUTURO.owl#hasPredefinedName"/>
                <owl:hasValue>dress</owl:hasValue>
            </owl:Restriction>
        </rdfs:subClassOf>
        <rdfs:isDefinedBy rdf:resource="http://www.ease-crc.org/ont/SUTURO.owl"/>
    </owl:Class>
    


    <!-- http://www.ease-crc.org/ont/SUTURO.owl#Drink -->

    <owl:Class rdf:about="http://www.ease-crc.org/ont/SUTURO.owl#Drink">
        <rdfs:subClassOf rdf:resource="http://www.ease-crc.org/ont/SUTURO.owl#Liquid"/>
        <rdfs:subClassOf>
            <owl:Restriction>
                <owl:onProperty rdf:resource="http://www.ease-crc.org/ont/SUTURO.owl#hasPredefinedName"/>
                <owl:hasValue>drink</owl:hasValue>
            </owl:Restriction>
        </rdfs:subClassOf>
        <rdfs:comment>A drink is a liquid that is consumed for the purpose of quenching thirst, providing hydration, or for enjoyment. Drinks can be alcoholic or non-alcoholic and can be served hot or cold, and come in a wide variety of flavors and types.</rdfs:comment>
        <rdfs:isDefinedBy rdf:resource="http://www.ease-crc.org/ont/SUTURO.owl"/>
    </owl:Class>
    


    <!-- http://www.ease-crc.org/ont/SUTURO.owl#DubbelFris -->

    <owl:Class rdf:about="http://www.ease-crc.org/ont/SUTURO.owl#DubbelFris">
        <rdfs:subClassOf rdf:resource="http://www.ease-crc.org/ont/SUTURO.owl#AppleJuice"/>
        <rdfs:subClassOf rdf:resource="http://www.ease-crc.org/ont/SUTURO.owl#RoboCupDrinks"/>
        <rdfs:subClassOf>
            <owl:Restriction>
                <owl:onProperty rdf:resource="http://www.ease-crc.org/ont/SUTURO.owl#hasPredefinedName"/>
                <owl:hasValue>dubbelfris</owl:hasValue>
            </owl:Restriction>
        </rdfs:subClassOf>
        <SUTURO:perceptionId rdf:datatype="http://www.w3.org/2001/XMLSchema#decimal">112</SUTURO:perceptionId>
        <rdfs:isDefinedBy rdf:resource="http://www.ease-crc.org/ont/SUTURO.owl"/>
    </owl:Class>
    


    <!-- http://www.ease-crc.org/ont/SUTURO.owl#Fanta -->

    <owl:Class rdf:about="http://www.ease-crc.org/ont/SUTURO.owl#Fanta">
        <rdfs:subClassOf rdf:resource="http://www.ease-crc.org/ont/SUTURO.owl#Drink"/>
        <rdfs:subClassOf rdf:resource="http://www.ease-crc.org/ont/SUTURO.owl#RoboCupDrinks"/>
    </owl:Class>
    


    <!-- http://www.ease-crc.org/ont/SUTURO.owl#FantaCan -->

    <owl:Class rdf:about="http://www.ease-crc.org/ont/SUTURO.owl#FantaCan">
        <rdfs:subClassOf rdf:resource="http://www.ease-crc.org/ont/SUTURO.owl#Fanta"/>
        <rdfs:subClassOf rdf:resource="http://www.ease-crc.org/ont/SUTURO.owl#RoboCupDrinks"/>
        <rdfs:subClassOf>
            <owl:Restriction>
                <owl:onProperty rdf:resource="http://www.ease-crc.org/ont/SUTURO.owl#hasPredefinedName"/>
                <owl:hasValue>fanta</owl:hasValue>
            </owl:Restriction>
        </rdfs:subClassOf>
        <SUTURO:perceptionId rdf:datatype="http://www.w3.org/2001/XMLSchema#decimal">110</SUTURO:perceptionId>
        <rdfs:isDefinedBy rdf:resource="http://www.ease-crc.org/ont/SUTURO.owl"/>
    </owl:Class>
    


    <!-- http://www.ease-crc.org/ont/SUTURO.owl#Fastener -->

    <owl:Class rdf:about="http://www.ease-crc.org/ont/SUTURO.owl#Fastener">
        <rdfs:subClassOf rdf:resource="http://www.ease-crc.org/ont/SUTURO.owl#HouseholdHardware"/>
        <rdfs:subClassOf>
            <owl:Restriction>
                <owl:onProperty rdf:resource="http://www.ease-crc.org/ont/SUTURO.owl#hasPredefinedName"/>
                <owl:hasValue>fastener</owl:hasValue>
            </owl:Restriction>
        </rdfs:subClassOf>
        <rdfs:comment>A fastener is a hardware device used to join two or more objects together, allowing for the creation of non-permanent joints that can be easily removed or disassembled.</rdfs:comment>
        <rdfs:isDefinedBy rdf:resource="http://www.ease-crc.org/ont/SUTURO.owl"/>
    </owl:Class>
    


    <!-- http://www.ease-crc.org/ont/SUTURO.owl#Fish -->

    <owl:Class rdf:about="http://www.ease-crc.org/ont/SUTURO.owl#Fish">
        <rdfs:subClassOf rdf:resource="http://www.ease-crc.org/ont/SUTURO.owl#Food"/>
        <rdfs:subClassOf>
            <owl:Restriction>
                <owl:onProperty rdf:resource="http://www.ease-crc.org/ont/SUTURO.owl#hasPredefinedName"/>
                <owl:hasValue>fish</owl:hasValue>
            </owl:Restriction>
        </rdfs:subClassOf>
        <rdfs:comment>Fish are aquatic animals that are found in oceans, rivers, lakes, and other bodies of water. They come in a variety of shapes, sizes, and colors and are an important food source for humans and many other animals.</rdfs:comment>
        <rdfs:isDefinedBy rdf:resource="http://www.ease-crc.org/ont/SUTURO.owl"/>
    </owl:Class>
    


    <!-- http://www.ease-crc.org/ont/SUTURO.owl#FlatScrewdriver -->

    <owl:Class rdf:about="http://www.ease-crc.org/ont/SUTURO.owl#FlatScrewdriver">
        <rdfs:subClassOf rdf:resource="http://www.ease-crc.org/ont/SUTURO.owl#ScrewDriver"/>
        <rdfs:comment>A flat screwdriver is a hand tool characterized by a flat and narrow blade with a tip that fits into slotted screw heads. It is used for turning or tightening screws that have a single straight slot, commonly found in various mechanical and household applications.</rdfs:comment>
        <rdfs:isDefinedBy rdf:resource="http://www.ease-crc.org/ont/SUTURO.owl"/>
    </owl:Class>
    


    <!-- http://www.ease-crc.org/ont/SUTURO.owl#Flavor -->

    <owl:Class rdf:about="http://www.ease-crc.org/ont/SUTURO.owl#Flavor">
        <rdfs:subClassOf rdf:resource="http://www.ease-crc.org/ont/SOMA.owl#Intrinsic"/>
        <rdfs:comment>Flavor refers to the sensory experience of food or drink, specifically its taste and aroma.</rdfs:comment>
        <rdfs:isDefinedBy rdf:resource="http://www.ease-crc.org/ont/SUTURO.owl"/>
    </owl:Class>
    


    <!-- http://www.ease-crc.org/ont/SUTURO.owl#FoamBrick -->

    <owl:Class rdf:about="http://www.ease-crc.org/ont/SUTURO.owl#FoamBrick">
        <rdfs:subClassOf rdf:resource="http://www.ease-crc.org/ont/SUTURO.owl#Block"/>
        <rdfs:subClassOf>
            <owl:Restriction>
                <owl:onProperty rdf:resource="http://www.ease-crc.org/ont/SUTURO.owl#hasPredefinedName"/>
                <owl:hasValue>foam brick</owl:hasValue>
            </owl:Restriction>
        </rdfs:subClassOf>
        <SUTURO:perceptionId rdf:datatype="http://www.w3.org/2001/XMLSchema#int">4</SUTURO:perceptionId>
        <rdfs:comment>A foam brick is a soft, rectangular block made of foam, used for support or cushioning, often in sports or fitness activities.</rdfs:comment>
        <rdfs:isDefinedBy rdf:resource="http://www.ease-crc.org/ont/SUTURO.owl"/>
    </owl:Class>
    


    <!-- http://www.ease-crc.org/ont/SUTURO.owl#Food -->

    <owl:Class rdf:about="http://www.ease-crc.org/ont/SUTURO.owl#Food">
        <rdfs:subClassOf rdf:resource="http://www.ontologydesignpatterns.org/ont/dul/DUL.owl#BiologicalObject"/>
        <rdfs:comment>Food refers to any substance consumed by living organisms that provide nutritional support for the body&apos;s growth, development, and maintenance.</rdfs:comment>
        <rdfs:isDefinedBy rdf:resource="http://www.ease-crc.org/ont/SUTURO.owl"/>
    </owl:Class>
    


    <!-- http://www.ease-crc.org/ont/SUTURO.owl#Footlocker -->

    <owl:Class rdf:about="http://www.ease-crc.org/ont/SUTURO.owl#Footlocker">
        <rdfs:subClassOf rdf:resource="http://www.ease-crc.org/ont/SOMA.owl#DesignedContainer"/>
        <rdfs:comment>A type of storage trunk used to hold clothing and other personal items.</rdfs:comment>
        <rdfs:isDefinedBy rdf:resource="http://www.ease-crc.org/ont/SUTURO.owl"/>
    </owl:Class>
    


    <!-- http://www.ease-crc.org/ont/SUTURO.owl#ForceConcentratingTool -->

    <owl:Class rdf:about="http://www.ease-crc.org/ont/SUTURO.owl#ForceConcentratingTool">
        <rdfs:subClassOf rdf:resource="http://www.ease-crc.org/ont/SOMA.owl#DesignedTool"/>
        <rdfs:comment>Force-concentrating tools are hand tools designed to concentrate a force onto a small area to enable the user to exert a greater amount of force than would otherwise be possible.</rdfs:comment>
        <rdfs:isDefinedBy rdf:resource="http://www.ease-crc.org/ont/SUTURO.owl"/>
    </owl:Class>
    


    <!-- http://www.ease-crc.org/ont/SUTURO.owl#Fragility -->

    <owl:Class rdf:about="http://www.ease-crc.org/ont/SUTURO.owl#Fragility">
        <rdfs:subClassOf rdf:resource="http://www.ease-crc.org/ont/SOMA.owl#Disposition"/>
    </owl:Class>
    


    <!-- http://www.ease-crc.org/ont/SUTURO.owl#FrenchsYellowMustardBottle -->

    <owl:Class rdf:about="http://www.ease-crc.org/ont/SUTURO.owl#FrenchsYellowMustardBottle">
        <rdfs:subClassOf rdf:resource="http://www.ease-crc.org/ont/SUTURO.owl#MustardBottle"/>
        <rdfs:subClassOf>
            <owl:Restriction>
                <owl:onProperty rdf:resource="http://www.ease-crc.org/ont/SUTURO.owl#hasPredefinedName"/>
                <owl:hasValue>frenchs yellow mustard bottle</owl:hasValue>
            </owl:Restriction>
        </rdfs:subClassOf>
        <rdfs:comment>French&apos;s Mustard bottle refers to a squeezable container that dispenses French&apos;s brand of yellow mustard.</rdfs:comment>
        <rdfs:isDefinedBy rdf:resource="http://www.ease-crc.org/ont/SUTURO.owl"/>
    </owl:Class>
    


    <!-- http://www.ease-crc.org/ont/SUTURO.owl#Fruit -->

    <owl:Class rdf:about="http://www.ease-crc.org/ont/SUTURO.owl#Fruit">
        <rdfs:subClassOf rdf:resource="http://www.ease-crc.org/ont/SUTURO.owl#Food"/>
        <rdfs:subClassOf>
            <owl:Restriction>
                <owl:onProperty rdf:resource="http://www.ease-crc.org/ont/SUTURO.owl#isInRoom"/>
                <owl:allValuesFrom rdf:resource="http://www.ease-crc.org/ont/SOMA.owl#Kitchen"/>
            </owl:Restriction>
        </rdfs:subClassOf>
        <rdfs:subClassOf>
            <owl:Restriction>
                <owl:onProperty rdf:resource="http://www.ease-crc.org/ont/SUTURO.owl#hasPredefinedName"/>
                <owl:hasValue>fruit</owl:hasValue>
            </owl:Restriction>
        </rdfs:subClassOf>
        <rdfs:comment>Fruit is the sweet and fleshy product of a tree or other plant that contains seed and can be eaten as food.</rdfs:comment>
        <rdfs:isDefinedBy rdf:resource="http://www.ease-crc.org/ont/SUTURO.owl"/>
    </owl:Class>
    


    <!-- http://www.ease-crc.org/ont/SUTURO.owl#GelatineBox -->

    <owl:Class rdf:about="http://www.ease-crc.org/ont/SUTURO.owl#GelatineBox">
        <rdfs:subClassOf rdf:resource="http://www.ease-crc.org/ont/SOMA.owl#Box"/>
        <rdfs:subClassOf>
            <owl:Restriction>
                <owl:onProperty rdf:resource="http://www.ease-crc.org/ont/SUTURO.owl#hasPredefinedName"/>
                <owl:hasValue>gelatine box</owl:hasValue>
            </owl:Restriction>
        </rdfs:subClassOf>
        <SUTURO:perceptionId rdf:datatype="http://www.w3.org/2001/XMLSchema#decimal">72</SUTURO:perceptionId>
        <rdfs:isDefinedBy rdf:resource="http://www.ease-crc.org/ont/SUTURO.owl"/>
    </owl:Class>
    


    <!-- http://www.ease-crc.org/ont/SUTURO.owl#GinTonic -->

    <owl:Class rdf:about="http://www.ease-crc.org/ont/SUTURO.owl#GinTonic">
        <rdfs:subClassOf rdf:resource="http://www.ease-crc.org/ont/SUTURO.owl#Drink"/>
        <rdfs:subClassOf>
            <owl:Restriction>
                <owl:onProperty rdf:resource="http://www.ease-crc.org/ont/SUTURO.owl#hasPredefinedName"/>
                <owl:hasValue>gin tonic</owl:hasValue>
            </owl:Restriction>
        </rdfs:subClassOf>
        <rdfs:isDefinedBy rdf:resource="http://www.ease-crc.org/ont/SUTURO.owl"/>
    </owl:Class>
    


    <!-- http://www.ease-crc.org/ont/SUTURO.owl#GingerAle -->

    <owl:Class rdf:about="http://www.ease-crc.org/ont/SUTURO.owl#GingerAle">
        <rdfs:subClassOf rdf:resource="http://www.ease-crc.org/ont/SUTURO.owl#Drink"/>
        <rdfs:subClassOf>
            <owl:Restriction>
                <owl:onProperty rdf:resource="http://www.ease-crc.org/ont/SUTURO.owl#hasPredefinedName"/>
                <owl:hasValue>ginger ale</owl:hasValue>
            </owl:Restriction>
        </rdfs:subClassOf>
        <rdfs:isDefinedBy rdf:resource="http://www.ease-crc.org/ont/SUTURO.owl"/>
    </owl:Class>
    


    <!-- http://www.ease-crc.org/ont/SUTURO.owl#GlassCleanerSprayBottle -->

    <owl:Class rdf:about="http://www.ease-crc.org/ont/SUTURO.owl#GlassCleanerSprayBottle">
        <rdfs:subClassOf rdf:resource="http://www.ease-crc.org/ont/SUTURO.owl#SprayBottle"/>
        <rdfs:subClassOf>
            <owl:Restriction>
                <owl:onProperty rdf:resource="http://www.ease-crc.org/ont/SUTURO.owl#hasPredefinedName"/>
                <owl:hasValue>glass cleaner spray bottle</owl:hasValue>
            </owl:Restriction>
        </rdfs:subClassOf>
        <SUTURO:perceptionId rdf:datatype="http://www.w3.org/2001/XMLSchema#int">38</SUTURO:perceptionId>
        <rdfs:comment>A glass cleaner spray bottle is a container designed to hold a cleaning solution specifically formulated for cleaning glass surfaces. It typically has a spray nozzle that dispenses the solution in a fine mist for easy application onto the surface.</rdfs:comment>
        <rdfs:isDefinedBy rdf:resource="http://www.ease-crc.org/ont/SUTURO.owl"/>
    </owl:Class>
    


    <!-- http://www.ease-crc.org/ont/SUTURO.owl#Gloves -->

    <owl:Class rdf:about="http://www.ease-crc.org/ont/SUTURO.owl#Gloves">
        <rdfs:subClassOf rdf:resource="http://www.ease-crc.org/ont/SUTURO.owl#Clothing"/>
        <rdfs:subClassOf>
            <owl:Restriction>
                <owl:onProperty rdf:resource="http://www.ease-crc.org/ont/SUTURO.owl#hasPredefinedName"/>
                <owl:hasValue>gloves</owl:hasValue>
            </owl:Restriction>
        </rdfs:subClassOf>
        <rdfs:isDefinedBy rdf:resource="http://www.ease-crc.org/ont/SUTURO.owl"/>
    </owl:Class>
    


    <!-- http://www.ease-crc.org/ont/SUTURO.owl#GolfBall -->

    <owl:Class rdf:about="http://www.ease-crc.org/ont/SUTURO.owl#GolfBall">
        <rdfs:subClassOf rdf:resource="http://www.ease-crc.org/ont/SUTURO.owl#Ball"/>
        <rdfs:subClassOf>
            <owl:Restriction>
                <owl:onProperty rdf:resource="http://www.ease-crc.org/ont/SUTURO.owl#hasPredefinedName"/>
                <owl:hasValue>golf ball</owl:hasValue>
            </owl:Restriction>
        </rdfs:subClassOf>
        <SUTURO:perceptionId rdf:datatype="http://www.w3.org/2001/XMLSchema#int">32</SUTURO:perceptionId>
        <rdfs:comment>A golf ball is a small, round ball used in the sport of golf, typically made of rubber and synthetic materials, with dimples on its surface to increase lift and reduce drag.</rdfs:comment>
        <rdfs:isDefinedBy rdf:resource="http://www.ease-crc.org/ont/SUTURO.owl"/>
    </owl:Class>
    


    <!-- http://www.ease-crc.org/ont/SUTURO.owl#Grapes -->

    <owl:Class rdf:about="http://www.ease-crc.org/ont/SUTURO.owl#Grapes">
        <rdfs:subClassOf rdf:resource="http://www.ease-crc.org/ont/SUTURO.owl#Fruit"/>
        <rdfs:subClassOf rdf:resource="http://www.ease-crc.org/ont/SUTURO.owl#RoboCupFruits"/>
        <rdfs:subClassOf>
            <owl:Restriction>
                <owl:onProperty rdf:resource="http://www.ease-crc.org/ont/SUTURO.owl#hasPredefinedName"/>
                <owl:hasValue>grapes</owl:hasValue>
            </owl:Restriction>
        </rdfs:subClassOf>
        <SUTURO:perceptionId rdf:datatype="http://www.w3.org/2001/XMLSchema#decimal">100</SUTURO:perceptionId>
        <rdfs:comment>Grapes are small round fruits that can be green or dark purple and can have seeds inside them.</rdfs:comment>
        <rdfs:isDefinedBy rdf:resource="http://www.ease-crc.org/ont/SUTURO.owl"/>
    </owl:Class>
    


    <!-- http://www.ease-crc.org/ont/SUTURO.owl#GroceryBag -->

    <owl:Class rdf:about="http://www.ease-crc.org/ont/SUTURO.owl#GroceryBag">
        <rdfs:subClassOf rdf:resource="http://www.ease-crc.org/ont/SUTURO.owl#Bag"/>
        <rdfs:subClassOf>
            <owl:Restriction>
                <owl:onProperty rdf:resource="http://www.ease-crc.org/ont/SUTURO.owl#hasPredefinedName"/>
                <owl:hasValue>grocery bag</owl:hasValue>
            </owl:Restriction>
        </rdfs:subClassOf>
        <SUTURO:perceptionId rdf:datatype="http://www.w3.org/2001/XMLSchema#decimal">128</SUTURO:perceptionId>
        <rdfs:isDefinedBy rdf:resource="http://www.ease-crc.org/ont/SUTURO.owl"/>
    </owl:Class>
    


    <!-- http://www.ease-crc.org/ont/SUTURO.owl#Hagelslag -->

    <owl:Class rdf:about="http://www.ease-crc.org/ont/SUTURO.owl#Hagelslag">
        <rdfs:subClassOf rdf:resource="http://www.ease-crc.org/ont/SUTURO.owl#ProcessedFood"/>
        <rdfs:subClassOf rdf:resource="http://www.ease-crc.org/ont/SUTURO.owl#RoboCupFood"/>
        <rdfs:subClassOf>
            <owl:Restriction>
                <owl:onProperty rdf:resource="http://www.ease-crc.org/ont/SUTURO.owl#hasPredefinedName"/>
                <owl:hasValue>chocolate sprinkles</owl:hasValue>
            </owl:Restriction>
        </rdfs:subClassOf>
        <rdfs:subClassOf>
            <owl:Restriction>
                <owl:onProperty rdf:resource="http://www.ease-crc.org/ont/SUTURO.owl#hasPredefinedName"/>
                <owl:hasValue>hagelslag</owl:hasValue>
            </owl:Restriction>
        </rdfs:subClassOf>
        <SUTURO:perceptionId rdf:datatype="http://www.w3.org/2001/XMLSchema#decimal">119</SUTURO:perceptionId>
        <rdfs:isDefinedBy rdf:resource="http://www.ease-crc.org/ont/SUTURO.owl"/>
    </owl:Class>
    


    <!-- http://www.ease-crc.org/ont/SUTURO.owl#Hallway -->

    <owl:Class rdf:about="http://www.ease-crc.org/ont/SUTURO.owl#Hallway">
        <rdfs:subClassOf rdf:resource="http://www.ease-crc.org/ont/SOMA.owl#Room"/>
        <rdfs:subClassOf>
            <owl:Restriction>
                <owl:onProperty rdf:resource="http://www.ease-crc.org/ont/SUTURO.owl#hasPredefinedName"/>
                <owl:hasValue>hallway</owl:hasValue>
            </owl:Restriction>
        </rdfs:subClassOf>
        <rdfs:comment rdf:resource="http://www.ease-crc.org/ont/SUTURO.owl"/>
    </owl:Class>
    


    <!-- http://www.ease-crc.org/ont/SUTURO.owl#Hammer -->

    <owl:Class rdf:about="http://www.ease-crc.org/ont/SUTURO.owl#Hammer">
        <rdfs:subClassOf rdf:resource="http://www.ease-crc.org/ont/SUTURO.owl#ForceConcentratingTool"/>
        <rdfs:subClassOf>
            <owl:Restriction>
                <owl:onProperty rdf:resource="http://www.ease-crc.org/ont/SOMA.owl#hasPhysicalComponent"/>
                <owl:someValuesFrom rdf:resource="http://www.ease-crc.org/ont/SOMA.owl#DesignedHandle"/>
            </owl:Restriction>
        </rdfs:subClassOf>
        <rdfs:subClassOf>
            <owl:Restriction>
                <owl:onProperty rdf:resource="http://www.ease-crc.org/ont/SUTURO.owl#hasPredefinedName"/>
                <owl:hasValue>hammer</owl:hasValue>
            </owl:Restriction>
        </rdfs:subClassOf>
        <SUTURO:perceptionId rdf:datatype="http://www.w3.org/2001/XMLSchema#decimal">104</SUTURO:perceptionId>
        <rdfs:comment>A hammer is a hand-held tool with a heavy metal head and a handle used for driving nails, breaking objects apart, or shaping metal.</rdfs:comment>
        <rdfs:isDefinedBy rdf:resource="http://www.ease-crc.org/ont/SUTURO.owl"/>
    </owl:Class>
    


    <!-- http://www.ease-crc.org/ont/SUTURO.owl#HansanoWeidemilchMilkPack -->

    <owl:Class rdf:about="http://www.ease-crc.org/ont/SUTURO.owl#HansanoWeidemilchMilkPack">
        <rdfs:subClassOf rdf:resource="http://www.ease-crc.org/ont/SOMA.owl#MilkPack"/>
        <rdfs:isDefinedBy rdf:resource="http://www.ease-crc.org/ont/SUTURO.owl"/>
    </owl:Class>
    


    <!-- http://www.ease-crc.org/ont/SUTURO.owl#Hat -->

    <owl:Class rdf:about="http://www.ease-crc.org/ont/SUTURO.owl#Hat">
        <rdfs:subClassOf rdf:resource="http://www.ease-crc.org/ont/SUTURO.owl#Clothing"/>
        <rdfs:subClassOf>
            <owl:Restriction>
                <owl:onProperty rdf:resource="http://www.ease-crc.org/ont/SUTURO.owl#hasPredefinedName"/>
                <owl:hasValue>hat</owl:hasValue>
            </owl:Restriction>
        </rdfs:subClassOf>
        <rdfs:isDefinedBy rdf:resource="http://www.ease-crc.org/ont/SUTURO.owl"/>
    </owl:Class>
    


    <!-- http://www.ease-crc.org/ont/SUTURO.owl#Hoodie -->

    <owl:Class rdf:about="http://www.ease-crc.org/ont/SUTURO.owl#Hoodie">
        <rdfs:subClassOf rdf:resource="http://www.ease-crc.org/ont/SUTURO.owl#Clothing"/>
        <rdfs:subClassOf>
            <owl:Restriction>
                <owl:onProperty rdf:resource="http://www.ease-crc.org/ont/SUTURO.owl#hasPredefinedName"/>
                <owl:hasValue>hoodie</owl:hasValue>
            </owl:Restriction>
        </rdfs:subClassOf>
        <rdfs:isDefinedBy rdf:resource="http://www.ease-crc.org/ont/SUTURO.owl"/>
    </owl:Class>
    


    <!-- http://www.ease-crc.org/ont/SUTURO.owl#HotChocolate -->

    <owl:Class rdf:about="http://www.ease-crc.org/ont/SUTURO.owl#HotChocolate">
        <rdfs:subClassOf rdf:resource="http://www.ease-crc.org/ont/SUTURO.owl#Drink"/>
        <rdfs:subClassOf>
            <owl:Restriction>
                <owl:onProperty rdf:resource="http://www.ease-crc.org/ont/SUTURO.owl#hasPredefinedName"/>
                <owl:hasValue>hot chocolate</owl:hasValue>
            </owl:Restriction>
        </rdfs:subClassOf>
        <rdfs:isDefinedBy rdf:resource="http://www.ease-crc.org/ont/SUTURO.owl"/>
    </owl:Class>
    


    <!-- http://www.ease-crc.org/ont/SUTURO.owl#HouseholdHardware -->

    <owl:Class rdf:about="http://www.ease-crc.org/ont/SUTURO.owl#HouseholdHardware">
        <rdfs:subClassOf rdf:resource="http://www.ease-crc.org/ont/SOMA.owl#DesignedTool"/>
        <rdfs:comment>Household hardware (or simply, hardware) is equipment that can be touched or held by hand such as keys, locks, nuts, screws, washers, hinges, latches, handles, wire, chains, belts, plumbing supplies, electrical supplies, tools, utensils, cutlery and machine parts.</rdfs:comment>
        <rdfs:isDefinedBy rdf:resource="http://www.ease-crc.org/ont/SUTURO.owl"/>
    </owl:Class>
    


    <!-- http://www.ease-crc.org/ont/SUTURO.owl#HygieneProduct -->

    <owl:Class rdf:about="http://www.ease-crc.org/ont/SUTURO.owl#HygieneProduct">
        <rdfs:subClassOf rdf:resource="http://www.ontologydesignpatterns.org/ont/dul/DUL.owl#DesignedSubstance"/>
        <rdfs:comment>Hygiene products are items that are used to promote cleanliness and personal hygiene. This can include products such as soap, shampoo, toothpaste, deodorant, and feminine hygiene products.</rdfs:comment>
        <rdfs:isDefinedBy rdf:resource="http://www.ease-crc.org/ont/SUTURO.owl"/>
    </owl:Class>
    


    <!-- http://www.ease-crc.org/ont/SUTURO.owl#IceTea -->

    <owl:Class rdf:about="http://www.ease-crc.org/ont/SUTURO.owl#IceTea">
        <rdfs:subClassOf rdf:resource="http://www.ease-crc.org/ont/SUTURO.owl#Drink"/>
        <rdfs:subClassOf rdf:resource="http://www.ease-crc.org/ont/SUTURO.owl#RoboCupDrinks"/>
        <rdfs:subClassOf rdf:resource="http://www.ease-crc.org/ont/SUTURO.owl#Tea"/>
        <rdfs:subClassOf>
            <owl:Restriction>
                <owl:onProperty rdf:resource="http://www.ease-crc.org/ont/SUTURO.owl#hasPredefinedName"/>
                <owl:hasValue>ice tea</owl:hasValue>
            </owl:Restriction>
        </rdfs:subClassOf>
        <rdfs:subClassOf>
            <owl:Restriction>
                <owl:onProperty rdf:resource="http://www.ease-crc.org/ont/SUTURO.owl#hasPredefinedName"/>
                <owl:hasValue>iced tea</owl:hasValue>
            </owl:Restriction>
        </rdfs:subClassOf>
        <rdfs:comment>Iced tea is a beverage made by steeping tea leaves in hot water, then chilling the tea and serving it over ice. It can be sweetened and flavored with lemon, peach, or other fruits, and is a popular refreshment, especially during hot weather.</rdfs:comment>
        <rdfs:isDefinedBy rdf:resource="http://www.ease-crc.org/ont/SUTURO.owl"/>
    </owl:Class>
    


    <!-- http://www.ease-crc.org/ont/SUTURO.owl#IceTeaBottle -->

    <owl:Class rdf:about="http://www.ease-crc.org/ont/SUTURO.owl#IceTeaBottle">
        <rdfs:subClassOf rdf:resource="http://www.ease-crc.org/ont/SOMA.owl#Bottle"/>
        <rdfs:subClassOf rdf:resource="http://www.ease-crc.org/ont/SUTURO.owl#IceTea"/>
        <rdfs:subClassOf rdf:resource="http://www.ease-crc.org/ont/SUTURO.owl#RoboCupDrinks"/>
        <rdfs:subClassOf>
            <owl:Restriction>
                <owl:onProperty rdf:resource="http://www.ease-crc.org/ont/SUTURO.owl#hasPredefinedName"/>
                <owl:hasValue>ice tea bottle</owl:hasValue>
            </owl:Restriction>
        </rdfs:subClassOf>
        <SUTURO:perceptionId rdf:datatype="http://www.w3.org/2001/XMLSchema#int">86</SUTURO:perceptionId>
        <rdfs:comment>An iced tea bottle is a container, commonly made of plastic or glass, designed specifically for storing and dispensing iced tea. It typically features a screw-top or snap cap for resealability, allowing the beverage to stay fresh and chilled, and is favored for its portability and convenience.</rdfs:comment>
        <rdfs:isDefinedBy rdf:resource="http://www.ease-crc.org/ont/SUTURO.owl"/>
    </owl:Class>
    


    <!-- http://www.ease-crc.org/ont/SUTURO.owl#IceTeaBox -->

    <owl:Class rdf:about="http://www.ease-crc.org/ont/SUTURO.owl#IceTeaBox">
        <rdfs:subClassOf rdf:resource="http://www.ease-crc.org/ont/SOMA.owl#Box"/>
        <rdfs:comment>An ice tea box refers to the container or packaging used to store and sell iced tea, usually in a ready-to-drink form. The box may contain individual servings or larger quantities, and can be made of various materials such as cardboard, plastic, or glass.</rdfs:comment>
        <rdfs:isDefinedBy rdf:resource="http://www.ease-crc.org/ont/SUTURO.owl"/>
    </owl:Class>
    


    <!-- http://www.ease-crc.org/ont/SUTURO.owl#IceTeaCan -->

    <owl:Class rdf:about="http://www.ease-crc.org/ont/SUTURO.owl#IceTeaCan">
        <rdfs:subClassOf rdf:resource="http://www.ease-crc.org/ont/SUTURO.owl#IceTea"/>
        <rdfs:subClassOf rdf:resource="http://www.ease-crc.org/ont/SUTURO.owl#RoboCupDrinks"/>
        <rdfs:subClassOf>
            <owl:Restriction>
                <owl:onProperty rdf:resource="http://www.ease-crc.org/ont/SUTURO.owl#hasPredefinedName"/>
                <owl:hasValue>ice tea</owl:hasValue>
            </owl:Restriction>
        </rdfs:subClassOf>
        <SUTURO:perceptionId rdf:datatype="http://www.w3.org/2001/XMLSchema#decimal">111</SUTURO:perceptionId>
        <rdfs:isDefinedBy rdf:resource="http://www.ease-crc.org/ont/SUTURO.owl"/>
    </owl:Class>
    


    <!-- http://www.ease-crc.org/ont/SUTURO.owl#IcedCoffee -->

    <owl:Class rdf:about="http://www.ease-crc.org/ont/SUTURO.owl#IcedCoffee">
        <rdfs:subClassOf rdf:resource="http://www.ease-crc.org/ont/SUTURO.owl#Coffee"/>
        <rdfs:subClassOf>
            <owl:Restriction>
                <owl:onProperty rdf:resource="http://www.ease-crc.org/ont/SUTURO.owl#hasPredefinedName"/>
                <owl:hasValue>iced coffee</owl:hasValue>
            </owl:Restriction>
        </rdfs:subClassOf>
        <rdfs:isDefinedBy rdf:resource="http://www.ease-crc.org/ont/SUTURO.owl"/>
    </owl:Class>
    


    <!-- http://www.ease-crc.org/ont/SUTURO.owl#JaFettarmeHMilchMilkPack -->

    <owl:Class rdf:about="http://www.ease-crc.org/ont/SUTURO.owl#JaFettarmeHMilchMilkPack">
        <rdfs:subClassOf rdf:resource="http://www.ease-crc.org/ont/SOMA.owl#MilkPack"/>
        <rdfs:isDefinedBy rdf:resource="http://www.ease-crc.org/ont/SUTURO.owl"/>
    </owl:Class>
    


    <!-- http://www.ease-crc.org/ont/SUTURO.owl#Jacket -->

    <owl:Class rdf:about="http://www.ease-crc.org/ont/SUTURO.owl#Jacket">
        <rdfs:subClassOf rdf:resource="http://www.ease-crc.org/ont/SUTURO.owl#Clothing"/>
        <rdfs:subClassOf>
            <owl:Restriction>
                <owl:onProperty rdf:resource="http://www.ease-crc.org/ont/SUTURO.owl#hasPredefinedName"/>
                <owl:hasValue>jacket</owl:hasValue>
            </owl:Restriction>
        </rdfs:subClassOf>
        <rdfs:isDefinedBy rdf:resource="http://www.ease-crc.org/ont/SUTURO.owl"/>
    </owl:Class>
    


    <!-- http://www.ease-crc.org/ont/SUTURO.owl#JellOChocolatePuddingBox -->

    <owl:Class rdf:about="http://www.ease-crc.org/ont/SUTURO.owl#JellOChocolatePuddingBox">
        <rdfs:subClassOf rdf:resource="http://www.ease-crc.org/ont/SUTURO.owl#PuddingBox"/>
        <rdfs:subClassOf rdf:resource="http://www.ease-crc.org/ont/SUTURO.owl#RoboCupFood"/>
        <rdfs:subClassOf>
            <owl:Restriction>
                <owl:onProperty rdf:resource="http://www.ease-crc.org/ont/SUTURO.owl#hasPredefinedName"/>
                <owl:hasValue>jello chocolate pudding box</owl:hasValue>
            </owl:Restriction>
        </rdfs:subClassOf>
        <SUTURO:perceptionId rdf:datatype="http://www.w3.org/2001/XMLSchema#int">19</SUTURO:perceptionId>
        <rdfs:comment>A box containing, or at least normally intended to contain, Jell-O brand chocolate flavored pudding powder.</rdfs:comment>
        <rdfs:isDefinedBy rdf:resource="http://www.ease-crc.org/ont/SUTURO.owl"/>
    </owl:Class>
    


    <!-- http://www.ease-crc.org/ont/SUTURO.owl#JellOStrawberryBox -->

    <owl:Class rdf:about="http://www.ease-crc.org/ont/SUTURO.owl#JellOStrawberryBox">
        <rdfs:subClassOf rdf:resource="http://www.ease-crc.org/ont/SUTURO.owl#JelloBox"/>
        <rdfs:subClassOf rdf:resource="http://www.ease-crc.org/ont/SUTURO.owl#RoboCupFood"/>
        <rdfs:subClassOf>
            <owl:Restriction>
                <owl:onProperty rdf:resource="http://www.ease-crc.org/ont/SUTURO.owl#hasPredefinedName"/>
                <owl:hasValue>jello strawberry box</owl:hasValue>
            </owl:Restriction>
        </rdfs:subClassOf>
        <rdfs:comment>A box containing, or at least normally intended to contain, Jell-O brand strawberry flavored gelatin.</rdfs:comment>
        <rdfs:isDefinedBy rdf:resource="http://www.ease-crc.org/ont/SUTURO.owl"/>
    </owl:Class>
    


    <!-- http://www.ease-crc.org/ont/SUTURO.owl#Jello -->

    <owl:Class rdf:about="http://www.ease-crc.org/ont/SUTURO.owl#Jello">
        <rdfs:subClassOf rdf:resource="http://www.ontologydesignpatterns.org/ont/dul/DUL.owl#DesignedSubstance"/>
        <rdfs:comment>Jello, also known as gelatin, is a sweet dessert made by combining gelatin powder with hot water, sugar, and flavorings, then cooling and setting the mixture in a mold. It is a popular treat for both children and adults, and comes in a variety of flavors and colors.</rdfs:comment>
        <rdfs:isDefinedBy rdf:resource="http://www.ease-crc.org/ont/SUTURO.owl"/>
    </owl:Class>
    


    <!-- http://www.ease-crc.org/ont/SUTURO.owl#JelloBox -->

    <owl:Class rdf:about="http://www.ease-crc.org/ont/SUTURO.owl#JelloBox">
        <rdfs:subClassOf rdf:resource="http://www.ease-crc.org/ont/SOMA.owl#Box"/>
        <rdfs:subClassOf>
            <owl:Restriction>
                <owl:onProperty rdf:resource="http://www.ease-crc.org/ont/SUTURO.owl#hasPredefinedName"/>
                <owl:hasValue>jello box</owl:hasValue>
            </owl:Restriction>
        </rdfs:subClassOf>
        <SUTURO:perceptionId rdf:datatype="http://www.w3.org/2001/XMLSchema#int">48</SUTURO:perceptionId>
        <rdfs:comment>A box containing, or at least normally intended to contain, jello.</rdfs:comment>
        <rdfs:isDefinedBy rdf:resource="http://www.ease-crc.org/ont/SUTURO.owl"/>
    </owl:Class>
    


    <!-- http://www.ease-crc.org/ont/SUTURO.owl#Jug -->

    <owl:Class rdf:about="http://www.ease-crc.org/ont/SUTURO.owl#Jug">
        <rdfs:subClassOf rdf:resource="http://www.ease-crc.org/ont/SOMA.owl#DesignedContainer"/>
        <rdfs:subClassOf>
            <owl:Restriction>
                <owl:onProperty rdf:resource="http://www.ease-crc.org/ont/SUTURO.owl#hasPredefinedName"/>
                <owl:hasValue>jug</owl:hasValue>
            </owl:Restriction>
        </rdfs:subClassOf>
        <rdfs:isDefinedBy rdf:resource="http://www.ease-crc.org/ont/SUTURO.owl"/>
    </owl:Class>
    


    <!-- http://www.ease-crc.org/ont/SUTURO.owl#Juice -->

    <owl:Class rdf:about="http://www.ease-crc.org/ont/SUTURO.owl#Juice">
        <rdfs:subClassOf rdf:resource="http://www.ease-crc.org/ont/SUTURO.owl#Drink"/>
        <rdfs:subClassOf>
            <owl:Restriction>
                <owl:onProperty rdf:resource="http://www.ease-crc.org/ont/SUTURO.owl#hasPredefinedName"/>
                <owl:hasValue>juice</owl:hasValue>
            </owl:Restriction>
        </rdfs:subClassOf>
        <rdfs:comment>Juice is a beverage made from the extraction or pressing of the natural liquid contained in fruits and vegetables. It can be consumed as a refreshing drink, and is often marketed as a source of vitamins and other nutrients.</rdfs:comment>
        <rdfs:isDefinedBy rdf:resource="http://www.ease-crc.org/ont/SUTURO.owl"/>
    </owl:Class>
    


    <!-- http://www.ease-crc.org/ont/SUTURO.owl#JuiceBottle -->

    <owl:Class rdf:about="http://www.ease-crc.org/ont/SUTURO.owl#JuiceBottle">
        <rdfs:subClassOf rdf:resource="http://www.ease-crc.org/ont/SOMA.owl#Bottle"/>
        <rdfs:subClassOf>
            <owl:Restriction>
                <owl:onProperty rdf:resource="http://www.ease-crc.org/ont/SUTURO.owl#hasPredefinedName"/>
                <owl:hasValue>juice bottle</owl:hasValue>
            </owl:Restriction>
        </rdfs:subClassOf>
        <rdfs:comment>A juice bottle is a container, typically made from plastic or glass, that&apos;s specifically designed for storing and dispensing juice. It often features a screw-top or snap cap to maintain freshness and ease of use, and its portability makes it a popular choice for consumption at home or on the go.</rdfs:comment>
        <rdfs:isDefinedBy rdf:resource="http://www.ease-crc.org/ont/SUTURO.owl"/>
    </owl:Class>
    


    <!-- http://www.ease-crc.org/ont/SUTURO.owl#JuiceBox -->

    <owl:Class rdf:about="http://www.ease-crc.org/ont/SUTURO.owl#JuiceBox">
        <rdfs:subClassOf rdf:resource="http://www.ease-crc.org/ont/SOMA.owl#Box"/>
        <rdfs:subClassOf>
            <owl:Restriction>
                <owl:onProperty rdf:resource="http://www.ease-crc.org/ont/SUTURO.owl#hasPredefinedName"/>
                <owl:hasValue>juice box</owl:hasValue>
            </owl:Restriction>
        </rdfs:subClassOf>
        <SUTURO:perceptionId rdf:datatype="http://www.w3.org/2001/XMLSchema#int">70</SUTURO:perceptionId>
        <rdfs:comment>A juice box is a container made of paperboard, with a small attached plastic straw, used for packaging and drinking juice. They are typically single-serving and convenient for on-the-go consumption.</rdfs:comment>
        <rdfs:isDefinedBy rdf:resource="http://www.ease-crc.org/ont/SUTURO.owl"/>
    </owl:Class>
    


    <!-- http://www.ease-crc.org/ont/SUTURO.owl#JuicePack -->

    <owl:Class rdf:about="http://www.ease-crc.org/ont/SUTURO.owl#JuicePack">
        <rdfs:subClassOf rdf:resource="http://www.ease-crc.org/ont/SOMA.owl#Pack"/>
        <rdfs:subClassOf rdf:resource="http://www.ease-crc.org/ont/SUTURO.owl#RoboCupDrinks"/>
        <rdfs:subClassOf>
            <owl:Restriction>
                <owl:onProperty rdf:resource="http://www.ease-crc.org/ont/SUTURO.owl#hasPredefinedName"/>
                <owl:hasValue>dubbelfris</owl:hasValue>
            </owl:Restriction>
        </rdfs:subClassOf>
        <rdfs:subClassOf>
            <owl:Restriction>
                <owl:onProperty rdf:resource="http://www.ease-crc.org/ont/SUTURO.owl#hasPredefinedName"/>
                <owl:hasValue>juice pack</owl:hasValue>
            </owl:Restriction>
        </rdfs:subClassOf>
        <SUTURO:perceptionId rdf:datatype="http://www.w3.org/2001/XMLSchema#int">82</SUTURO:perceptionId>
        <rdfs:comment>A juice pack is a portable container, often made of plastic or a combination of plastic, paper, and aluminum, designed to hold and dispense single servings of juice. It typically comes with a resealable cap or a pre-punched hole for a straw, providing a convenient option for on-the-go consumption and packed lunches.</rdfs:comment>
        <rdfs:isDefinedBy rdf:resource="http://www.ease-crc.org/ont/SUTURO.owl"/>
    </owl:Class>
    


    <!-- http://www.ease-crc.org/ont/SUTURO.owl#KelloggsCornFlakes -->

    <owl:Class rdf:about="http://www.ease-crc.org/ont/SUTURO.owl#KelloggsCornFlakes">
        <rdfs:subClassOf rdf:resource="http://www.ease-crc.org/ont/SUTURO.owl#Cereal"/>
        <rdfs:subClassOf>
            <owl:Restriction>
                <owl:onProperty rdf:resource="http://www.ease-crc.org/ont/SUTURO.owl#hasPredefinedName"/>
                <owl:hasValue>kelloggs corn flakes</owl:hasValue>
            </owl:Restriction>
        </rdfs:subClassOf>
        <rdfs:comment>Kellogg&apos;s Corn Flakes are a popular brand of breakfast cereal made from milled corn and malt flavoring. They were first created in the late 19th century by John Harvey Kellogg and his brother Will Keith Kellogg, and are known for their crunchy texture and mild, slightly sweet flavor.</rdfs:comment>
        <rdfs:isDefinedBy rdf:resource="http://www.ease-crc.org/ont/SUTURO.owl"/>
    </owl:Class>
    


    <!-- http://www.ease-crc.org/ont/SUTURO.owl#KelloggsCornFlakesBox -->

    <owl:Class rdf:about="http://www.ease-crc.org/ont/SUTURO.owl#KelloggsCornFlakesBox">
        <rdfs:subClassOf rdf:resource="http://www.ease-crc.org/ont/SOMA.owl#CerealBox"/>
        <rdfs:comment>A Kellogg&apos;s Corn Flakes box is a cardboard packaging that contains corn flakes, a popular breakfast cereal made from toasted corn.</rdfs:comment>
        <rdfs:isDefinedBy rdf:resource="http://www.ease-crc.org/ont/SUTURO.owl"/>
    </owl:Class>
    


    <!-- http://www.ease-crc.org/ont/SUTURO.owl#Ketchup -->

    <owl:Class rdf:about="http://www.ease-crc.org/ont/SUTURO.owl#Ketchup">
        <rdfs:subClassOf rdf:resource="http://www.ease-crc.org/ont/SUTURO.owl#Condiment"/>
        <rdfs:subClassOf>
            <owl:Restriction>
                <owl:onProperty rdf:resource="http://www.ease-crc.org/ont/SUTURO.owl#hasPredefinedName"/>
                <owl:hasValue>ketchup</owl:hasValue>
            </owl:Restriction>
        </rdfs:subClassOf>
        <rdfs:comment>Ketchup is a sweet and tangy condiment made from tomatoes, vinegar, sugar, and spices. It is commonly used as a topping for burgers, fries, and hot dogs, and is a popular ingredient in many sauces and dressings.</rdfs:comment>
        <rdfs:isDefinedBy rdf:resource="http://www.ease-crc.org/ont/SUTURO.owl"/>
    </owl:Class>
    


    <!-- http://www.ease-crc.org/ont/SUTURO.owl#KitchenTable -->

    <owl:Class rdf:about="http://www.ease-crc.org/ont/SUTURO.owl#KitchenTable">
        <rdfs:subClassOf rdf:resource="http://www.ease-crc.org/ont/SOMA.owl#Table"/>
        <rdfs:subClassOf>
            <owl:Restriction>
                <owl:onProperty rdf:resource="http://www.ease-crc.org/ont/SUTURO.owl#hasPredefinedName"/>
                <owl:hasValue>kitchen table</owl:hasValue>
            </owl:Restriction>
        </rdfs:subClassOf>
        <rdfs:comment>A table that is placed inside a kitchen and that is used for doing kitchen tasks like preparing meals.</rdfs:comment>
        <rdfs:isDefinedBy rdf:resource="http://www.ease-crc.org/ont/SUTURO.owl"/>
    </owl:Class>
    


    <!-- http://www.ease-crc.org/ont/SUTURO.owl#Kiwi -->

    <owl:Class rdf:about="http://www.ease-crc.org/ont/SUTURO.owl#Kiwi">
        <rdfs:subClassOf rdf:resource="http://www.ease-crc.org/ont/SUTURO.owl#Fruit"/>
        <rdfs:subClassOf rdf:resource="http://www.ease-crc.org/ont/SUTURO.owl#RoboCupFruits"/>
        <rdfs:subClassOf>
            <owl:Restriction>
                <owl:onProperty rdf:resource="http://www.ease-crc.org/ont/SUTURO.owl#hasPredefinedName"/>
                <owl:hasValue>kiwi</owl:hasValue>
            </owl:Restriction>
        </rdfs:subClassOf>
        <SUTURO:perceptionId rdf:datatype="http://www.w3.org/2001/XMLSchema#int">59</SUTURO:perceptionId>
        <rdfs:comment>Kiwi is a small, oval-shaped fruit with brown fuzzy skin and bright green flesh inside, packed with nutrients such as vitamin C, vitamin K, and potassium. It has a tangy, sweet flavor and is often eaten raw, added to salads or smoothies, or used as a garnish.</rdfs:comment>
        <rdfs:isDefinedBy rdf:resource="http://www.ease-crc.org/ont/SUTURO.owl"/>
    </owl:Class>
    


    <!-- http://www.ease-crc.org/ont/SUTURO.owl#KoellnKnusperSchokoKeksBox -->

    <owl:Class rdf:about="http://www.ease-crc.org/ont/SUTURO.owl#KoellnKnusperSchokoKeksBox">
        <rdfs:subClassOf rdf:resource="http://www.ease-crc.org/ont/SOMA.owl#CerealBox"/>
        <rdfs:comment>The Kölln Knusper Schoko &amp; Keks box contains crunchy chocolate and cookie flakes that can be enjoyed as a breakfast cereal or snack.</rdfs:comment>
        <rdfs:isDefinedBy rdf:resource="http://www.ease-crc.org/ont/SUTURO.owl"/>
    </owl:Class>
    


    <!-- http://www.ease-crc.org/ont/SUTURO.owl#LargeMarker -->

    <owl:Class rdf:about="http://www.ease-crc.org/ont/SUTURO.owl#LargeMarker">
        <rdfs:subClassOf rdf:resource="http://www.ease-crc.org/ont/SUTURO.owl#WritingTool"/>
        <rdfs:subClassOf>
            <owl:Restriction>
                <owl:onProperty rdf:resource="http://www.ease-crc.org/ont/SUTURO.owl#hasPredefinedName"/>
                <owl:hasValue>large marker</owl:hasValue>
            </owl:Restriction>
        </rdfs:subClassOf>
        <SUTURO:perceptionId rdf:datatype="http://www.w3.org/2001/XMLSchema#decimal">96</SUTURO:perceptionId>
        <rdfs:comment>A large marker is a pen-like writing tool with a wide, felt tip used for creating bold, colorful marks or lettering on posters, signs, or other large surfaces.</rdfs:comment>
        <rdfs:isDefinedBy rdf:resource="http://www.ease-crc.org/ont/SUTURO.owl"/>
    </owl:Class>
    


    <!-- http://www.ease-crc.org/ont/SUTURO.owl#Leggings -->

    <owl:Class rdf:about="http://www.ease-crc.org/ont/SUTURO.owl#Leggings">
        <rdfs:subClassOf rdf:resource="http://www.ease-crc.org/ont/SUTURO.owl#Clothing"/>
        <rdfs:subClassOf>
            <owl:Restriction>
                <owl:onProperty rdf:resource="http://www.ease-crc.org/ont/SUTURO.owl#hasPredefinedName"/>
                <owl:hasValue>leggings</owl:hasValue>
            </owl:Restriction>
        </rdfs:subClassOf>
        <rdfs:isDefinedBy rdf:resource="http://www.ease-crc.org/ont/SUTURO.owl"/>
    </owl:Class>
    


    <!-- http://www.ease-crc.org/ont/SUTURO.owl#Lego -->

    <owl:Class rdf:about="http://www.ease-crc.org/ont/SUTURO.owl#Lego">
        <rdfs:subClassOf rdf:resource="http://www.ease-crc.org/ont/SUTURO.owl#Toy"/>
        <rdfs:subClassOf>
            <owl:Restriction>
                <owl:onProperty rdf:resource="http://www.ease-crc.org/ont/SUTURO.owl#hasPredefinedName"/>
                <owl:hasValue>lego</owl:hasValue>
            </owl:Restriction>
        </rdfs:subClassOf>
        <rdfs:comment>LEGO is a popular construction toy consisting of colorful interlocking plastic bricks and other components that can be assembled and reconfigured into various shapes and structures.</rdfs:comment>
        <rdfs:isDefinedBy rdf:resource="http://www.ease-crc.org/ont/SUTURO.owl"/>
    </owl:Class>
    


    <!-- http://www.ease-crc.org/ont/SUTURO.owl#LegoDuplo -->

    <owl:Class rdf:about="http://www.ease-crc.org/ont/SUTURO.owl#LegoDuplo">
        <rdfs:subClassOf rdf:resource="http://www.ease-crc.org/ont/SUTURO.owl#Lego"/>
        <rdfs:subClassOf>
            <owl:Restriction>
                <owl:onProperty rdf:resource="http://www.ease-crc.org/ont/SUTURO.owl#hasPredefinedName"/>
                <owl:hasValue>lego duplo</owl:hasValue>
            </owl:Restriction>
        </rdfs:subClassOf>
        <rdfs:comment>Lego Duplo is a line of Lego building toys designed for children aged 1.5 to 5 years old.</rdfs:comment>
        <rdfs:isDefinedBy rdf:resource="http://www.ease-crc.org/ont/SUTURO.owl"/>
    </owl:Class>
    


    <!-- http://www.ease-crc.org/ont/SUTURO.owl#Lemon -->

    <owl:Class rdf:about="http://www.ease-crc.org/ont/SUTURO.owl#Lemon">
        <rdfs:subClassOf rdf:resource="http://www.ease-crc.org/ont/SUTURO.owl#Fruit"/>
        <rdfs:subClassOf rdf:resource="http://www.ease-crc.org/ont/SUTURO.owl#RoboCupFruits"/>
        <rdfs:subClassOf>
            <owl:Restriction>
                <owl:onProperty rdf:resource="http://www.ease-crc.org/ont/SUTURO.owl#hasPredefinedName"/>
                <owl:hasValue>lemon</owl:hasValue>
            </owl:Restriction>
        </rdfs:subClassOf>
        <SUTURO:perceptionId rdf:datatype="http://www.w3.org/2001/XMLSchema#int">76</SUTURO:perceptionId>
        <rdfs:comment>A lemon is a yellow citrus fruit with a sour taste, acidic juice, and versatile use in cooking and beverages.</rdfs:comment>
        <rdfs:isDefinedBy rdf:resource="http://www.ease-crc.org/ont/SUTURO.owl"/>
    </owl:Class>
    


    <!-- http://www.ease-crc.org/ont/SUTURO.owl#Lemonade -->

    <owl:Class rdf:about="http://www.ease-crc.org/ont/SUTURO.owl#Lemonade">
        <rdfs:subClassOf rdf:resource="http://www.ease-crc.org/ont/SUTURO.owl#Drink"/>
        <rdfs:subClassOf>
            <owl:Restriction>
                <owl:onProperty rdf:resource="http://www.ease-crc.org/ont/SUTURO.owl#hasPredefinedName"/>
                <owl:hasValue>lemonade</owl:hasValue>
            </owl:Restriction>
        </rdfs:subClassOf>
        <rdfs:isDefinedBy rdf:resource="http://www.ease-crc.org/ont/SUTURO.owl"/>
    </owl:Class>
    


    <!-- http://www.ease-crc.org/ont/SUTURO.owl#Liquid -->

    <owl:Class rdf:about="http://www.ease-crc.org/ont/SUTURO.owl#Liquid">
        <rdfs:subClassOf rdf:resource="http://www.ease-crc.org/ont/SOMA.owl#Fluid"/>
        <rdfs:subClassOf rdf:resource="http://www.ease-crc.org/ont/SUTURO.owl#Food"/>
        <rdfs:subClassOf>
            <owl:Restriction>
                <owl:onProperty rdf:resource="http://www.ease-crc.org/ont/SOMA.owl#hasDisposition"/>
                <owl:allValuesFrom rdf:resource="http://www.ease-crc.org/ont/SUTURO.owl#Perishable"/>
            </owl:Restriction>
        </rdfs:subClassOf>
        <rdfs:subClassOf>
            <owl:Restriction>
                <owl:onProperty rdf:resource="http://www.ease-crc.org/ont/SUTURO.owl#hasPredefinedName"/>
                <owl:hasValue>liquid</owl:hasValue>
            </owl:Restriction>
        </rdfs:subClassOf>
        <rdfs:comment>Liquid food is a type of food that is in a liquid state and can be consumed without chewing.</rdfs:comment>
        <rdfs:isDefinedBy rdf:resource="http://www.ease-crc.org/ont/SUTURO.owl"/>
    </owl:Class>
    


    <!-- http://www.ease-crc.org/ont/SUTURO.owl#Liquorice -->

    <owl:Class rdf:about="http://www.ease-crc.org/ont/SUTURO.owl#Liquorice">
        <rdfs:subClassOf rdf:resource="http://www.ease-crc.org/ont/SUTURO.owl#RoboCupSnacks"/>
        <rdfs:subClassOf rdf:resource="http://www.ease-crc.org/ont/SUTURO.owl#Sweets"/>
        <rdfs:subClassOf>
            <owl:Restriction>
                <owl:onProperty rdf:resource="http://www.ease-crc.org/ont/SUTURO.owl#hasPredefinedName"/>
                <owl:hasValue>liquorice</owl:hasValue>
            </owl:Restriction>
        </rdfs:subClassOf>
        <SUTURO:perceptionId rdf:datatype="http://www.w3.org/2001/XMLSchema#decimal">125</SUTURO:perceptionId>
        <rdfs:isDefinedBy rdf:resource="http://www.ease-crc.org/ont/SUTURO.owl"/>
    </owl:Class>
    


    <!-- http://www.ease-crc.org/ont/SUTURO.owl#LivingRoom -->

    <owl:Class rdf:about="http://www.ease-crc.org/ont/SUTURO.owl#LivingRoom">
        <rdfs:subClassOf rdf:resource="http://www.ease-crc.org/ont/SOMA.owl#Room"/>
        <rdfs:subClassOf>
            <owl:Restriction>
                <owl:onProperty rdf:resource="http://www.ease-crc.org/ont/SUTURO.owl#hasPredefinedName"/>
                <owl:hasValue>living room</owl:hasValue>
            </owl:Restriction>
        </rdfs:subClassOf>
        <rdfs:comment>A living room is a common area in a home designed for socializing, entertainment, and relaxation. It usually features comfortable seating, such as sofas and chairs, and may include a television, coffee table, and other furniture for gathering and conversation.</rdfs:comment>
        <rdfs:isDefinedBy rdf:resource="http://www.ease-crc.org/ont/SUTURO.owl"/>
    </owl:Class>
    


    <!-- http://www.ease-crc.org/ont/SUTURO.owl#Lobby -->

    <owl:Class rdf:about="http://www.ease-crc.org/ont/SUTURO.owl#Lobby">
        <rdfs:subClassOf rdf:resource="http://www.ease-crc.org/ont/SOMA.owl#Room"/>
        <rdfs:subClassOf>
            <owl:Restriction>
                <owl:onProperty rdf:resource="http://www.ease-crc.org/ont/SUTURO.owl#hasPredefinedName"/>
                <owl:hasValue>lobby</owl:hasValue>
            </owl:Restriction>
        </rdfs:subClassOf>
        <rdfs:isDefinedBy rdf:resource="http://www.ease-crc.org/ont/SUTURO.owl"/>
    </owl:Class>
    


    <!-- http://www.ease-crc.org/ont/SUTURO.owl#LowFatLongLastingMilk -->

    <owl:Class rdf:about="http://www.ease-crc.org/ont/SUTURO.owl#LowFatLongLastingMilk">
        <rdfs:subClassOf rdf:resource="http://www.ease-crc.org/ont/SUTURO.owl#Milk"/>
        <rdfs:subClassOf>
            <owl:Restriction>
                <owl:onProperty rdf:resource="http://www.ease-crc.org/ont/SUTURO.owl#hasPredefinedName"/>
                <owl:hasValue>low fat long lasting milk</owl:hasValue>
            </owl:Restriction>
        </rdfs:subClassOf>
        <rdfs:comment>Low-fat long-lasting milk is a type of milk that has been processed to remove some of the fat and extend its shelf life. This milk is typically heated to a high temperature, which kills off bacteria and enzymes that can cause spoilage, and then packaged in airtight containers.</rdfs:comment>
        <rdfs:isDefinedBy rdf:resource="http://www.ease-crc.org/ont/SUTURO.owl"/>
    </owl:Class>
    


    <!-- http://www.ease-crc.org/ont/SUTURO.owl#Magazine -->

    <owl:Class rdf:about="http://www.ease-crc.org/ont/SUTURO.owl#Magazine">
        <rdfs:subClassOf rdf:resource="http://www.ease-crc.org/ont/SUTURO.owl#PrintedMatter"/>
        <rdfs:comment>A magazine is a publication containing articles and illustrations, often on a particular subject or aimed at a particular audience.</rdfs:comment>
        <rdfs:isDefinedBy rdf:resource="http://www.ease-crc.org/ont/SUTURO.owl"/>
    </owl:Class>
    


    <!-- http://www.ease-crc.org/ont/SUTURO.owl#Marble -->

    <owl:Class rdf:about="http://www.ease-crc.org/ont/SUTURO.owl#Marble">
        <rdfs:subClassOf rdf:resource="http://www.ease-crc.org/ont/SUTURO.owl#Ball"/>
        <rdfs:subClassOf>
            <owl:Restriction>
                <owl:onProperty rdf:resource="http://www.ease-crc.org/ont/SUTURO.owl#hasPredefinedName"/>
                <owl:hasValue>marble</owl:hasValue>
            </owl:Restriction>
        </rdfs:subClassOf>
        <SUTURO:perceptionId rdf:datatype="http://www.w3.org/2001/XMLSchema#int">41</SUTURO:perceptionId>
        <rdfs:comment>A marble is a small, spherical toy made of glass, stone, or other materials, used in games, competitions, or for decoration.</rdfs:comment>
        <rdfs:isDefinedBy rdf:resource="http://www.ease-crc.org/ont/SUTURO.owl"/>
    </owl:Class>
    


    <!-- http://www.ease-crc.org/ont/SUTURO.owl#MasterchefCan -->

    <owl:Class rdf:about="http://www.ease-crc.org/ont/SUTURO.owl#MasterchefCan">
        <rdfs:subClassOf rdf:resource="http://www.ease-crc.org/ont/SUTURO.owl#Can"/>
        <SUTURO:perceptionId rdf:datatype="http://www.w3.org/2001/XMLSchema#decimal">97</SUTURO:perceptionId>
        <rdfs:isDefinedBy rdf:resource="http://www.ease-crc.org/ont/SUTURO.owl"/>
    </owl:Class>
    


    <!-- http://www.ease-crc.org/ont/SUTURO.owl#Mayonaise -->

    <owl:Class rdf:about="http://www.ease-crc.org/ont/SUTURO.owl#Mayonaise">
        <rdfs:subClassOf rdf:resource="http://www.ease-crc.org/ont/SUTURO.owl#Condiment"/>
        <rdfs:subClassOf rdf:resource="http://www.ease-crc.org/ont/SUTURO.owl#RoboCupFood"/>
        <rdfs:subClassOf>
            <owl:Restriction>
                <owl:onProperty rdf:resource="http://www.ease-crc.org/ont/SUTURO.owl#hasPredefinedName"/>
                <owl:hasValue>mayonaise</owl:hasValue>
            </owl:Restriction>
        </rdfs:subClassOf>
        <SUTURO:perceptionId rdf:datatype="http://www.w3.org/2001/XMLSchema#decimal">118</SUTURO:perceptionId>
        <rdfs:isDefinedBy rdf:resource="http://www.ease-crc.org/ont/SUTURO.owl"/>
    </owl:Class>
    


    <!-- http://www.ease-crc.org/ont/SUTURO.owl#Meat -->

    <owl:Class rdf:about="http://www.ease-crc.org/ont/SUTURO.owl#Meat">
        <rdfs:subClassOf rdf:resource="http://www.ease-crc.org/ont/SUTURO.owl#Food"/>
        <rdfs:subClassOf>
            <owl:Restriction>
                <owl:onProperty rdf:resource="http://www.ease-crc.org/ont/SUTURO.owl#hasPredefinedName"/>
                <owl:hasValue>meat</owl:hasValue>
            </owl:Restriction>
        </rdfs:subClassOf>
        <rdfs:isDefinedBy rdf:resource="http://www.ease-crc.org/ont/SUTURO.owl"/>
    </owl:Class>
    


    <!-- http://www.ease-crc.org/ont/SUTURO.owl#MetalBowl -->

    <owl:Class rdf:about="http://www.ease-crc.org/ont/SUTURO.owl#MetalBowl">
        <rdfs:subClassOf rdf:resource="http://www.ease-crc.org/ont/SOMA.owl#Bowl"/>
        <rdfs:subClassOf>
            <owl:Restriction>
                <owl:onProperty rdf:resource="http://www.ease-crc.org/ont/SUTURO.owl#hasPredefinedName"/>
                <owl:hasValue>metal bowl</owl:hasValue>
            </owl:Restriction>
        </rdfs:subClassOf>
        <SUTURO:perceptionId rdf:datatype="http://www.w3.org/2001/XMLSchema#int">56</SUTURO:perceptionId>
        <rdfs:comment>A metal bowl is a container made from metal material, typically stainless steel or aluminum, and used for various purposes such as mixing ingredients, serving food, or as a decorative object. It is durable, easy to clean, and can withstand high temperatures, making it ideal for use in the kitchen.</rdfs:comment>
        <rdfs:isDefinedBy rdf:resource="http://www.ease-crc.org/ont/SUTURO.owl"/>
    </owl:Class>
    


    <!-- http://www.ease-crc.org/ont/SUTURO.owl#MetalCup -->

    <owl:Class rdf:about="http://www.ease-crc.org/ont/SUTURO.owl#MetalCup">
        <rdfs:subClassOf rdf:resource="http://www.ease-crc.org/ont/SOMA.owl#Cup"/>
        <rdfs:subClassOf>
            <owl:Restriction>
                <owl:onProperty rdf:resource="http://www.ease-crc.org/ont/SUTURO.owl#hasPredefinedName"/>
                <owl:hasValue>metal cup</owl:hasValue>
            </owl:Restriction>
        </rdfs:subClassOf>
        <rdfs:isDefinedBy rdf:resource="http://www.ease-crc.org/ont/SUTURO.owl"/>
    </owl:Class>
    


    <!-- http://www.ease-crc.org/ont/SUTURO.owl#MetalHardware -->

    <owl:Class rdf:about="http://www.ease-crc.org/ont/SUTURO.owl#MetalHardware">
        <rdfs:subClassOf rdf:resource="http://www.ease-crc.org/ont/SOMA.owl#DesignedTool"/>
        <rdfs:comment>Metal hardware refers to various metal components, such as nuts, bolts, screws, washers, and hinges, used in manufacturing and construction to join or secure different objects or materials together.</rdfs:comment>
        <rdfs:isDefinedBy rdf:resource="http://www.ease-crc.org/ont/SUTURO.owl"/>
    </owl:Class>
    


    <!-- http://www.ease-crc.org/ont/SUTURO.owl#MetalKnife -->

    <owl:Class rdf:about="http://www.ease-crc.org/ont/SUTURO.owl#MetalKnife">
        <rdfs:subClassOf rdf:resource="http://www.ease-crc.org/ont/SOMA.owl#Knife"/>
        <rdfs:subClassOf>
            <owl:Restriction>
                <owl:onProperty rdf:resource="http://www.ease-crc.org/ont/SUTURO.owl#hasPredefinedName"/>
                <owl:hasValue>metal knife</owl:hasValue>
            </owl:Restriction>
        </rdfs:subClassOf>
        <rdfs:isDefinedBy rdf:resource="http://www.ease-crc.org/ont/SUTURO.owl"/>
    </owl:Class>
    


    <!-- http://www.ease-crc.org/ont/SUTURO.owl#MetalMug -->

    <owl:Class rdf:about="http://www.ease-crc.org/ont/SUTURO.owl#MetalMug">
        <rdfs:subClassOf rdf:resource="http://www.ease-crc.org/ont/SUTURO.owl#Mug"/>
        <rdfs:subClassOf>
            <owl:Restriction>
                <owl:onProperty rdf:resource="http://www.ease-crc.org/ont/SUTURO.owl#hasPredefinedName"/>
                <owl:hasValue>metal mug</owl:hasValue>
            </owl:Restriction>
        </rdfs:subClassOf>
        <SUTURO:perceptionId rdf:datatype="http://www.w3.org/2001/XMLSchema#int">43</SUTURO:perceptionId>
        <rdfs:comment>A metal mug is a drinking vessel made from metal material, typically stainless steel or copper, and designed to hold hot or cold beverages. It is sturdy, reusable, and often used for camping, outdoor activities, or as a travel mug.</rdfs:comment>
        <rdfs:isDefinedBy rdf:resource="http://www.ease-crc.org/ont/SUTURO.owl"/>
    </owl:Class>
    


    <!-- http://www.ease-crc.org/ont/SUTURO.owl#MetalPlate -->

    <owl:Class rdf:about="http://www.ease-crc.org/ont/SUTURO.owl#MetalPlate">
        <rdfs:subClassOf rdf:resource="http://www.ease-crc.org/ont/SOMA.owl#Plate"/>
        <SUTURO:perceptionId rdf:datatype="http://www.w3.org/2001/XMLSchema#decimal">35</SUTURO:perceptionId>
        <rdfs:isDefinedBy rdf:resource="http://www.ease-crc.org/ont/SUTURO.owl"/>
    </owl:Class>
    


    <!-- http://www.ease-crc.org/ont/SUTURO.owl#Microwave -->

    <owl:Class rdf:about="http://www.ease-crc.org/ont/SUTURO.owl#Microwave">
        <rdfs:subClassOf rdf:resource="http://www.ease-crc.org/ont/SOMA.owl#Appliance"/>
        <rdfs:subClassOf rdf:resource="http://www.ease-crc.org/ont/SOMA.owl#DesignedContainer"/>
        <rdfs:subClassOf>
            <owl:Restriction>
                <owl:onProperty rdf:resource="http://www.ease-crc.org/ont/SUTURO.owl#hasPredefinedName"/>
                <owl:hasValue>microwave</owl:hasValue>
            </owl:Restriction>
        </rdfs:subClassOf>
        <rdfs:comment>A microwave is an appliance that cooks or heats up food by using microwave radiation to excite the molecules in the food.</rdfs:comment>
        <rdfs:isDefinedBy rdf:resource="http://www.ease-crc.org/ont/SUTURO.owl"/>
    </owl:Class>
    


    <!-- http://www.ease-crc.org/ont/SUTURO.owl#Milk -->

    <owl:Class rdf:about="http://www.ease-crc.org/ont/SUTURO.owl#Milk">
        <rdfs:subClassOf rdf:resource="http://www.ease-crc.org/ont/SUTURO.owl#Drink"/>
        <rdfs:subClassOf rdf:resource="http://www.ease-crc.org/ont/SUTURO.owl#RoboCupDrinks"/>
        <rdfs:subClassOf>
            <owl:Restriction>
                <owl:onProperty rdf:resource="http://www.ease-crc.org/ont/SUTURO.owl#hasOriginLocation"/>
                <owl:allValuesFrom rdf:resource="http://www.ease-crc.org/ont/SOMA.owl#Refrigerator"/>
            </owl:Restriction>
        </rdfs:subClassOf>
        <rdfs:subClassOf>
            <owl:Restriction>
                <owl:onProperty rdf:resource="http://www.ease-crc.org/ont/SUTURO.owl#hasPredefinedName"/>
                <owl:hasValue>milk</owl:hasValue>
            </owl:Restriction>
        </rdfs:subClassOf>
        <rdfs:comment>Milk is a nutrient-rich liquid that comes from cows or other mammals and is commonly consumed by humans.</rdfs:comment>
        <rdfs:isDefinedBy rdf:resource="http://www.ease-crc.org/ont/SUTURO.owl"/>
    </owl:Class>
    


    <!-- http://www.ease-crc.org/ont/SUTURO.owl#MilkCoffee -->

    <owl:Class rdf:about="http://www.ease-crc.org/ont/SUTURO.owl#MilkCoffee">
        <rdfs:subClassOf rdf:resource="http://www.ease-crc.org/ont/SUTURO.owl#Coffee"/>
        <rdfs:subClassOf>
            <owl:Restriction>
                <owl:onProperty rdf:resource="http://www.ease-crc.org/ont/SUTURO.owl#hasPredefinedName"/>
                <owl:hasValue>milk coffee</owl:hasValue>
            </owl:Restriction>
        </rdfs:subClassOf>
        <rdfs:isDefinedBy rdf:resource="http://www.ease-crc.org/ont/SUTURO.owl"/>
    </owl:Class>
    


    <!-- http://www.ease-crc.org/ont/SUTURO.owl#MilkGlass -->

    <owl:Class rdf:about="http://www.ease-crc.org/ont/SUTURO.owl#MilkGlass">
        <rdfs:subClassOf rdf:resource="http://www.ease-crc.org/ont/SOMA.owl#Glass"/>
        <rdfs:subClassOf>
            <owl:Restriction>
                <owl:onProperty rdf:resource="http://www.ease-crc.org/ont/SUTURO.owl#hasPredefinedName"/>
                <owl:hasValue>milk glass</owl:hasValue>
            </owl:Restriction>
        </rdfs:subClassOf>
        <rdfs:comment>A glass which holds, or at least is intended to usually hold, water. Also affords drinking from it.</rdfs:comment>
        <rdfs:isDefinedBy rdf:resource="http://www.ease-crc.org/ont/SUTURO.owl"/>
    </owl:Class>
    


    <!-- http://www.ease-crc.org/ont/SUTURO.owl#MilkJug -->

    <owl:Class rdf:about="http://www.ease-crc.org/ont/SUTURO.owl#MilkJug">
        <rdfs:subClassOf rdf:resource="http://www.ease-crc.org/ont/SUTURO.owl#Jug"/>
        <rdfs:subClassOf>
            <owl:Restriction>
                <owl:onProperty rdf:resource="http://www.ease-crc.org/ont/SUTURO.owl#hasPredefinedName"/>
                <owl:hasValue>milk jug</owl:hasValue>
            </owl:Restriction>
        </rdfs:subClassOf>
        <rdfs:isDefinedBy rdf:resource="http://www.ease-crc.org/ont/SUTURO.owl"/>
    </owl:Class>
    


    <!-- http://www.ease-crc.org/ont/SUTURO.owl#MilkPackJa -->

    <owl:Class rdf:about="http://www.ease-crc.org/ont/SUTURO.owl#MilkPackJa">
        <rdfs:subClassOf rdf:resource="http://www.ease-crc.org/ont/SOMA.owl#MilkPack"/>
        <SUTURO:perceptionId rdf:datatype="http://www.w3.org/2001/XMLSchema#decimal">91</SUTURO:perceptionId>
        <rdfs:isDefinedBy rdf:resource="http://www.ease-crc.org/ont/SOMA-HOME.owl"/>
    </owl:Class>
    


    <!-- http://www.ease-crc.org/ont/SUTURO.owl#Mineral -->

    <owl:Class rdf:about="http://www.ease-crc.org/ont/SUTURO.owl#Mineral">
        <rdfs:subClassOf rdf:resource="http://www.ontologydesignpatterns.org/ont/dul/DUL.owl#Substance"/>
        <rdfs:comment>A mineral is a naturally occurring inorganic substance that has a specific chemical composition and a crystalline structure. They are found in rocks and the Earth&apos;s crust and have many practical uses, such as being used as building materials, in electronics, and in the production of jewelry.</rdfs:comment>
        <rdfs:isDefinedBy rdf:resource="http://www.ease-crc.org/ont/SUTURO.owl"/>
    </owl:Class>
    


    <!-- http://www.ease-crc.org/ont/SUTURO.owl#MineralWater -->

    <owl:Class rdf:about="http://www.ease-crc.org/ont/SUTURO.owl#MineralWater">
        <rdfs:subClassOf rdf:resource="http://www.ease-crc.org/ont/SUTURO.owl#Drink"/>
        <rdfs:subClassOf>
            <owl:Restriction>
                <owl:onProperty rdf:resource="http://www.ease-crc.org/ont/SUTURO.owl#hasPredefinedName"/>
                <owl:hasValue>mineral water</owl:hasValue>
            </owl:Restriction>
        </rdfs:subClassOf>
        <rdfs:isDefinedBy rdf:resource="http://www.ease-crc.org/ont/SUTURO.owl"/>
    </owl:Class>
    


    <!-- http://www.ease-crc.org/ont/SUTURO.owl#MiniSoccerBall -->

    <owl:Class rdf:about="http://www.ease-crc.org/ont/SUTURO.owl#MiniSoccerBall">
        <rdfs:subClassOf rdf:resource="http://www.ease-crc.org/ont/SUTURO.owl#Ball"/>
        <rdfs:subClassOf rdf:resource="http://www.ease-crc.org/ont/SUTURO.owl#RoboCupToys"/>
        <rdfs:subClassOf>
            <owl:Restriction>
                <owl:onProperty rdf:resource="http://www.ease-crc.org/ont/SUTURO.owl#hasPredefinedName"/>
                <owl:hasValue>mini soccer ball</owl:hasValue>
            </owl:Restriction>
        </rdfs:subClassOf>
        <SUTURO:perceptionId rdf:datatype="http://www.w3.org/2001/XMLSchema#int">11</SUTURO:perceptionId>
        <rdfs:comment>A mini soccer ball is a smaller version of a regulation soccer ball, often used for training, indoor or recreational play, or for promotional or decorative purposes.</rdfs:comment>
        <rdfs:isDefinedBy rdf:resource="http://www.ease-crc.org/ont/SUTURO.owl"/>
    </owl:Class>
    


    <!-- http://www.ease-crc.org/ont/SUTURO.owl#Muesli -->

    <owl:Class rdf:about="http://www.ease-crc.org/ont/SUTURO.owl#Muesli">
        <rdfs:subClassOf rdf:resource="http://www.ease-crc.org/ont/SUTURO.owl#ProcessedFood"/>
        <rdfs:subClassOf>
            <owl:Restriction>
                <owl:onProperty rdf:resource="http://www.ease-crc.org/ont/SUTURO.owl#hasPredefinedName"/>
                <owl:hasValue>muesli</owl:hasValue>
            </owl:Restriction>
        </rdfs:subClassOf>
        <rdfs:isDefinedBy rdf:resource="http://www.ease-crc.org/ont/SUTURO.owl"/>
    </owl:Class>
    


    <!-- http://www.ease-crc.org/ont/SUTURO.owl#MuesliBox -->

    <owl:Class rdf:about="http://www.ease-crc.org/ont/SUTURO.owl#MuesliBox">
        <rdfs:subClassOf rdf:resource="http://www.ease-crc.org/ont/SOMA.owl#Box"/>
        <rdfs:subClassOf>
            <owl:Restriction>
                <owl:onProperty rdf:resource="http://www.ease-crc.org/ont/SUTURO.owl#hasPredefinedName"/>
                <owl:hasValue>mueslibox</owl:hasValue>
            </owl:Restriction>
        </rdfs:subClassOf>
        <SUTURO:perceptionId rdf:datatype="http://www.w3.org/2001/XMLSchema#decimal">92</SUTURO:perceptionId>
        <rdfs:isDefinedBy rdf:resource="http://www.ease-crc.org/ont/SUTURO.owl"/>
    </owl:Class>
    


    <!-- http://www.ease-crc.org/ont/SUTURO.owl#Mug -->

    <owl:Class rdf:about="http://www.ease-crc.org/ont/SUTURO.owl#Mug">
        <rdfs:subClassOf rdf:resource="http://www.ease-crc.org/ont/SOMA.owl#Cup"/>
        <rdfs:subClassOf>
            <owl:Restriction>
                <owl:onProperty rdf:resource="http://www.ease-crc.org/ont/SUTURO.owl#hasPredefinedName"/>
                <owl:hasValue>mug</owl:hasValue>
            </owl:Restriction>
        </rdfs:subClassOf>
        <rdfs:comment>A mug is a cylindrical-shaped cup, usually made of ceramic, porcelain, or glass, with a handle for holding and drinking hot beverages such as coffee or tea.</rdfs:comment>
        <rdfs:isDefinedBy rdf:resource="http://www.ease-crc.org/ont/SUTURO.owl"/>
    </owl:Class>
    


    <!-- http://www.ease-crc.org/ont/SUTURO.owl#MulledWineTea -->

    <owl:Class rdf:about="http://www.ease-crc.org/ont/SUTURO.owl#MulledWineTea">
        <rdfs:subClassOf rdf:resource="http://www.ease-crc.org/ont/SUTURO.owl#Tea"/>
        <rdfs:subClassOf>
            <owl:Restriction>
                <owl:onProperty rdf:resource="http://www.ease-crc.org/ont/SUTURO.owl#hasPredefinedName"/>
                <owl:hasValue>mulled wine tea</owl:hasValue>
            </owl:Restriction>
        </rdfs:subClassOf>
        <rdfs:comment>Mulled wine tea is a type of tea that is typically made with a blend of black tea, spices, and dried fruit, such as orange peel or cinnamon. It is often served as a warm, comforting beverage during the winter months and is known for its rich, aromatic flavor and spicy notes.</rdfs:comment>
        <rdfs:isDefinedBy rdf:resource="http://www.ease-crc.org/ont/SUTURO.owl"/>
    </owl:Class>
    


    <!-- http://www.ease-crc.org/ont/SUTURO.owl#Mustard -->

    <owl:Class rdf:about="http://www.ease-crc.org/ont/SUTURO.owl#Mustard">
        <rdfs:subClassOf rdf:resource="http://www.ease-crc.org/ont/SUTURO.owl#Condiment"/>
        <rdfs:subClassOf>
            <owl:Restriction>
                <owl:onProperty rdf:resource="http://www.ease-crc.org/ont/SUTURO.owl#hasPredefinedName"/>
                <owl:hasValue>mustard</owl:hasValue>
            </owl:Restriction>
        </rdfs:subClassOf>
        <rdfs:comment>Mustard is a condiment made from the seeds of the mustard plant, which are ground into a powder and mixed with vinegar or other liquids to create a paste or sauce. It is commonly used as a flavoring for sandwiches, dressings, marinades, and many other dishes.</rdfs:comment>
        <rdfs:isDefinedBy rdf:resource="http://www.ease-crc.org/ont/SUTURO.owl"/>
    </owl:Class>
    


    <!-- http://www.ease-crc.org/ont/SUTURO.owl#MustardBottle -->

    <owl:Class rdf:about="http://www.ease-crc.org/ont/SUTURO.owl#MustardBottle">
        <rdfs:subClassOf rdf:resource="http://www.ease-crc.org/ont/SOMA.owl#Bottle"/>
        <rdfs:subClassOf rdf:resource="http://www.ease-crc.org/ont/SUTURO.owl#RoboCupFood"/>
        <rdfs:subClassOf>
            <owl:Restriction>
                <owl:onProperty rdf:resource="http://www.ease-crc.org/ont/SUTURO.owl#hasPredefinedName"/>
                <owl:hasValue>mustard bottle</owl:hasValue>
            </owl:Restriction>
        </rdfs:subClassOf>
        <SUTURO:perceptionId rdf:datatype="http://www.w3.org/2001/XMLSchema#int">18</SUTURO:perceptionId>
        <rdfs:comment>Mustard bottle refers to a squeezable container that dispenses mustard.</rdfs:comment>
        <rdfs:isDefinedBy rdf:resource="http://www.ease-crc.org/ont/SUTURO.owl"/>
    </owl:Class>
    


    <!-- http://www.ease-crc.org/ont/SUTURO.owl#Nail -->

    <owl:Class rdf:about="http://www.ease-crc.org/ont/SUTURO.owl#Nail">
        <rdfs:subClassOf rdf:resource="http://www.ease-crc.org/ont/SUTURO.owl#Fastener"/>
        <rdfs:subClassOf rdf:resource="http://www.ease-crc.org/ont/SUTURO.owl#MetalHardware"/>
        <rdfs:subClassOf>
            <owl:Restriction>
                <owl:onProperty rdf:resource="http://www.ease-crc.org/ont/SUTURO.owl#hasPredefinedName"/>
                <owl:hasValue>nail</owl:hasValue>
            </owl:Restriction>
        </rdfs:subClassOf>
        <rdfs:comment>A nail is a thin, pointed metal or wood fastener with a flat head used for attaching or joining two objects together, or for securing an object to a surface.</rdfs:comment>
        <rdfs:isDefinedBy rdf:resource="http://www.ease-crc.org/ont/SUTURO.owl"/>
    </owl:Class>
    


    <!-- http://www.ease-crc.org/ont/SUTURO.owl#Napkin -->

    <owl:Class rdf:about="http://www.ease-crc.org/ont/SUTURO.owl#Napkin">
        <rdfs:subClassOf rdf:resource="http://www.ease-crc.org/ont/SUTURO.owl#DesignedFabric"/>
        <rdfs:subClassOf>
            <owl:Restriction>
                <owl:onProperty rdf:resource="http://www.ease-crc.org/ont/SUTURO.owl#hasPredefinedName"/>
                <owl:hasValue>napkin</owl:hasValue>
            </owl:Restriction>
        </rdfs:subClassOf>
        <SUTURO:perceptionId rdf:datatype="http://www.w3.org/2001/XMLSchema#int">17</SUTURO:perceptionId>
        <rdfs:comment>A square piece of cloth or paper used at a meal to wipe the fingers or lips and to protect garments</rdfs:comment>
        <rdfs:isDefinedBy rdf:resource="http://www.ease-crc.org/ont/SUTURO.owl"/>
    </owl:Class>
    


    <!-- http://www.ease-crc.org/ont/SUTURO.owl#NesquickCerealBox -->

    <owl:Class rdf:about="http://www.ease-crc.org/ont/SUTURO.owl#NesquickCerealBox">
        <rdfs:subClassOf rdf:resource="http://www.ease-crc.org/ont/SOMA.owl#CerealBox"/>
        <rdfs:subClassOf>
            <owl:Restriction>
                <owl:onProperty rdf:resource="http://www.ease-crc.org/ont/SUTURO.owl#hasPredefinedName"/>
                <owl:hasValue>nesquick cereal box</owl:hasValue>
            </owl:Restriction>
        </rdfs:subClassOf>
        <SUTURO:perceptionId rdf:datatype="http://www.w3.org/2001/XMLSchema#decimal">90</SUTURO:perceptionId>
        <rdfs:isDefinedBy rdf:resource="http://www.ease-crc.org/ont/SUTURO.owl"/>
    </owl:Class>
    


    <!-- http://www.ease-crc.org/ont/SUTURO.owl#NinePegHoleTest -->

    <owl:Class rdf:about="http://www.ease-crc.org/ont/SUTURO.owl#NinePegHoleTest">
        <rdfs:subClassOf rdf:resource="http://www.ease-crc.org/ont/SUTURO.owl#Toy"/>
        <rdfs:subClassOf>
            <owl:Restriction>
                <owl:onProperty rdf:resource="http://www.ease-crc.org/ont/SUTURO.owl#hasPredefinedName"/>
                <owl:hasValue>nine peg hole test</owl:hasValue>
            </owl:Restriction>
        </rdfs:subClassOf>
        <rdfs:comment>A pegboard with nine holes used for cognitive and psychomotor testing.</rdfs:comment>
        <rdfs:isDefinedBy rdf:resource="http://www.ease-crc.org/ont/SUTURO.owl"/>
    </owl:Class>
    


    <!-- http://www.ease-crc.org/ont/SUTURO.owl#Nut -->

    <owl:Class rdf:about="http://www.ease-crc.org/ont/SUTURO.owl#Nut">
        <rdfs:subClassOf rdf:resource="http://www.ease-crc.org/ont/SUTURO.owl#Fastener"/>
        <rdfs:subClassOf rdf:resource="http://www.ease-crc.org/ont/SUTURO.owl#MetalHardware"/>
        <rdfs:subClassOf>
            <owl:Restriction>
                <owl:onProperty rdf:resource="http://www.ease-crc.org/ont/SUTURO.owl#hasPredefinedName"/>
                <owl:hasValue>nut</owl:hasValue>
            </owl:Restriction>
        </rdfs:subClassOf>
        <rdfs:comment>A nut is a small, usually hexagonal-shaped metal or plastic fastener with a threaded hole used for securing a bolt or screw in place.</rdfs:comment>
        <rdfs:isDefinedBy rdf:resource="http://www.ease-crc.org/ont/SUTURO.owl"/>
    </owl:Class>
    


    <!-- http://www.ease-crc.org/ont/SUTURO.owl#Office -->

    <owl:Class rdf:about="http://www.ease-crc.org/ont/SUTURO.owl#Office">
        <rdfs:subClassOf rdf:resource="http://www.ease-crc.org/ont/SOMA.owl#Room"/>
        <rdfs:subClassOf>
            <owl:Restriction>
                <owl:onProperty rdf:resource="http://www.ease-crc.org/ont/SUTURO.owl#hasPredefinedName"/>
                <owl:hasValue>office</owl:hasValue>
            </owl:Restriction>
        </rdfs:subClassOf>
        <rdfs:isDefinedBy rdf:resource="http://www.ease-crc.org/ont/SUTURO.owl"/>
    </owl:Class>
    


    <!-- http://www.ease-crc.org/ont/SUTURO.owl#Orange -->

    <owl:Class rdf:about="http://www.ease-crc.org/ont/SUTURO.owl#Orange">
        <rdfs:subClassOf rdf:resource="http://www.ease-crc.org/ont/SUTURO.owl#Fruit"/>
        <rdfs:subClassOf rdf:resource="http://www.ease-crc.org/ont/SUTURO.owl#RoboCupFruits"/>
        <rdfs:subClassOf>
            <owl:Restriction>
                <owl:onProperty rdf:resource="http://www.ease-crc.org/ont/SUTURO.owl#hasPredefinedName"/>
                <owl:hasValue>orange</owl:hasValue>
            </owl:Restriction>
        </rdfs:subClassOf>
        <SUTURO:perceptionId rdf:datatype="http://www.w3.org/2001/XMLSchema#int">27</SUTURO:perceptionId>
        <rdfs:comment>An orange is a round citrus fruit with a tough, bright orange skin, pulpy flesh with sections, and a juicy, tangy flavor.</rdfs:comment>
        <rdfs:isDefinedBy rdf:resource="http://www.ease-crc.org/ont/SUTURO.owl"/>
    </owl:Class>
    


    <!-- http://www.ease-crc.org/ont/SUTURO.owl#OrangeJuice -->

    <owl:Class rdf:about="http://www.ease-crc.org/ont/SUTURO.owl#OrangeJuice">
        <rdfs:subClassOf rdf:resource="http://www.ease-crc.org/ont/SUTURO.owl#Juice"/>
        <rdfs:subClassOf>
            <owl:Restriction>
                <owl:onProperty rdf:resource="http://www.ease-crc.org/ont/SUTURO.owl#hasPredefinedName"/>
                <owl:hasValue>orange juice</owl:hasValue>
            </owl:Restriction>
        </rdfs:subClassOf>
    </owl:Class>
    


    <!-- http://www.ease-crc.org/ont/SUTURO.owl#OrangeJuiceBox -->

    <owl:Class rdf:about="http://www.ease-crc.org/ont/SUTURO.owl#OrangeJuiceBox">
        <rdfs:subClassOf rdf:resource="http://www.ease-crc.org/ont/SUTURO.owl#JuiceBox"/>
        <rdfs:subClassOf rdf:resource="http://www.ease-crc.org/ont/SUTURO.owl#RoboCupDrinks"/>
        <rdfs:subClassOf>
            <owl:Restriction>
                <owl:onProperty rdf:resource="http://www.ease-crc.org/ont/SUTURO.owl#hasPredefinedName"/>
                <owl:hasValue>orange juice box</owl:hasValue>
            </owl:Restriction>
        </rdfs:subClassOf>
        <SUTURO:perceptionId rdf:datatype="http://www.w3.org/2001/XMLSchema#int">87</SUTURO:perceptionId>
        <rdfs:comment>An OrangeJuiceBox is a portable, typically single-serving container made of paperboard or other lightweight materials, designed to hold and dispense orange juice. It is commonly equipped with a straw or a pull-tab for easy consumption, and is popular for its convenience and use in packed lunches or on-the-go situations.</rdfs:comment>
        <rdfs:isDefinedBy rdf:resource="http://www.ease-crc.org/ont/SUTURO.owl"/>
    </owl:Class>
    


    <!-- http://www.ease-crc.org/ont/SUTURO.owl#Oregano -->

    <owl:Class rdf:about="http://www.ease-crc.org/ont/SUTURO.owl#Oregano">
        <rdfs:subClassOf rdf:resource="http://www.ease-crc.org/ont/SUTURO.owl#Spice"/>
        <rdfs:subClassOf>
            <owl:Restriction>
                <owl:onProperty rdf:resource="http://www.ease-crc.org/ont/SUTURO.owl#hasPredefinedName"/>
                <owl:hasValue>oregano</owl:hasValue>
            </owl:Restriction>
        </rdfs:subClassOf>
        <rdfs:comment>Oregano is a fragrant herb commonly used in Mediterranean and Mexican cuisine. It has a strong, slightly bitter flavor and is often used dried to add depth to tomato-based sauces, meats, and vegetables.</rdfs:comment>
        <rdfs:isDefinedBy rdf:resource="http://www.ease-crc.org/ont/SUTURO.owl"/>
    </owl:Class>
    


    <!-- http://www.ease-crc.org/ont/SUTURO.owl#OreganoShaker -->

    <owl:Class rdf:about="http://www.ease-crc.org/ont/SUTURO.owl#OreganoShaker">
        <rdfs:subClassOf rdf:resource="http://www.ease-crc.org/ont/SOMA.owl#Shaker"/>
        <rdfs:subClassOf>
            <owl:Restriction>
                <owl:onProperty rdf:resource="http://www.ease-crc.org/ont/SUTURO.owl#hasPredefinedName"/>
                <owl:hasValue>oregano shaker</owl:hasValue>
            </owl:Restriction>
        </rdfs:subClassOf>
        <SUTURO:perceptionId rdf:datatype="http://www.w3.org/2001/XMLSchema#int">65</SUTURO:perceptionId>
        <rdfs:comment>An oregano shaker is a container used for storing and dispensing dried oregano spice, which is commonly used in cooking to add flavor and aroma to dishes. The shaker typically has small holes or slots on the top to allow for controlled dispensing of the oregano flakes.</rdfs:comment>
        <rdfs:isDefinedBy rdf:resource="http://www.ease-crc.org/ont/SUTURO.owl"/>
    </owl:Class>
    


    <!-- http://www.ease-crc.org/ont/SUTURO.owl#Package -->

    <owl:Class rdf:about="http://www.ease-crc.org/ont/SUTURO.owl#Package">
        <rdfs:subClassOf rdf:resource="http://www.ease-crc.org/ont/SOMA.owl#DesignedContainer"/>
        <rdfs:comment>A package is a wrapped or boxed object that contains one or more items for transport or storage. Packages can range in size from small envelopes to large boxes or crates.</rdfs:comment>
        <rdfs:isDefinedBy rdf:resource="http://www.ease-crc.org/ont/SUTURO.owl"/>
    </owl:Class>
    


    <!-- http://www.ease-crc.org/ont/SUTURO.owl#PadlockAndKeys -->

    <owl:Class rdf:about="http://www.ease-crc.org/ont/SUTURO.owl#PadlockAndKeys">
        <rdfs:subClassOf rdf:resource="http://www.ease-crc.org/ont/SUTURO.owl#HouseholdHardware"/>
        <rdfs:subClassOf>
            <owl:Restriction>
                <owl:onProperty rdf:resource="http://www.ease-crc.org/ont/SUTURO.owl#hasPredefinedName"/>
                <owl:hasValue>padlock and keys</owl:hasValue>
            </owl:Restriction>
        </rdfs:subClassOf>
        <rdfs:comment>A padlock and keys are a security device used for locking and securing doors, gates, or other objects, consisting of a metal lock with a U-shaped bar and a set of keys to open and close it.</rdfs:comment>
        <rdfs:isDefinedBy rdf:resource="http://www.ease-crc.org/ont/SUTURO.owl"/>
    </owl:Class>
    


    <!-- http://www.ease-crc.org/ont/SUTURO.owl#PancakeMix -->

    <owl:Class rdf:about="http://www.ease-crc.org/ont/SUTURO.owl#PancakeMix">
        <rdfs:subClassOf rdf:resource="http://www.ease-crc.org/ont/SUTURO.owl#ProcessedFood"/>
        <rdfs:subClassOf rdf:resource="http://www.ease-crc.org/ont/SUTURO.owl#RoboCupFood"/>
        <rdfs:subClassOf>
            <owl:Restriction>
                <owl:onProperty rdf:resource="http://www.ease-crc.org/ont/SUTURO.owl#hasPredefinedName"/>
                <owl:hasValue>pancake mix</owl:hasValue>
            </owl:Restriction>
        </rdfs:subClassOf>
        <SUTURO:perceptionId rdf:datatype="http://www.w3.org/2001/XMLSchema#decimal">121</SUTURO:perceptionId>
        <rdfs:isDefinedBy rdf:resource="http://www.ease-crc.org/ont/SUTURO.owl"/>
    </owl:Class>
    


    <!-- http://www.ease-crc.org/ont/SUTURO.owl#PancakeMixBottle -->

    <owl:Class rdf:about="http://www.ease-crc.org/ont/SUTURO.owl#PancakeMixBottle">
        <rdfs:subClassOf rdf:resource="http://www.ease-crc.org/ont/SOMA.owl#Bottle"/>
        <rdfs:subClassOf>
            <owl:Restriction>
                <owl:onProperty rdf:resource="http://www.ease-crc.org/ont/SUTURO.owl#hasPredefinedName"/>
                <owl:hasValue>pancake mix bottle</owl:hasValue>
            </owl:Restriction>
        </rdfs:subClassOf>
        <SUTURO:perceptionId rdf:datatype="http://www.w3.org/2001/XMLSchema#int">71</SUTURO:perceptionId>
        <rdfs:comment>A pancake mix bottle is a container that holds pre-made pancake batter, ready to be cooked. These bottles usually come with a nozzle for easy pouring and can be found in different sizes and shapes.</rdfs:comment>
        <rdfs:isDefinedBy rdf:resource="http://www.ease-crc.org/ont/SUTURO.owl"/>
    </owl:Class>
    


    <!-- http://www.ease-crc.org/ont/SUTURO.owl#Pantry -->

    <owl:Class rdf:about="http://www.ease-crc.org/ont/SUTURO.owl#Pantry">
        <rdfs:subClassOf rdf:resource="http://www.ease-crc.org/ont/SOMA.owl#Room"/>
        <rdfs:subClassOf>
            <owl:Restriction>
                <owl:onProperty rdf:resource="http://www.ease-crc.org/ont/SUTURO.owl#hasPredefinedName"/>
                <owl:hasValue>pantry</owl:hasValue>
            </owl:Restriction>
        </rdfs:subClassOf>
        <rdfs:isDefinedBy rdf:resource="http://www.ease-crc.org/ont/SUTURO.owl"/>
    </owl:Class>
    


    <!-- http://www.ease-crc.org/ont/SUTURO.owl#Pants -->

    <owl:Class rdf:about="http://www.ease-crc.org/ont/SUTURO.owl#Pants">
        <rdfs:subClassOf rdf:resource="http://www.ease-crc.org/ont/SUTURO.owl#Clothing"/>
        <rdfs:subClassOf>
            <owl:Restriction>
                <owl:onProperty rdf:resource="http://www.ease-crc.org/ont/SUTURO.owl#hasPredefinedName"/>
                <owl:hasValue>pants</owl:hasValue>
            </owl:Restriction>
        </rdfs:subClassOf>
        <rdfs:isDefinedBy rdf:resource="http://www.ease-crc.org/ont/SUTURO.owl"/>
    </owl:Class>
    


    <!-- http://www.ease-crc.org/ont/SUTURO.owl#PaperBag -->

    <owl:Class rdf:about="http://www.ease-crc.org/ont/SUTURO.owl#PaperBag">
        <rdfs:subClassOf rdf:resource="http://www.ease-crc.org/ont/SUTURO.owl#Bag"/>
        <rdfs:subClassOf>
            <owl:Restriction>
                <owl:onProperty rdf:resource="http://www.ease-crc.org/ont/SUTURO.owl#hasPredefinedName"/>
                <owl:hasValue>paper bag</owl:hasValue>
            </owl:Restriction>
        </rdfs:subClassOf>
        <rdfs:comment>A paper bag is a type of bag made from paper materials, such as kraft paper or recycled paper. It is commonly used for carrying groceries, snacks, and other lightweight items, and is often considered a more environmentally-friendly option compared to plastic bags. Paper bags can be recycled and are biodegradable, making them a sustainable choice for packaging and transporting goods.</rdfs:comment>
        <rdfs:isDefinedBy rdf:resource="http://www.ease-crc.org/ont/SUTURO.owl"/>
    </owl:Class>
    


    <!-- http://www.ease-crc.org/ont/SUTURO.owl#PastryBox -->

    <owl:Class rdf:about="http://www.ease-crc.org/ont/SUTURO.owl#PastryBox">
        <rdfs:subClassOf rdf:resource="http://www.ease-crc.org/ont/SOMA.owl#Box"/>
        <rdfs:subClassOf>
            <owl:Restriction>
                <owl:onProperty rdf:resource="http://www.ease-crc.org/ont/SUTURO.owl#hasPredefinedName"/>
                <owl:hasValue>pastry box</owl:hasValue>
            </owl:Restriction>
        </rdfs:subClassOf>
        <SUTURO:perceptionId rdf:datatype="http://www.w3.org/2001/XMLSchema#int">74</SUTURO:perceptionId>
        <rdfs:comment>A pastry box is a container used to transport and store pastries such as cakes, pies, and tarts. It is typically made of cardboard or plastic and designed to keep the pastries fresh and protected during transport, with features such as secure lids and inserts to prevent movement and damage.</rdfs:comment>
        <rdfs:isDefinedBy rdf:resource="http://www.ease-crc.org/ont/SUTURO.owl"/>
    </owl:Class>
    


    <!-- http://www.ease-crc.org/ont/SUTURO.owl#PeaSoupCan -->

    <owl:Class rdf:about="http://www.ease-crc.org/ont/SUTURO.owl#PeaSoupCan">
        <rdfs:subClassOf rdf:resource="http://www.ease-crc.org/ont/SUTURO.owl#RoboCupFood"/>
        <rdfs:subClassOf rdf:resource="http://www.ease-crc.org/ont/SUTURO.owl#SoupCan"/>
        <rdfs:subClassOf>
            <owl:Restriction>
                <owl:onProperty rdf:resource="http://www.ease-crc.org/ont/SUTURO.owl#hasPredefinedName"/>
                <owl:hasValue>pea soup</owl:hasValue>
            </owl:Restriction>
        </rdfs:subClassOf>
        <SUTURO:perceptionId rdf:datatype="http://www.w3.org/2001/XMLSchema#decimal">115</SUTURO:perceptionId>
        <rdfs:isDefinedBy rdf:resource="http://www.ease-crc.org/ont/SUTURO.owl"/>
    </owl:Class>
    


    <!-- http://www.ease-crc.org/ont/SUTURO.owl#Peach -->

    <owl:Class rdf:about="http://www.ease-crc.org/ont/SUTURO.owl#Peach">
        <rdfs:subClassOf rdf:resource="http://www.ease-crc.org/ont/SUTURO.owl#Fruit"/>
        <rdfs:subClassOf rdf:resource="http://www.ease-crc.org/ont/SUTURO.owl#RoboCupFruits"/>
        <rdfs:subClassOf>
            <owl:Restriction>
                <owl:onProperty rdf:resource="http://www.ease-crc.org/ont/SUTURO.owl#hasPredefinedName"/>
                <owl:hasValue>peach</owl:hasValue>
            </owl:Restriction>
        </rdfs:subClassOf>
        <SUTURO:perceptionId rdf:datatype="http://www.w3.org/2001/XMLSchema#decimal">79</SUTURO:perceptionId>
        <rdfs:comment>A peach is a round fruit with a fuzzy skin, juicy flesh, a large pit in the center, and a sweet, delicate flavor.</rdfs:comment>
        <rdfs:isDefinedBy rdf:resource="http://www.ease-crc.org/ont/SUTURO.owl"/>
    </owl:Class>
    


    <!-- http://www.ease-crc.org/ont/SUTURO.owl#PeachIceTeaBox -->

    <owl:Class rdf:about="http://www.ease-crc.org/ont/SUTURO.owl#PeachIceTeaBox">
        <rdfs:subClassOf rdf:resource="http://www.ease-crc.org/ont/SUTURO.owl#IceTeaBox"/>
        <rdfs:subClassOf>
            <owl:Restriction>
                <owl:onProperty rdf:resource="http://www.ease-crc.org/ont/SUTURO.owl#hasPredefinedName"/>
                <owl:hasValue>peach ice tea box</owl:hasValue>
            </owl:Restriction>
        </rdfs:subClassOf>
        <rdfs:comment>Peach ice tea box refers to the container or packaging used to store and sell peach-flavored iced tea, usually in a ready-to-drink form. The box may contain individual servings or larger quantities, and can be made of various materials such as cardboard, plastic, or glass.</rdfs:comment>
        <rdfs:isDefinedBy rdf:resource="http://www.ease-crc.org/ont/SUTURO.owl"/>
    </owl:Class>
    


    <!-- http://www.ease-crc.org/ont/SUTURO.owl#Pear -->

    <owl:Class rdf:about="http://www.ease-crc.org/ont/SUTURO.owl#Pear">
        <rdfs:subClassOf rdf:resource="http://www.ease-crc.org/ont/SUTURO.owl#Fruit"/>
        <rdfs:subClassOf rdf:resource="http://www.ease-crc.org/ont/SUTURO.owl#RoboCupFruits"/>
        <rdfs:subClassOf>
            <owl:Restriction>
                <owl:onProperty rdf:resource="http://www.ease-crc.org/ont/SUTURO.owl#hasPredefinedName"/>
                <owl:hasValue>pear</owl:hasValue>
            </owl:Restriction>
        </rdfs:subClassOf>
        <SUTURO:perceptionId rdf:datatype="http://www.w3.org/2001/XMLSchema#int">75</SUTURO:perceptionId>
        <rdfs:comment>A pear is a sweet, juicy fruit with a bulbous shape, a thin skin, and a core with seeds in the center.</rdfs:comment>
        <rdfs:isDefinedBy rdf:resource="http://www.ease-crc.org/ont/SUTURO.owl"/>
    </owl:Class>
    


    <!-- http://www.ease-crc.org/ont/SUTURO.owl#Perishable -->

    <owl:Class rdf:about="http://www.ease-crc.org/ont/SUTURO.owl#Perishable">
        <rdfs:subClassOf rdf:resource="http://www.ease-crc.org/ont/SOMA.owl#Disposition"/>
    </owl:Class>
    


    <!-- http://www.ease-crc.org/ont/SUTURO.owl#PhillipsScrewdriver -->

    <owl:Class rdf:about="http://www.ease-crc.org/ont/SUTURO.owl#PhillipsScrewdriver">
        <rdfs:subClassOf rdf:resource="http://www.ease-crc.org/ont/SUTURO.owl#ScrewDriver"/>
        <rdfs:comment>A Phillips screwdriver is a hand-held tool with a cross-shaped tip used for driving screws with a corresponding cross-shaped indentation in their head.</rdfs:comment>
        <rdfs:isDefinedBy rdf:resource="http://www.ease-crc.org/ont/SUTURO.owl"/>
    </owl:Class>
    


    <!-- http://www.ease-crc.org/ont/SUTURO.owl#PicklesJar -->

    <owl:Class rdf:about="http://www.ease-crc.org/ont/SUTURO.owl#PicklesJar">
        <rdfs:subClassOf rdf:resource="http://www.ease-crc.org/ont/SOMA.owl#Jar"/>
        <rdfs:subClassOf>
            <owl:Restriction>
                <owl:onProperty rdf:resource="http://www.ease-crc.org/ont/SUTURO.owl#hasPredefinedName"/>
                <owl:hasValue>pickles jar</owl:hasValue>
            </owl:Restriction>
        </rdfs:subClassOf>
        <rdfs:isDefinedBy rdf:resource="http://www.ease-crc.org/ont/SUTURO.owl"/>
    </owl:Class>
    


    <!-- http://www.ease-crc.org/ont/SUTURO.owl#PillBox -->

    <owl:Class rdf:about="http://www.ease-crc.org/ont/SUTURO.owl#PillBox">
        <rdfs:subClassOf rdf:resource="http://www.ease-crc.org/ont/SOMA.owl#Box"/>
        <rdfs:subClassOf>
            <owl:Restriction>
                <owl:onProperty rdf:resource="http://www.ease-crc.org/ont/SUTURO.owl#hasPredefinedName"/>
                <owl:hasValue>pill box</owl:hasValue>
            </owl:Restriction>
        </rdfs:subClassOf>
        <rdfs:isDefinedBy rdf:resource="http://www.ease-crc.org/ont/SUTURO.owl"/>
    </owl:Class>
    


    <!-- http://www.ease-crc.org/ont/SUTURO.owl#Pitcher -->

    <owl:Class rdf:about="http://www.ease-crc.org/ont/SUTURO.owl#Pitcher">
        <rdfs:subClassOf rdf:resource="http://www.ease-crc.org/ont/SOMA.owl#DesignedContainer"/>
        <rdfs:subClassOf>
            <owl:Restriction>
                <owl:onProperty rdf:resource="http://www.ease-crc.org/ont/SUTURO.owl#hasPredefinedName"/>
                <owl:hasValue>pitcher</owl:hasValue>
            </owl:Restriction>
        </rdfs:subClassOf>
        <SUTURO:perceptionId rdf:datatype="http://www.w3.org/2001/XMLSchema#int">7</SUTURO:perceptionId>
        <rdfs:comment>A pitcher is a container, usually made of glass or ceramic, with a handle and spout used for holding and pouring beverages such as water, juice, or tea.</rdfs:comment>
        <rdfs:isDefinedBy rdf:resource="http://www.ease-crc.org/ont/SUTURO.owl"/>
    </owl:Class>
    


    <!-- http://www.ease-crc.org/ont/SUTURO.owl#PitcherLid -->

    <owl:Class rdf:about="http://www.ease-crc.org/ont/SUTURO.owl#PitcherLid">
        <rdfs:subClassOf rdf:resource="http://www.ease-crc.org/ont/SOMA.owl#Lid"/>
        <rdfs:comment>A pitcher lid is a cover used to close the opening of a pitcher and prevent the contents from spilling or becoming contaminated.</rdfs:comment>
        <rdfs:isDefinedBy rdf:resource="http://www.ease-crc.org/ont/SUTURO.owl"/>
    </owl:Class>
    


    <!-- http://www.ease-crc.org/ont/SUTURO.owl#PlasticChain -->

    <owl:Class rdf:about="http://www.ease-crc.org/ont/SUTURO.owl#PlasticChain">
        <rdfs:subClassOf rdf:resource="http://www.ease-crc.org/ont/SUTURO.owl#Chain"/>
        <rdfs:subClassOf>
            <owl:Restriction>
                <owl:onProperty rdf:resource="http://www.ease-crc.org/ont/SUTURO.owl#hasPredefinedName"/>
                <owl:hasValue>plastic chain</owl:hasValue>
            </owl:Restriction>
        </rdfs:subClassOf>
        <SUTURO:perceptionId rdf:datatype="http://www.w3.org/2001/XMLSchema#int">51</SUTURO:perceptionId>
        <rdfs:comment>Plastic chain is a chain made from plastic links that are interconnected to form a continuous chain. It is often used as a visual barrier or for crowd control in public places, as well as for decorative purposes in events, exhibitions, and retail displays.</rdfs:comment>
        <rdfs:isDefinedBy rdf:resource="http://www.ease-crc.org/ont/SUTURO.owl"/>
    </owl:Class>
    


    <!-- http://www.ease-crc.org/ont/SUTURO.owl#PlasticKnife -->

    <owl:Class rdf:about="http://www.ease-crc.org/ont/SUTURO.owl#PlasticKnife">
        <rdfs:subClassOf rdf:resource="http://www.ease-crc.org/ont/SOMA.owl#Knife"/>
        <rdfs:subClassOf>
            <owl:Restriction>
                <owl:onProperty rdf:resource="http://www.ease-crc.org/ont/SUTURO.owl#hasPredefinedName"/>
                <owl:hasValue>plastic knife</owl:hasValue>
            </owl:Restriction>
        </rdfs:subClassOf>
        <SUTURO:perceptionId rdf:datatype="http://www.w3.org/2001/XMLSchema#int">1</SUTURO:perceptionId>
        <rdfs:comment>A plastic knife is a cutting tool made from plastic material, typically polypropylene or polystyrene, and is lightweight and disposable. It is commonly used for cutting soft foods such as cake or fruit, or as a safer alternative to metal knives in environments where metal utensils are not allowed.</rdfs:comment>
        <rdfs:isDefinedBy rdf:resource="http://www.ease-crc.org/ont/SUTURO.owl"/>
    </owl:Class>
    


    <!-- http://www.ease-crc.org/ont/SUTURO.owl#Plum -->

    <owl:Class rdf:about="http://www.ease-crc.org/ont/SUTURO.owl#Plum">
        <rdfs:subClassOf rdf:resource="http://www.ease-crc.org/ont/SUTURO.owl#Fruit"/>
        <rdfs:subClassOf rdf:resource="http://www.ease-crc.org/ont/SUTURO.owl#RoboCupFruits"/>
        <rdfs:subClassOf>
            <owl:Restriction>
                <owl:onProperty rdf:resource="http://www.ease-crc.org/ont/SUTURO.owl#hasPredefinedName"/>
                <owl:hasValue>plum</owl:hasValue>
            </owl:Restriction>
        </rdfs:subClassOf>
        <SUTURO:perceptionId rdf:datatype="http://www.w3.org/2001/XMLSchema#int">80</SUTURO:perceptionId>
        <rdfs:comment>A plum is a small, round or oval-shaped fruit with a smooth, edible skin, juicy, sweet or tart flesh, and a small pit in the center.</rdfs:comment>
        <rdfs:isDefinedBy rdf:resource="http://www.ease-crc.org/ont/SUTURO.owl"/>
    </owl:Class>
    


    <!-- http://www.ease-crc.org/ont/SUTURO.owl#PottedMeatCan -->

    <owl:Class rdf:about="http://www.ease-crc.org/ont/SUTURO.owl#PottedMeatCan">
        <rdfs:subClassOf rdf:resource="http://www.ease-crc.org/ont/SUTURO.owl#Can"/>
        <rdfs:subClassOf rdf:resource="http://www.ease-crc.org/ont/SUTURO.owl#RoboCupFood"/>
        <rdfs:subClassOf>
            <owl:Restriction>
                <owl:onProperty rdf:resource="http://www.ease-crc.org/ont/SUTURO.owl#hasPredefinedName"/>
                <owl:hasValue>potted meat can</owl:hasValue>
            </owl:Restriction>
        </rdfs:subClassOf>
        <SUTURO:perceptionId rdf:datatype="http://www.w3.org/2001/XMLSchema#decimal">78</SUTURO:perceptionId>
        <rdfs:comment>A can containing, or at least normally intended to contain, potted meat</rdfs:comment>
        <rdfs:isDefinedBy rdf:resource="http://www.ease-crc.org/ont/SUTURO.owl"/>
    </owl:Class>
    


    <!-- http://www.ease-crc.org/ont/SUTURO.owl#PowerDrill -->

    <owl:Class rdf:about="http://www.ease-crc.org/ont/SUTURO.owl#PowerDrill">
        <rdfs:subClassOf rdf:resource="http://www.ease-crc.org/ont/SUTURO.owl#ForceConcentratingTool"/>
        <rdfs:comment>A power drill is a motorized tool used for making holes in a variety of materials, or for driving screws or bolts into them, often used in woodworking, metalworking, or construction projects.</rdfs:comment>
        <rdfs:isDefinedBy rdf:resource="http://www.ease-crc.org/ont/SUTURO.owl"/>
    </owl:Class>
    


    <!-- http://www.ease-crc.org/ont/SUTURO.owl#PredefinedCategory -->

    <owl:Class rdf:about="http://www.ease-crc.org/ont/SUTURO.owl#PredefinedCategory">
        <rdfs:subClassOf rdf:resource="http://www.ontologydesignpatterns.org/ont/dul/DUL.owl#Collection"/>
        <rdfs:comment>A predefined category refers to a predetermined classification or grouping system that is established in advance. It allows for the organization and categorization of various elements, such as objects, concepts, or data, based on predefined criteria or characteristics.

In the context of the RoboCup, objects are usually categorized into predefined categories, that might not align with the structure of the exisiting ontologie. To handle this information, objects can be assigned a predefined category.</rdfs:comment>
        <rdfs:isDefinedBy rdf:resource="http://www.ease-crc.org/ont/SUTURO.owl"/>
    </owl:Class>
    


    <!-- http://www.ease-crc.org/ont/SUTURO.owl#Pringles -->

    <owl:Class rdf:about="http://www.ease-crc.org/ont/SUTURO.owl#Pringles">
        <rdfs:subClassOf rdf:resource="http://www.ease-crc.org/ont/SUTURO.owl#ProcessedFood"/>
        <rdfs:isDefinedBy rdf:resource="http://www.ease-crc.org/ont/SUTURO.owl"/>
    </owl:Class>
    


    <!-- http://www.ease-crc.org/ont/SUTURO.owl#PringlesChipsCan -->

    <owl:Class rdf:about="http://www.ease-crc.org/ont/SUTURO.owl#PringlesChipsCan">
        <rdfs:subClassOf rdf:resource="http://www.ease-crc.org/ont/SUTURO.owl#ChipsCan"/>
        <rdfs:subClassOf rdf:resource="http://www.ease-crc.org/ont/SUTURO.owl#RoboCupSnacks"/>
        <rdfs:subClassOf>
            <owl:Restriction>
                <owl:onProperty rdf:resource="http://www.ease-crc.org/ont/SUTURO.owl#hasPredefinedName"/>
                <owl:hasValue>pringles</owl:hasValue>
            </owl:Restriction>
        </rdfs:subClassOf>
        <SUTURO:perceptionId rdf:datatype="http://www.w3.org/2001/XMLSchema#int">36</SUTURO:perceptionId>
        <rdfs:comment>Pringles chips can refers to a cylindrical container that holds Pringles brand potato chips.</rdfs:comment>
        <rdfs:isDefinedBy rdf:resource="http://www.ease-crc.org/ont/SUTURO.owl"/>
    </owl:Class>
    


    <!-- http://www.ease-crc.org/ont/SUTURO.owl#PrintedMatter -->

    <owl:Class rdf:about="http://www.ease-crc.org/ont/SUTURO.owl#PrintedMatter">
        <rdfs:subClassOf rdf:resource="http://www.ontologydesignpatterns.org/ont/dul/DUL.owl#DesignedArtifact"/>
        <rdfs:comment>Printed matter refers to any material that has been printed, including books, magazines, newspapers, brochures, flyers, posters, and other forms of printed media.</rdfs:comment>
        <rdfs:isDefinedBy rdf:resource="http://www.ease-crc.org/ont/SUTURO.owl"/>
    </owl:Class>
    


    <!-- http://www.ease-crc.org/ont/SUTURO.owl#ProcessedFood -->

    <owl:Class rdf:about="http://www.ease-crc.org/ont/SUTURO.owl#ProcessedFood">
        <rdfs:subClassOf rdf:resource="http://www.ease-crc.org/ont/SOMA.owl#Dish"/>
        <rdfs:subClassOf rdf:resource="http://www.ease-crc.org/ont/SUTURO.owl#Food"/>
        <rdfs:subClassOf>
            <owl:Restriction>
                <owl:onProperty rdf:resource="http://www.ease-crc.org/ont/SUTURO.owl#hasPredefinedName"/>
                <owl:hasValue>processed food</owl:hasValue>
            </owl:Restriction>
        </rdfs:subClassOf>
        <rdfs:comment>Processed food refers to food that has been altered in some way from its natural state through various methods such as canning, freezing, cooking, or adding preservatives and additives. It often contains high amounts of salt, sugar, and fat, and is typically less nutritious than fresh, unprocessed food.</rdfs:comment>
        <rdfs:isDefinedBy rdf:resource="http://www.ease-crc.org/ont/SUTURO.owl"/>
    </owl:Class>
    


    <!-- http://www.ease-crc.org/ont/SUTURO.owl#PuddingBox -->

    <owl:Class rdf:about="http://www.ease-crc.org/ont/SUTURO.owl#PuddingBox">
        <rdfs:subClassOf rdf:resource="http://www.ease-crc.org/ont/SOMA.owl#Box"/>
        <rdfs:subClassOf>
            <owl:Restriction>
                <owl:onProperty rdf:resource="http://www.ease-crc.org/ont/SUTURO.owl#hasPredefinedName"/>
                <owl:hasValue>pudding box</owl:hasValue>
            </owl:Restriction>
        </rdfs:subClassOf>
        <rdfs:comment>A box containing, or at least normally intended to contain pudding powder.</rdfs:comment>
        <rdfs:isDefinedBy rdf:resource="http://www.ease-crc.org/ont/SUTURO.owl"/>
    </owl:Class>
    


    <!-- http://www.ease-crc.org/ont/SUTURO.owl#Pullover -->

    <owl:Class rdf:about="http://www.ease-crc.org/ont/SUTURO.owl#Pullover">
        <rdfs:subClassOf rdf:resource="http://www.ease-crc.org/ont/SUTURO.owl#Clothing"/>
        <rdfs:subClassOf>
            <owl:Restriction>
                <owl:onProperty rdf:resource="http://www.ease-crc.org/ont/SUTURO.owl#hasPredefinedName"/>
                <owl:hasValue>pullover</owl:hasValue>
            </owl:Restriction>
        </rdfs:subClassOf>
        <rdfs:isDefinedBy rdf:resource="http://www.ease-crc.org/ont/SUTURO.owl"/>
    </owl:Class>
    


    <!-- http://www.ease-crc.org/ont/SUTURO.owl#Rack -->

    <owl:Class rdf:about="http://www.ease-crc.org/ont/SUTURO.owl#Rack">
        <rdfs:subClassOf rdf:resource="http://www.ease-crc.org/ont/SOMA.owl#DesignedFurniture"/>
        <rdfs:subClassOf>
            <owl:Restriction>
                <owl:onProperty rdf:resource="http://www.ease-crc.org/ont/SUTURO.owl#hasPredefinedName"/>
                <owl:hasValue>rack</owl:hasValue>
            </owl:Restriction>
        </rdfs:subClassOf>
        <rdfs:comment>A rack is a framework or support structure used for holding or organizing various objects or equipment in a specific arrangement or pattern.</rdfs:comment>
        <rdfs:isDefinedBy rdf:resource="http://www.ease-crc.org/ont/SUTURO.owl"/>
    </owl:Class>
    


    <!-- http://www.ease-crc.org/ont/SUTURO.owl#Racquetball -->

    <owl:Class rdf:about="http://www.ease-crc.org/ont/SUTURO.owl#Racquetball">
        <rdfs:subClassOf rdf:resource="http://www.ease-crc.org/ont/SUTURO.owl#Ball"/>
        <rdfs:subClassOf>
            <owl:Restriction>
                <owl:onProperty rdf:resource="http://www.ease-crc.org/ont/SUTURO.owl#hasPredefinedName"/>
                <owl:hasValue>racquet ball</owl:hasValue>
            </owl:Restriction>
        </rdfs:subClassOf>
        <SUTURO:perceptionId rdf:datatype="http://www.w3.org/2001/XMLSchema#int">47</SUTURO:perceptionId>
        <rdfs:comment>A racquetball ball is a small, hollow rubber ball used in the sport of racquetball, designed to be bouncy and to move quickly in the enclosed court.</rdfs:comment>
        <rdfs:isDefinedBy rdf:resource="http://www.ease-crc.org/ont/SUTURO.owl"/>
    </owl:Class>
    


    <!-- http://www.ease-crc.org/ont/SUTURO.owl#RaspberryJuice -->

    <owl:Class rdf:about="http://www.ease-crc.org/ont/SUTURO.owl#RaspberryJuice">
        <rdfs:subClassOf rdf:resource="http://www.ease-crc.org/ont/SUTURO.owl#Juice"/>
        <rdfs:subClassOf>
            <owl:Restriction>
                <owl:onProperty rdf:resource="http://www.ease-crc.org/ont/SUTURO.owl#hasPredefinedName"/>
                <owl:hasValue>raspberry juice</owl:hasValue>
            </owl:Restriction>
        </rdfs:subClassOf>
        <rdfs:comment>Raspberry juice is a beverage made by pressing or extracting the natural liquid from raspberries, a sweet and tart fruit. It is often consumed as a refreshing drink or used as an ingredient in cocktails, smoothies, and other beverages. Raspberry juice is also believed to be a good source of vitamin C and other nutrients.</rdfs:comment>
        <rdfs:isDefinedBy rdf:resource="http://www.ease-crc.org/ont/SUTURO.owl"/>
    </owl:Class>
    


    <!-- http://www.ease-crc.org/ont/SUTURO.owl#RaspberryJuiceBox -->

    <owl:Class rdf:about="http://www.ease-crc.org/ont/SUTURO.owl#RaspberryJuiceBox">
        <rdfs:subClassOf rdf:resource="http://www.ease-crc.org/ont/SUTURO.owl#JuiceBox"/>
        <rdfs:subClassOf>
            <owl:Restriction>
                <owl:onProperty rdf:resource="http://www.ease-crc.org/ont/SUTURO.owl#hasPredefinedName"/>
                <owl:hasValue>raspberry juice box</owl:hasValue>
            </owl:Restriction>
        </rdfs:subClassOf>
        <rdfs:comment>A raspberry juice box is a small, rectangular-shaped container typically made of cardboard or plastic, designed to hold and dispense raspberry juice. It often includes a straw or a screw-on cap for easy access and is a popular choice for on-the-go consumption.</rdfs:comment>
        <rdfs:isDefinedBy rdf:resource="http://www.ease-crc.org/ont/SUTURO.owl"/>
    </owl:Class>
    


    <!-- http://www.ease-crc.org/ont/SUTURO.owl#RedWine -->

    <owl:Class rdf:about="http://www.ease-crc.org/ont/SUTURO.owl#RedWine">
        <rdfs:subClassOf rdf:resource="http://www.ease-crc.org/ont/SUTURO.owl#Drink"/>
        <rdfs:subClassOf>
            <owl:Restriction>
                <owl:onProperty rdf:resource="http://www.ease-crc.org/ont/SUTURO.owl#hasPredefinedName"/>
                <owl:hasValue>red wine</owl:hasValue>
            </owl:Restriction>
        </rdfs:subClassOf>
        <rdfs:isDefinedBy rdf:resource="http://www.ease-crc.org/ont/SUTURO.owl"/>
    </owl:Class>
    


    <!-- http://www.ease-crc.org/ont/SUTURO.owl#RoboCup2023Categories -->

    <owl:Class rdf:about="http://www.ease-crc.org/ont/SUTURO.owl#RoboCup2023Categories">
        <rdfs:subClassOf rdf:resource="http://www.ease-crc.org/ont/SUTURO.owl#PredefinedCategory"/>
        <rdfs:comment>Categories of objects in RoboCup@Home 2023 Bordeaux</rdfs:comment>
        <rdfs:isDefinedBy rdf:resource="http://www.ease-crc.org/ont/SUTURO.owl"/>
    </owl:Class>
    


    <!-- http://www.ease-crc.org/ont/SUTURO.owl#RoboCupChallenge -->

    <owl:Class rdf:about="http://www.ease-crc.org/ont/SUTURO.owl#RoboCupChallenge">
        <rdfs:subClassOf rdf:resource="http://www.ontologydesignpatterns.org/ont/dul/DUL.owl#Plan"/>
        <rdfs:comment>The RoboCup@Home competition consists of a series of challenges/tests which the robots have to solve, and the specific tests will change over the years to become more advanced. The performance of the robots is evaluated based on a score derived from competition rules and evaluation by a jury.

The challenges in the RoboCup@Home competition are designed to test a variety of skills relevant to domestic service robots.</rdfs:comment>
        <rdfs:isDefinedBy rdf:resource="http://www.ease-crc.org/ont/SUTURO.owl#"/>
    </owl:Class>
    


    <!-- http://www.ease-crc.org/ont/SUTURO.owl#RoboCupCleaningSupplies -->

    <owl:Class rdf:about="http://www.ease-crc.org/ont/SUTURO.owl#RoboCupCleaningSupplies">
        <rdfs:subClassOf rdf:resource="http://www.ease-crc.org/ont/SUTURO.owl#RoboCup2023Categories"/>
        <rdfs:isDefinedBy rdf:resource="http://www.ease-crc.org/ont/SUTURO.owl"/>
        <rdfs:label>Cleaning supplies</rdfs:label>
    </owl:Class>
    


    <!-- http://www.ease-crc.org/ont/SUTURO.owl#RoboCupDishes -->

    <owl:Class rdf:about="http://www.ease-crc.org/ont/SUTURO.owl#RoboCupDishes">
        <rdfs:subClassOf rdf:resource="http://www.ease-crc.org/ont/SUTURO.owl#RoboCup2023Categories"/>
        <rdfs:isDefinedBy rdf:resource="http://www.ease-crc.org/ont/SUTURO.owl"/>
        <rdfs:label>Dishes</rdfs:label>
    </owl:Class>
    


    <!-- http://www.ease-crc.org/ont/SUTURO.owl#RoboCupDrinks -->

    <owl:Class rdf:about="http://www.ease-crc.org/ont/SUTURO.owl#RoboCupDrinks">
        <rdfs:subClassOf rdf:resource="http://www.ease-crc.org/ont/SUTURO.owl#Drink"/>
        <rdfs:subClassOf rdf:resource="http://www.ease-crc.org/ont/SUTURO.owl#RoboCup2023Categories"/>
        <rdfs:subClassOf rdf:resource="http://www.ease-crc.org/ont/SUTURO.owl#RoboCupDrinks"/>
        <rdfs:subClassOf>
            <owl:Restriction>
                <owl:onProperty rdf:resource="http://www.ease-crc.org/ont/SUTURO.owl#hasGraspPose"/>
                <owl:hasValue>front</owl:hasValue>
            </owl:Restriction>
        </rdfs:subClassOf>
        <rdfs:isDefinedBy rdf:resource="http://www.ease-crc.org/ont/SUTURO.owl"/>
        <rdfs:label>Drinks</rdfs:label>
    </owl:Class>
    


    <!-- http://www.ease-crc.org/ont/SUTURO.owl#RoboCupFood -->

    <owl:Class rdf:about="http://www.ease-crc.org/ont/SUTURO.owl#RoboCupFood">
        <rdfs:subClassOf rdf:resource="http://www.ease-crc.org/ont/SUTURO.owl#RoboCup2023Categories"/>
        <rdfs:isDefinedBy rdf:resource="http://www.ease-crc.org/ont/SUTURO.owl"/>
        <rdfs:label>Food</rdfs:label>
    </owl:Class>
    


    <!-- http://www.ease-crc.org/ont/SUTURO.owl#RoboCupFruits -->

    <owl:Class rdf:about="http://www.ease-crc.org/ont/SUTURO.owl#RoboCupFruits">
        <rdfs:subClassOf rdf:resource="http://www.ease-crc.org/ont/SUTURO.owl#RoboCup2023Categories"/>
        <rdfs:isDefinedBy rdf:resource="http://www.ease-crc.org/ont/SUTURO.owl"/>
        <rdfs:label>Fruits</rdfs:label>
    </owl:Class>
    


    <!-- http://www.ease-crc.org/ont/SUTURO.owl#RoboCupSnacks -->

    <owl:Class rdf:about="http://www.ease-crc.org/ont/SUTURO.owl#RoboCupSnacks">
        <rdfs:subClassOf rdf:resource="http://www.ease-crc.org/ont/SUTURO.owl#RoboCup2023Categories"/>
        <rdfs:subClassOf>
            <owl:Restriction>
                <owl:onProperty rdf:resource="http://www.ease-crc.org/ont/SUTURO.owl#hasGraspPose"/>
                <owl:hasValue>front</owl:hasValue>
            </owl:Restriction>
        </rdfs:subClassOf>
        <rdfs:isDefinedBy rdf:resource="http://www.ease-crc.org/ont/SUTURO.owl"/>
        <rdfs:label>Snacks</rdfs:label>
    </owl:Class>
    


    <!-- http://www.ease-crc.org/ont/SUTURO.owl#RoboCupToys -->

    <owl:Class rdf:about="http://www.ease-crc.org/ont/SUTURO.owl#RoboCupToys">
        <rdfs:subClassOf rdf:resource="http://www.ease-crc.org/ont/SUTURO.owl#RoboCup2023Categories"/>
        <rdfs:isDefinedBy rdf:resource="http://www.ease-crc.org/ont/SUTURO.owl"/>
        <rdfs:label>Toys</rdfs:label>
    </owl:Class>
    


    <!-- http://www.ease-crc.org/ont/SUTURO.owl#Rope -->

    <owl:Class rdf:about="http://www.ease-crc.org/ont/SUTURO.owl#Rope">
        <rdfs:subClassOf rdf:resource="http://www.ease-crc.org/ont/SUTURO.owl#Fastener"/>
        <rdfs:subClassOf>
            <owl:Restriction>
                <owl:onProperty rdf:resource="http://www.ease-crc.org/ont/SUTURO.owl#hasPredefinedName"/>
                <owl:hasValue>rope</owl:hasValue>
            </owl:Restriction>
        </rdfs:subClassOf>
        <SUTURO:perceptionId rdf:datatype="http://www.w3.org/2001/XMLSchema#int">44</SUTURO:perceptionId>
        <rdfs:comment>A rope is a length of thick, strong, twisted or braided fibers or cords, typically made of natural or synthetic materials, used for tying, lifting, pulling, or securing objects or people.</rdfs:comment>
        <rdfs:isDefinedBy rdf:resource="http://www.ease-crc.org/ont/SUTURO.owl"/>
    </owl:Class>
    


    <!-- http://www.ease-crc.org/ont/SUTURO.owl#RubiksCube -->

    <owl:Class rdf:about="http://www.ease-crc.org/ont/SUTURO.owl#RubiksCube">
        <rdfs:subClassOf rdf:resource="http://www.ease-crc.org/ont/SUTURO.owl#RoboCupToys"/>
        <rdfs:subClassOf rdf:resource="http://www.ease-crc.org/ont/SUTURO.owl#Toy"/>
        <rdfs:subClassOf>
            <owl:Restriction>
                <owl:onProperty rdf:resource="http://www.ease-crc.org/ont/SUTURO.owl#hasPredefinedName"/>
                <owl:hasValue>rubiks cube</owl:hasValue>
            </owl:Restriction>
        </rdfs:subClassOf>
        <SUTURO:perceptionId rdf:datatype="http://www.w3.org/2001/XMLSchema#int">88</SUTURO:perceptionId>
        <rdfs:comment>A Rubik&apos;s Cube is a three-dimensional puzzle game that consists of a cube with six faces, each made up of nine smaller squares of different colors, and the object of the game is to twist and turn the cube to solve the puzzle by aligning the colors on each face.</rdfs:comment>
        <rdfs:isDefinedBy rdf:resource="http://www.ease-crc.org/ont/SUTURO.owl"/>
    </owl:Class>
    


    <!-- http://www.ease-crc.org/ont/SUTURO.owl#Salt -->

    <owl:Class rdf:about="http://www.ease-crc.org/ont/SUTURO.owl#Salt">
        <rdfs:subClassOf rdf:resource="http://www.ease-crc.org/ont/SUTURO.owl#Mineral"/>
        <rdfs:subClassOf rdf:resource="http://www.ease-crc.org/ont/SUTURO.owl#Spice"/>
        <rdfs:subClassOf>
            <owl:Restriction>
                <owl:onProperty rdf:resource="http://www.ease-crc.org/ont/SUTURO.owl#hasPredefinedName"/>
                <owl:hasValue>salt</owl:hasValue>
            </owl:Restriction>
        </rdfs:subClassOf>
        <rdfs:comment>Salt is a mineral substance that is composed of sodium and chloride ions and is commonly used as a seasoning and preservative in food. It is an essential nutrient for the human body and is found in many natural sources such as seawater and rock formations.</rdfs:comment>
        <rdfs:isDefinedBy rdf:resource="http://www.ease-crc.org/ont/SUTURO.owl"/>
    </owl:Class>
    


    <!-- http://www.ease-crc.org/ont/SUTURO.owl#Sandwich -->

    <owl:Class rdf:about="http://www.ease-crc.org/ont/SUTURO.owl#Sandwich">
        <rdfs:subClassOf rdf:resource="http://www.ease-crc.org/ont/SUTURO.owl#ProcessedFood"/>
        <rdfs:subClassOf>
            <owl:Restriction>
                <owl:onProperty rdf:resource="http://www.ease-crc.org/ont/SUTURO.owl#hasPredefinedName"/>
                <owl:hasValue>sandwich</owl:hasValue>
            </owl:Restriction>
        </rdfs:subClassOf>
        <rdfs:isDefinedBy rdf:resource="http://www.ease-crc.org/ont/SUTURO.owl"/>
    </owl:Class>
    


    <!-- http://www.ease-crc.org/ont/SUTURO.owl#Sausages -->

    <owl:Class rdf:about="http://www.ease-crc.org/ont/SUTURO.owl#Sausages">
        <rdfs:subClassOf rdf:resource="http://www.ease-crc.org/ont/SUTURO.owl#Meat"/>
        <rdfs:subClassOf rdf:resource="http://www.ease-crc.org/ont/SUTURO.owl#RoboCupFood"/>
        <rdfs:subClassOf>
            <owl:Restriction>
                <owl:onProperty rdf:resource="http://www.ease-crc.org/ont/SUTURO.owl#hasPredefinedName"/>
                <owl:hasValue>sausages</owl:hasValue>
            </owl:Restriction>
        </rdfs:subClassOf>
        <SUTURO:perceptionId rdf:datatype="http://www.w3.org/2001/XMLSchema#decimal">120</SUTURO:perceptionId>
        <rdfs:isDefinedBy rdf:resource="http://www.ease-crc.org/ont/SUTURO.owl"/>
    </owl:Class>
    


    <!-- http://www.ease-crc.org/ont/SUTURO.owl#Scissors -->

    <owl:Class rdf:about="http://www.ease-crc.org/ont/SUTURO.owl#Scissors">
        <rdfs:subClassOf rdf:resource="http://www.ease-crc.org/ont/SOMA.owl#CuttingTool"/>
        <rdfs:subClassOf>
            <owl:Restriction>
                <owl:onProperty rdf:resource="http://www.ease-crc.org/ont/SOMA.owl#hasPhysicalComponent"/>
                <owl:someValuesFrom rdf:resource="http://www.ease-crc.org/ont/SOMA.owl#Blade"/>
            </owl:Restriction>
        </rdfs:subClassOf>
        <rdfs:subClassOf>
            <owl:Restriction>
                <owl:onProperty rdf:resource="http://www.ease-crc.org/ont/SUTURO.owl#hasPredefinedName"/>
                <owl:hasValue>scissors</owl:hasValue>
            </owl:Restriction>
        </rdfs:subClassOf>
        <SUTURO:perceptionId rdf:datatype="http://www.w3.org/2001/XMLSchema#decimal">98</SUTURO:perceptionId>
        <rdfs:comment>Scissors are a cutting tool consisting of two blades joined together by a pivot, used for cutting paper, fabric, hair, or other materials.</rdfs:comment>
        <rdfs:isDefinedBy rdf:resource="http://www.ease-crc.org/ont/SUTURO.owl"/>
    </owl:Class>
    


    <!-- http://www.ease-crc.org/ont/SUTURO.owl#ScotchBriteDobieSponge -->

    <owl:Class rdf:about="http://www.ease-crc.org/ont/SUTURO.owl#ScotchBriteDobieSponge">
        <rdfs:subClassOf rdf:resource="http://www.ease-crc.org/ont/SUTURO.owl#AbrasiveSponge"/>
        <rdfs:subClassOf>
            <owl:Restriction>
                <owl:onProperty rdf:resource="http://www.ease-crc.org/ont/SUTURO.owl#hasPredefinedName"/>
                <owl:hasValue>scotch brite dobie sponge</owl:hasValue>
            </owl:Restriction>
        </rdfs:subClassOf>
        <rdfs:comment>A Scotch Brite Dobie sponge is a small, rectangular sponge with a scrubbing surface on one side, designed for cleaning dishes and surfaces.</rdfs:comment>
        <rdfs:isDefinedBy rdf:resource="http://www.ease-crc.org/ont/SUTURO.owl"/>
    </owl:Class>
    


    <!-- http://www.ease-crc.org/ont/SUTURO.owl#Screw -->

    <owl:Class rdf:about="http://www.ease-crc.org/ont/SUTURO.owl#Screw">
        <rdfs:subClassOf rdf:resource="http://www.ease-crc.org/ont/SUTURO.owl#Fastener"/>
        <rdfs:subClassOf rdf:resource="http://www.ease-crc.org/ont/SUTURO.owl#MetalHardware"/>
        <rdfs:subClassOf>
            <owl:Restriction>
                <owl:onProperty rdf:resource="http://www.ease-crc.org/ont/SUTURO.owl#hasPredefinedName"/>
                <owl:hasValue>screw</owl:hasValue>
            </owl:Restriction>
        </rdfs:subClassOf>
        <rdfs:comment>A screw is a threaded metal or wood fastener with a pointed tip used for attaching two objects together or for securing an object in place.</rdfs:comment>
        <rdfs:isDefinedBy rdf:resource="http://www.ease-crc.org/ont/SUTURO.owl"/>
    </owl:Class>
    


    <!-- http://www.ease-crc.org/ont/SUTURO.owl#ScrewDriver -->

    <owl:Class rdf:about="http://www.ease-crc.org/ont/SUTURO.owl#ScrewDriver">
        <rdfs:subClassOf rdf:resource="http://www.ease-crc.org/ont/SUTURO.owl#ForceConcentratingTool"/>
        <rdfs:subClassOf>
            <owl:Restriction>
                <owl:onProperty rdf:resource="http://www.ease-crc.org/ont/SOMA.owl#hasPhysicalComponent"/>
                <owl:someValuesFrom rdf:resource="http://www.ease-crc.org/ont/SOMA.owl#DesignedHandle"/>
            </owl:Restriction>
        </rdfs:subClassOf>
        <rdfs:subClassOf>
            <owl:Restriction>
                <owl:onProperty rdf:resource="http://www.ease-crc.org/ont/SUTURO.owl#hasPredefinedName"/>
                <owl:hasValue>screwdriver</owl:hasValue>
            </owl:Restriction>
        </rdfs:subClassOf>
        <SUTURO:perceptionId rdf:datatype="http://www.w3.org/2001/XMLSchema#decimal">102</SUTURO:perceptionId>
        <rdfs:comment>A screwdriver is a hand tool consisting of a handle and a shaft with a shaped tip designed to fit into the corresponding slot or recess of a screw head. It is used for turning screws to fasten or loosen them in a wide range of applications, from construction and carpentry to electronics and household repairs.</rdfs:comment>
        <rdfs:isDefinedBy rdf:resource="http://www.ease-crc.org/ont/SUTURO.owl"/>
    </owl:Class>
    


    <!-- http://www.ease-crc.org/ont/SUTURO.owl#ScrubCleaner -->

    <owl:Class rdf:about="http://www.ease-crc.org/ont/SUTURO.owl#ScrubCleaner">
        <rdfs:subClassOf rdf:resource="http://www.ease-crc.org/ont/SUTURO.owl#CleaningProduct"/>
        <rdfs:subClassOf>
            <owl:Restriction>
                <owl:onProperty rdf:resource="http://www.ease-crc.org/ont/SUTURO.owl#hasPredefinedName"/>
                <owl:hasValue>scrub cleaner</owl:hasValue>
            </owl:Restriction>
        </rdfs:subClassOf>
        <SUTURO:perceptionId rdf:datatype="http://www.w3.org/2001/XMLSchema#decimal">99</SUTURO:perceptionId>
        <rdfs:isDefinedBy rdf:resource="http://www.ease-crc.org/ont/SUTURO.owl"/>
    </owl:Class>
    


    <!-- http://www.ease-crc.org/ont/SUTURO.owl#ServingMat -->

    <owl:Class rdf:about="http://www.ease-crc.org/ont/SUTURO.owl#ServingMat">
        <rdfs:subClassOf rdf:resource="http://www.ease-crc.org/ont/SUTURO.owl#DesignedFabric"/>
        <rdfs:subClassOf>
            <owl:Restriction>
                <owl:onProperty rdf:resource="http://www.ease-crc.org/ont/SUTURO.owl#hasPredefinedName"/>
                <owl:hasValue>serving mat</owl:hasValue>
            </owl:Restriction>
        </rdfs:subClassOf>
        <SUTURO:perceptionId rdf:datatype="http://www.w3.org/2001/XMLSchema#int">21</SUTURO:perceptionId>
        <rdfs:comment>A serving mat is a type of table mat used to protect surfaces from spills and stains while serving food or drinks. They are typically made from materials such as fabric, plastic, or silicone and come in various shapes, sizes, and designs to suit different occasions and styles.</rdfs:comment>
        <rdfs:isDefinedBy rdf:resource="http://www.ease-crc.org/ont/SUTURO.owl"/>
    </owl:Class>
    


    <!-- http://www.ease-crc.org/ont/SUTURO.owl#Shampoo -->

    <owl:Class rdf:about="http://www.ease-crc.org/ont/SUTURO.owl#Shampoo">
        <rdfs:subClassOf rdf:resource="http://www.ease-crc.org/ont/SUTURO.owl#HygieneProduct"/>
        <rdfs:subClassOf>
            <owl:Restriction>
                <owl:onProperty rdf:resource="http://www.ease-crc.org/ont/SUTURO.owl#hasPredefinedName"/>
                <owl:hasValue>shampoo</owl:hasValue>
            </owl:Restriction>
        </rdfs:subClassOf>
        <rdfs:isDefinedBy rdf:resource="http://www.ease-crc.org/ont/SUTURO.owl"/>
    </owl:Class>
    


    <!-- http://www.ease-crc.org/ont/SUTURO.owl#ShelfLayer -->

    <owl:Class rdf:about="http://www.ease-crc.org/ont/SUTURO.owl#ShelfLayer">
        <rdfs:subClassOf rdf:resource="http://www.ease-crc.org/ont/SOMA.owl#DesignedComponent"/>
        <SUTURO:perceptionId rdf:datatype="http://www.w3.org/2001/XMLSchema#int">25</SUTURO:perceptionId>
        <rdfs:comment>A shelf board is a flat piece of wood, metal, or glass which is attached to a wall or to the sides of a cupboard. Shelves are used for keeping things on.</rdfs:comment>
        <rdfs:isDefinedBy rdf:resource="http://www.ease-crc.org/ont/SUTURO.owl"/>
        <rdfs:label>ShelfLayer</rdfs:label>
    </owl:Class>
    


    <!-- http://www.ease-crc.org/ont/SUTURO.owl#ShelfUnit -->

    <owl:Class rdf:about="http://www.ease-crc.org/ont/SUTURO.owl#ShelfUnit">
        <rdfs:subClassOf rdf:resource="http://www.ease-crc.org/ont/SUTURO.owl#Rack"/>
        <rdfs:subClassOf>
            <owl:Restriction>
                <owl:onProperty rdf:resource="http://www.ease-crc.org/ont/SUTURO.owl#hasPredefinedName"/>
                <owl:hasValue>shelf unit</owl:hasValue>
            </owl:Restriction>
        </rdfs:subClassOf>
        <rdfs:comment>A shelf unit is a piece of furniture consisting of several shelves, designed to hold books, decor, and other items and is typically made of wood or metal.</rdfs:comment>
        <rdfs:isDefinedBy>http://www.ease-crc.org/ont/SUTURO.owl</rdfs:isDefinedBy>
        <rdfs:label>ShelfUnit</rdfs:label>
    </owl:Class>
    


    <!-- http://www.ease-crc.org/ont/SUTURO.owl#Shirt -->

    <owl:Class rdf:about="http://www.ease-crc.org/ont/SUTURO.owl#Shirt">
        <rdfs:subClassOf rdf:resource="http://www.ease-crc.org/ont/SUTURO.owl#Clothing"/>
        <rdfs:subClassOf>
            <owl:Restriction>
                <owl:onProperty rdf:resource="http://www.ease-crc.org/ont/SUTURO.owl#hasPredefinedName"/>
                <owl:hasValue>shirt</owl:hasValue>
            </owl:Restriction>
        </rdfs:subClassOf>
        <rdfs:isDefinedBy rdf:resource="http://www.ease-crc.org/ont/SUTURO.owl"/>
    </owl:Class>
    


    <!-- http://www.ease-crc.org/ont/SUTURO.owl#Shoes -->

    <owl:Class rdf:about="http://www.ease-crc.org/ont/SUTURO.owl#Shoes">
        <rdfs:subClassOf rdf:resource="http://www.ease-crc.org/ont/SUTURO.owl#Clothing"/>
        <rdfs:subClassOf>
            <owl:Restriction>
                <owl:onProperty rdf:resource="http://www.ease-crc.org/ont/SUTURO.owl#hasPredefinedName"/>
                <owl:hasValue>shoes</owl:hasValue>
            </owl:Restriction>
        </rdfs:subClassOf>
        <rdfs:isDefinedBy rdf:resource="http://www.ease-crc.org/ont/SUTURO.owl"/>
    </owl:Class>
    


    <!-- http://www.ease-crc.org/ont/SUTURO.owl#Sink -->

    <owl:Class rdf:about="http://www.ease-crc.org/ont/SUTURO.owl#Sink">
        <rdfs:subClassOf rdf:resource="http://www.ease-crc.org/ont/SOMA.owl#Appliance"/>
        <rdfs:subClassOf rdf:resource="http://www.ease-crc.org/ont/SOMA.owl#DesignedContainer"/>
        <rdfs:subClassOf>
            <owl:Restriction>
                <owl:onProperty rdf:resource="http://www.ease-crc.org/ont/SUTURO.owl#hasPredefinedName"/>
                <owl:hasValue>sink</owl:hasValue>
            </owl:Restriction>
        </rdfs:subClassOf>
        <rdfs:comment>A sink is a bowl-shaped fixture used for washing hands, dishes, and other small objects, typically located in a kitchen or bathroom.</rdfs:comment>
        <rdfs:isDefinedBy rdf:resource="http://www.ease-crc.org/ont/SUTURO.owl"/>
    </owl:Class>
    


    <!-- http://www.ease-crc.org/ont/SUTURO.owl#Skillet -->

    <owl:Class rdf:about="http://www.ease-crc.org/ont/SUTURO.owl#Skillet">
        <rdfs:subClassOf rdf:resource="http://www.ease-crc.org/ont/SOMA.owl#Pan"/>
        <rdfs:subClassOf>
            <owl:Restriction>
                <owl:onProperty rdf:resource="http://www.ease-crc.org/ont/SUTURO.owl#hasPredefinedName"/>
                <owl:hasValue>skillet</owl:hasValue>
            </owl:Restriction>
        </rdfs:subClassOf>
        <SUTURO:perceptionId rdf:datatype="http://www.w3.org/2001/XMLSchema#int">58</SUTURO:perceptionId>
        <rdfs:comment>A skillet is a flat-bottomed pan with slanted sides and a long handle, used for frying, sautéing, or searing foods.</rdfs:comment>
        <rdfs:isDefinedBy rdf:resource="http://www.ease-crc.org/ont/SUTURO.owl"/>
    </owl:Class>
    


    <!-- http://www.ease-crc.org/ont/SUTURO.owl#SkilletLid -->

    <owl:Class rdf:about="http://www.ease-crc.org/ont/SUTURO.owl#SkilletLid">
        <rdfs:subClassOf rdf:resource="http://www.ease-crc.org/ont/SOMA.owl#Lid"/>
        <rdfs:comment>A skillet lid is a cover made of metal or glass that fits onto a skillet and is used to prevent splatters and retain heat while cooking.</rdfs:comment>
        <rdfs:isDefinedBy rdf:resource="http://www.ease-crc.org/ont/SUTURO.owl"/>
    </owl:Class>
    


    <!-- http://www.ease-crc.org/ont/SUTURO.owl#SmallMarker -->

    <owl:Class rdf:about="http://www.ease-crc.org/ont/SUTURO.owl#SmallMarker">
        <rdfs:subClassOf rdf:resource="http://www.ease-crc.org/ont/SUTURO.owl#WritingTool"/>
        <rdfs:subClassOf>
            <owl:Restriction>
                <owl:onProperty rdf:resource="http://www.ease-crc.org/ont/SUTURO.owl#hasPredefinedName"/>
                <owl:hasValue>small marker</owl:hasValue>
            </owl:Restriction>
        </rdfs:subClassOf>
        <rdfs:comment>A small marker is a pen-like writing tool with a narrow, pointed tip used for writing or drawing with precision, often used for labeling, highlighting, or coloring.</rdfs:comment>
        <rdfs:isDefinedBy rdf:resource="http://www.ease-crc.org/ont/SUTURO.owl"/>
    </owl:Class>
    


    <!-- http://www.ease-crc.org/ont/SUTURO.owl#Soap -->

    <owl:Class rdf:about="http://www.ease-crc.org/ont/SUTURO.owl#Soap">
        <rdfs:subClassOf rdf:resource="http://www.ease-crc.org/ont/SUTURO.owl#HygieneProduct"/>
        <rdfs:subClassOf rdf:resource="http://www.ease-crc.org/ont/SUTURO.owl#RoboCupCleaningSupplies"/>
        <rdfs:subClassOf>
            <owl:Restriction>
                <owl:onProperty rdf:resource="http://www.ease-crc.org/ont/SUTURO.owl#hasPredefinedName"/>
                <owl:hasValue>soap</owl:hasValue>
            </owl:Restriction>
        </rdfs:subClassOf>
        <SUTURO:perceptionId rdf:datatype="http://www.w3.org/2001/XMLSchema#decimal">109</SUTURO:perceptionId>
        <rdfs:isDefinedBy rdf:resource="http://www.ease-crc.org/ont/SUTURO.owl"/>
    </owl:Class>
    


    <!-- http://www.ease-crc.org/ont/SUTURO.owl#SoccerBall -->

    <owl:Class rdf:about="http://www.ease-crc.org/ont/SUTURO.owl#SoccerBall">
        <rdfs:subClassOf rdf:resource="http://www.ease-crc.org/ont/SUTURO.owl#Ball"/>
        <rdfs:subClassOf>
            <owl:Restriction>
                <owl:onProperty rdf:resource="http://www.ease-crc.org/ont/SUTURO.owl#hasPredefinedName"/>
                <owl:hasValue>soccer ball</owl:hasValue>
            </owl:Restriction>
        </rdfs:subClassOf>
        <rdfs:isDefinedBy rdf:resource="http://www.ease-crc.org/ont/SUTURO.owl"/>
    </owl:Class>
    


    <!-- http://www.ease-crc.org/ont/SUTURO.owl#Socks -->

    <owl:Class rdf:about="http://www.ease-crc.org/ont/SUTURO.owl#Socks">
        <rdfs:subClassOf rdf:resource="http://www.ease-crc.org/ont/SUTURO.owl#Clothing"/>
        <rdfs:subClassOf>
            <owl:Restriction>
                <owl:onProperty rdf:resource="http://www.ease-crc.org/ont/SUTURO.owl#hasPredefinedName"/>
                <owl:hasValue>socks</owl:hasValue>
            </owl:Restriction>
        </rdfs:subClassOf>
        <rdfs:isDefinedBy rdf:resource="http://www.ease-crc.org/ont/SUTURO.owl"/>
    </owl:Class>
    


    <!-- http://www.ease-crc.org/ont/SUTURO.owl#SoftBall -->

    <owl:Class rdf:about="http://www.ease-crc.org/ont/SUTURO.owl#SoftBall">
        <rdfs:subClassOf rdf:resource="http://www.ease-crc.org/ont/SUTURO.owl#Ball"/>
        <rdfs:subClassOf>
            <owl:Restriction>
                <owl:onProperty rdf:resource="http://www.ease-crc.org/ont/SUTURO.owl#hasPredefinedName"/>
                <owl:hasValue>soft ball</owl:hasValue>
            </owl:Restriction>
        </rdfs:subClassOf>
        <SUTURO:perceptionId rdf:datatype="http://www.w3.org/2001/XMLSchema#int">33</SUTURO:perceptionId>
        <rdfs:comment>A soft ball is a ball made of a softer, lighter material than a regulation baseball, often used in recreational or amateur leagues, or in games played by children.</rdfs:comment>
        <rdfs:isDefinedBy rdf:resource="http://www.ease-crc.org/ont/SUTURO.owl"/>
    </owl:Class>
    


    <!-- http://www.ease-crc.org/ont/SUTURO.owl#Soup -->

    <owl:Class rdf:about="http://www.ease-crc.org/ont/SUTURO.owl#Soup">
        <rdfs:subClassOf rdf:resource="http://www.ease-crc.org/ont/SUTURO.owl#Liquid"/>
        <rdfs:subClassOf rdf:resource="http://www.ease-crc.org/ont/SUTURO.owl#ProcessedFood"/>
        <rdfs:subClassOf>
            <owl:Restriction>
                <owl:onProperty rdf:resource="http://www.ease-crc.org/ont/SUTURO.owl#hasPredefinedName"/>
                <owl:hasValue>soup</owl:hasValue>
            </owl:Restriction>
        </rdfs:subClassOf>
        <rdfs:comment>Soup is a liquid dish made by cooking vegetables, meat, or fish in water or stock, and often seasoned with herbs and spices. It is a versatile dish that can be served hot or cold, as an appetizer or main course, and is enjoyed around the world for its comforting and nourishing qualities.</rdfs:comment>
        <rdfs:isDefinedBy rdf:resource="http://www.ease-crc.org/ont/SUTURO.owl"/>
    </owl:Class>
    


    <!-- http://www.ease-crc.org/ont/SUTURO.owl#SoupCan -->

    <owl:Class rdf:about="http://www.ease-crc.org/ont/SUTURO.owl#SoupCan">
        <rdfs:subClassOf rdf:resource="http://www.ease-crc.org/ont/SUTURO.owl#Can"/>
        <rdfs:subClassOf>
            <owl:Restriction>
                <owl:onProperty rdf:resource="http://www.ease-crc.org/ont/SUTURO.owl#hasPredefinedName"/>
                <owl:hasValue>soup can</owl:hasValue>
            </owl:Restriction>
        </rdfs:subClassOf>
        <rdfs:comment>Soup can refers to a cylindrical metal container that holds condensed or ready-to-eat soup.</rdfs:comment>
        <rdfs:isDefinedBy rdf:resource="http://www.ease-crc.org/ont/SUTURO.owl"/>
    </owl:Class>
    


    <!-- http://www.ease-crc.org/ont/SUTURO.owl#Spam -->

    <owl:Class rdf:about="http://www.ease-crc.org/ont/SUTURO.owl#Spam">
        <rdfs:subClassOf rdf:resource="http://www.ease-crc.org/ont/SUTURO.owl#Meat"/>
        <rdfs:subClassOf>
            <owl:Restriction>
                <owl:onProperty rdf:resource="http://www.ease-crc.org/ont/SUTURO.owl#hasPredefinedName"/>
                <owl:hasValue>spam</owl:hasValue>
            </owl:Restriction>
        </rdfs:subClassOf>
        <rdfs:isDefinedBy rdf:resource="http://www.ease-crc.org/ont/SUTURO.owl"/>
    </owl:Class>
    


    <!-- http://www.ease-crc.org/ont/SUTURO.owl#Spice -->

    <owl:Class rdf:about="http://www.ease-crc.org/ont/SUTURO.owl#Spice">
        <rdfs:subClassOf rdf:resource="http://www.ease-crc.org/ont/SUTURO.owl#Food"/>
        <rdfs:subClassOf>
            <owl:Restriction>
                <owl:onProperty rdf:resource="http://www.ease-crc.org/ont/SUTURO.owl#hasPredefinedName"/>
                <owl:hasValue>spice</owl:hasValue>
            </owl:Restriction>
        </rdfs:subClassOf>
        <rdfs:comment>Spices are a group of plant-based ingredients that are used to add flavor and aroma to food. They are typically dried and ground into powder or used fresh, and can be used alone or in combination with other spices to create complex flavors in dishes.</rdfs:comment>
        <rdfs:isDefinedBy rdf:resource="http://www.ease-crc.org/ont/SUTURO.owl"/>
    </owl:Class>
    


    <!-- http://www.ease-crc.org/ont/SUTURO.owl#Sponge -->

    <owl:Class rdf:about="http://www.ease-crc.org/ont/SUTURO.owl#Sponge">
        <rdfs:subClassOf rdf:resource="http://www.ease-crc.org/ont/SUTURO.owl#CleaningTool"/>
        <rdfs:subClassOf rdf:resource="http://www.ease-crc.org/ont/SUTURO.owl#RoboCupCleaningSupplies"/>
        <rdfs:subClassOf>
            <owl:Restriction>
                <owl:onProperty rdf:resource="http://www.ease-crc.org/ont/SUTURO.owl#hasPredefinedName"/>
                <owl:hasValue>sponge</owl:hasValue>
            </owl:Restriction>
        </rdfs:subClassOf>
        <SUTURO:perceptionId rdf:datatype="http://www.w3.org/2001/XMLSchema#decimal">107</SUTURO:perceptionId>
        <rdfs:comment>A sponge is a porous material that is typically used for cleaning surfaces or absorbing liquid.</rdfs:comment>
        <rdfs:isDefinedBy rdf:resource="http://www.ease-crc.org/ont/SUTURO.owl"/>
    </owl:Class>
    


    <!-- http://www.ease-crc.org/ont/SUTURO.owl#SprayBottle -->

    <owl:Class rdf:about="http://www.ease-crc.org/ont/SUTURO.owl#SprayBottle">
        <rdfs:subClassOf rdf:resource="http://www.ease-crc.org/ont/SOMA.owl#Bottle"/>
        <rdfs:subClassOf>
            <owl:Restriction>
                <owl:onProperty rdf:resource="http://www.ease-crc.org/ont/SUTURO.owl#hasPredefinedName"/>
                <owl:hasValue>spray bottle</owl:hasValue>
            </owl:Restriction>
        </rdfs:subClassOf>
        <rdfs:comment>A spray bottle is a type of container that holds liquid and has a nozzle that can spray the liquid in a fine mist or stream.</rdfs:comment>
        <rdfs:isDefinedBy rdf:resource="http://www.ease-crc.org/ont/SUTURO.owl"/>
    </owl:Class>
    


    <!-- http://www.ease-crc.org/ont/SUTURO.owl#Sprite -->

    <owl:Class rdf:about="http://www.ease-crc.org/ont/SUTURO.owl#Sprite">
        <rdfs:subClassOf rdf:resource="http://www.ease-crc.org/ont/SUTURO.owl#Drink"/>
        <rdfs:subClassOf>
            <owl:Restriction>
                <owl:onProperty rdf:resource="http://www.ease-crc.org/ont/SUTURO.owl#hasPredefinedName"/>
                <owl:hasValue>sprite</owl:hasValue>
            </owl:Restriction>
        </rdfs:subClassOf>
        <rdfs:isDefinedBy rdf:resource="http://www.ease-crc.org/ont/SUTURO.owl"/>
    </owl:Class>
    


    <!-- http://www.ease-crc.org/ont/SUTURO.owl#StackingBlocks -->

    <owl:Class rdf:about="http://www.ease-crc.org/ont/SUTURO.owl#StackingBlocks">
        <rdfs:subClassOf rdf:resource="http://www.ease-crc.org/ont/SUTURO.owl#Toy"/>
        <rdfs:subClassOf>
            <owl:Restriction>
                <owl:onProperty rdf:resource="http://www.ease-crc.org/ont/SUTURO.owl#hasPredefinedName"/>
                <owl:hasValue>stacking blocks</owl:hasValue>
            </owl:Restriction>
        </rdfs:subClassOf>
        <SUTURO:perceptionId rdf:datatype="http://www.w3.org/2001/XMLSchema#int">45</SUTURO:perceptionId>
        <rdfs:comment>Stacking blocks are a popular children&apos;s toy consisting of various sized and shaped blocks that can be stacked on top of each other to form towers or structures. They are often made of wood, plastic or foam, and are used to improve fine motor skills, hand-eye coordination, and problem-solving abilities in young children.</rdfs:comment>
        <rdfs:isDefinedBy rdf:resource="http://www.ease-crc.org/ont/SUTURO.owl"/>
    </owl:Class>
    


    <!-- http://www.ease-crc.org/ont/SUTURO.owl#StapelChips -->

    <owl:Class rdf:about="http://www.ease-crc.org/ont/SUTURO.owl#StapelChips">
        <rdfs:subClassOf rdf:resource="http://www.ease-crc.org/ont/SUTURO.owl#ChipsCan"/>
        <rdfs:subClassOf>
            <owl:Restriction>
                <owl:onProperty rdf:resource="http://www.ease-crc.org/ont/SUTURO.owl#hasPredefinedName"/>
                <owl:hasValue>stapel chips</owl:hasValue>
            </owl:Restriction>
        </rdfs:subClassOf>
        <SUTURO:perceptionId rdf:datatype="http://www.w3.org/2001/XMLSchema#decimal">93</SUTURO:perceptionId>
        <rdfs:isDefinedBy rdf:resource="http://www.ease-crc.org/ont/SUTURO.owl"/>
    </owl:Class>
    


    <!-- http://www.ease-crc.org/ont/SUTURO.owl#Steak -->

    <owl:Class rdf:about="http://www.ease-crc.org/ont/SUTURO.owl#Steak">
        <rdfs:subClassOf rdf:resource="http://www.ease-crc.org/ont/SUTURO.owl#Meat"/>
        <rdfs:subClassOf>
            <owl:Restriction>
                <owl:onProperty rdf:resource="http://www.ease-crc.org/ont/SUTURO.owl#hasPredefinedName"/>
                <owl:hasValue>steak</owl:hasValue>
            </owl:Restriction>
        </rdfs:subClassOf>
        <rdfs:isDefinedBy rdf:resource="http://www.ease-crc.org/ont/SUTURO.owl"/>
    </owl:Class>
    


    <!-- http://www.ease-crc.org/ont/SUTURO.owl#Strawberry -->

    <owl:Class rdf:about="http://www.ease-crc.org/ont/SUTURO.owl#Strawberry">
        <rdfs:subClassOf rdf:resource="http://www.ease-crc.org/ont/SUTURO.owl#Fruit"/>
        <rdfs:subClassOf rdf:resource="http://www.ease-crc.org/ont/SUTURO.owl#RoboCupFruits"/>
        <rdfs:subClassOf>
            <owl:Restriction>
                <owl:onProperty rdf:resource="http://www.ease-crc.org/ont/SUTURO.owl#hasPredefinedName"/>
                <owl:hasValue>strawberry</owl:hasValue>
            </owl:Restriction>
        </rdfs:subClassOf>
        <SUTURO:perceptionId rdf:datatype="http://www.w3.org/2001/XMLSchema#int">37</SUTURO:perceptionId>
        <rdfs:comment>A strawberry is a small, red fruit with a juicy texture, sweet taste, and tiny seeds on the surface, commonly used in desserts or as a snack.</rdfs:comment>
        <rdfs:isDefinedBy rdf:resource="http://www.ease-crc.org/ont/SUTURO.owl"/>
    </owl:Class>
    


    <!-- http://www.ease-crc.org/ont/SUTURO.owl#StrawberryJello -->

    <owl:Class rdf:about="http://www.ease-crc.org/ont/SUTURO.owl#StrawberryJello">
        <rdfs:subClassOf rdf:resource="http://www.ease-crc.org/ont/SUTURO.owl#Jello"/>
        <rdfs:subClassOf>
            <owl:Restriction>
                <owl:onProperty rdf:resource="http://www.ease-crc.org/ont/SUTURO.owl#hasPredefinedName"/>
                <owl:hasValue>strawberry jello</owl:hasValue>
            </owl:Restriction>
        </rdfs:subClassOf>
        <rdfs:isDefinedBy rdf:resource="http://www.ease-crc.org/ont/SUTURO.owl"/>
    </owl:Class>
    


    <!-- http://www.ease-crc.org/ont/SUTURO.owl#Stroopwafels -->

    <owl:Class rdf:about="http://www.ease-crc.org/ont/SUTURO.owl#Stroopwafels">
        <rdfs:subClassOf rdf:resource="http://www.ease-crc.org/ont/SUTURO.owl#RoboCupSnacks"/>
        <rdfs:subClassOf rdf:resource="http://www.ease-crc.org/ont/SUTURO.owl#Sweets"/>
        <rdfs:subClassOf>
            <owl:Restriction>
                <owl:onProperty rdf:resource="http://www.ease-crc.org/ont/SUTURO.owl#hasPredefinedName"/>
                <owl:hasValue>stroopwafels</owl:hasValue>
            </owl:Restriction>
        </rdfs:subClassOf>
        <SUTURO:perceptionId rdf:datatype="http://www.w3.org/2001/XMLSchema#decimal">124</SUTURO:perceptionId>
        <rdfs:isDefinedBy rdf:resource="http://www.ease-crc.org/ont/SUTURO.owl"/>
    </owl:Class>
    


    <!-- http://www.ease-crc.org/ont/SUTURO.owl#StudyRoom -->

    <owl:Class rdf:about="http://www.ease-crc.org/ont/SUTURO.owl#StudyRoom">
        <rdfs:subClassOf rdf:resource="http://www.ease-crc.org/ont/SOMA.owl#Room"/>
        <rdfs:subClassOf>
            <owl:Restriction>
                <owl:onProperty rdf:resource="http://www.ease-crc.org/ont/SUTURO.owl#hasPredefinedName"/>
                <owl:hasValue>study room</owl:hasValue>
            </owl:Restriction>
        </rdfs:subClassOf>
        <rdfs:comment>A room dedicated to studying and working, mostly by reading or writing.</rdfs:comment>
    </owl:Class>
    


    <!-- http://www.ease-crc.org/ont/SUTURO.owl#Sugar -->

    <owl:Class rdf:about="http://www.ease-crc.org/ont/SUTURO.owl#Sugar">
        <rdfs:subClassOf rdf:resource="http://www.ease-crc.org/ont/SUTURO.owl#Spice"/>
        <rdfs:subClassOf>
            <owl:Restriction>
                <owl:onProperty rdf:resource="http://www.ease-crc.org/ont/SUTURO.owl#hasPredefinedName"/>
                <owl:hasValue>sugar</owl:hasValue>
            </owl:Restriction>
        </rdfs:subClassOf>
        <rdfs:isDefinedBy rdf:resource="http://www.ease-crc.org/ont/SUTURO.owl"/>
    </owl:Class>
    


    <!-- http://www.ease-crc.org/ont/SUTURO.owl#SugarBox -->

    <owl:Class rdf:about="http://www.ease-crc.org/ont/SUTURO.owl#SugarBox">
        <rdfs:subClassOf rdf:resource="http://www.ease-crc.org/ont/SOMA.owl#Box"/>
        <rdfs:subClassOf rdf:resource="http://www.ease-crc.org/ont/SUTURO.owl#RoboCupFood"/>
        <rdfs:subClassOf>
            <owl:Restriction>
                <owl:onProperty rdf:resource="http://www.ease-crc.org/ont/SUTURO.owl#hasPredefinedName"/>
                <owl:hasValue>sugar box</owl:hasValue>
            </owl:Restriction>
        </rdfs:subClassOf>
        <SUTURO:perceptionId rdf:datatype="http://www.w3.org/2001/XMLSchema#int">57</SUTURO:perceptionId>
        <rdfs:comment>A box containing, or at least usually intended to contain, sugar.</rdfs:comment>
        <rdfs:isDefinedBy rdf:resource="http://www.ease-crc.org/ont/SUTURO.owl"/>
    </owl:Class>
    


    <!-- http://www.ease-crc.org/ont/SUTURO.owl#Sweater -->

    <owl:Class rdf:about="http://www.ease-crc.org/ont/SUTURO.owl#Sweater">
        <rdfs:subClassOf rdf:resource="http://www.ease-crc.org/ont/SUTURO.owl#Clothing"/>
        <rdfs:subClassOf>
            <owl:Restriction>
                <owl:onProperty rdf:resource="http://www.ease-crc.org/ont/SUTURO.owl#hasPredefinedName"/>
                <owl:hasValue>sweater</owl:hasValue>
            </owl:Restriction>
        </rdfs:subClassOf>
        <rdfs:isDefinedBy rdf:resource="http://www.ease-crc.org/ont/SUTURO.owl"/>
    </owl:Class>
    


    <!-- http://www.ease-crc.org/ont/SUTURO.owl#Sweets -->

    <owl:Class rdf:about="http://www.ease-crc.org/ont/SUTURO.owl#Sweets">
        <rdfs:subClassOf rdf:resource="http://www.ease-crc.org/ont/SUTURO.owl#ProcessedFood"/>
        <rdfs:subClassOf>
            <owl:Restriction>
                <owl:onProperty rdf:resource="http://www.ease-crc.org/ont/SUTURO.owl#hasPredefinedName"/>
                <owl:hasValue>sweets</owl:hasValue>
            </owl:Restriction>
        </rdfs:subClassOf>
        <rdfs:comment>Sweets, also known as candy, are a type of confectionery made from sugar or a sugar substitute, and often flavored with fruit, chocolate, or other ingredients. They come in a wide variety of forms such as hard candies, gummies, caramels, and chocolates, and are enjoyed as a treat or dessert.</rdfs:comment>
        <rdfs:isDefinedBy rdf:resource="http://www.ease-crc.org/ont/SUTURO.owl"/>
    </owl:Class>
    


    <!-- http://www.ease-crc.org/ont/SUTURO.owl#TableCloth -->

    <owl:Class rdf:about="http://www.ease-crc.org/ont/SUTURO.owl#TableCloth">
        <rdfs:subClassOf rdf:resource="http://www.ease-crc.org/ont/SUTURO.owl#DesignedFabric"/>
        <rdfs:subClassOf>
            <owl:Restriction>
                <owl:onProperty rdf:resource="http://www.ease-crc.org/ont/SUTURO.owl#hasPredefinedName"/>
                <owl:hasValue>table cloth</owl:hasValue>
            </owl:Restriction>
        </rdfs:subClassOf>
        <SUTURO:perceptionId rdf:datatype="http://www.w3.org/2001/XMLSchema#int">13</SUTURO:perceptionId>
        <rdfs:comment>A tablecloth is a large, rectangular piece of fabric or vinyl used to cover and protect a dining table from spills and stains, as well as to add aesthetic appeal to the setting.</rdfs:comment>
        <rdfs:isDefinedBy rdf:resource="http://www.ease-crc.org/ont/SUTURO.owl"/>
    </owl:Class>
    


    <!-- http://www.ease-crc.org/ont/SUTURO.owl#Tea -->

    <owl:Class rdf:about="http://www.ease-crc.org/ont/SUTURO.owl#Tea">
        <rdfs:subClassOf rdf:resource="http://www.ease-crc.org/ont/SUTURO.owl#Drink"/>
        <rdfs:subClassOf>
            <owl:Restriction>
                <owl:onProperty rdf:resource="http://www.ease-crc.org/ont/SUTURO.owl#hasPredefinedName"/>
                <owl:hasValue>tea</owl:hasValue>
            </owl:Restriction>
        </rdfs:subClassOf>
        <rdfs:comment>Tea is a hot or cold beverage made by steeping dried leaves from the tea plant, Camellia sinensis, in water. It is one of the most widely consumed beverages in the world and is enjoyed for its unique flavor, aroma, and potential health benefits.</rdfs:comment>
        <rdfs:isDefinedBy rdf:resource="http://www.ease-crc.org/ont/SUTURO.owl"/>
    </owl:Class>
    


    <!-- http://www.ease-crc.org/ont/SUTURO.owl#TeaBagBox -->

    <owl:Class rdf:about="http://www.ease-crc.org/ont/SUTURO.owl#TeaBagBox">
        <rdfs:subClassOf rdf:resource="http://www.ease-crc.org/ont/SOMA.owl#Box"/>
        <rdfs:subClassOf>
            <owl:Restriction>
                <owl:onProperty rdf:resource="http://www.ease-crc.org/ont/SUTURO.owl#hasPredefinedName"/>
                <owl:hasValue>tea bag box</owl:hasValue>
            </owl:Restriction>
        </rdfs:subClassOf>
        <SUTURO:perceptionId rdf:datatype="http://www.w3.org/2001/XMLSchema#int">73</SUTURO:perceptionId>
        <rdfs:comment>A tea bag box is a container used for storing and organizing tea bags, typically made of cardboard or other durable materials and featuring separate compartments for different types or flavors of tea. These boxes are commonly used in households, offices, and restaurants to keep tea bags readily available for brewing.</rdfs:comment>
        <rdfs:isDefinedBy rdf:resource="http://www.ease-crc.org/ont/SUTURO.owl"/>
    </owl:Class>
    


    <!-- http://www.ease-crc.org/ont/SUTURO.owl#TennisBall -->

    <owl:Class rdf:about="http://www.ease-crc.org/ont/SUTURO.owl#TennisBall">
        <rdfs:subClassOf rdf:resource="http://www.ease-crc.org/ont/SUTURO.owl#Ball"/>
        <rdfs:subClassOf rdf:resource="http://www.ease-crc.org/ont/SUTURO.owl#RoboCupToys"/>
        <rdfs:subClassOf>
            <owl:Restriction>
                <owl:onProperty rdf:resource="http://www.ease-crc.org/ont/SUTURO.owl#hasPredefinedName"/>
                <owl:hasValue>tennis ball</owl:hasValue>
            </owl:Restriction>
        </rdfs:subClassOf>
        <SUTURO:perceptionId rdf:datatype="http://www.w3.org/2001/XMLSchema#int">39</SUTURO:perceptionId>
        <rdfs:comment>A tennis ball is a small, round ball made of rubber with a fuzzy, felt-like outer layer, used in the sport of tennis, as well as in other games, such as fetch for dogs.</rdfs:comment>
        <rdfs:isDefinedBy rdf:resource="http://www.ease-crc.org/ont/SUTURO.owl"/>
    </owl:Class>
    


    <!-- http://www.ease-crc.org/ont/SUTURO.owl#TicTac -->

    <owl:Class rdf:about="http://www.ease-crc.org/ont/SUTURO.owl#TicTac">
        <rdfs:subClassOf rdf:resource="http://www.ease-crc.org/ont/SUTURO.owl#Sweets"/>
        <rdfs:subClassOf>
            <owl:Restriction>
                <owl:onProperty rdf:resource="http://www.ease-crc.org/ont/SUTURO.owl#hasPredefinedName"/>
                <owl:hasValue>tictac</owl:hasValue>
            </owl:Restriction>
        </rdfs:subClassOf>
        <SUTURO:perceptionId rdf:datatype="http://www.w3.org/2001/XMLSchema#decimal">126</SUTURO:perceptionId>
        <rdfs:isDefinedBy rdf:resource="http://www.ease-crc.org/ont/SUTURO.owl"/>
    </owl:Class>
    


    <!-- http://www.ease-crc.org/ont/SUTURO.owl#Tie -->

    <owl:Class rdf:about="http://www.ease-crc.org/ont/SUTURO.owl#Tie">
        <rdfs:subClassOf rdf:resource="http://www.ease-crc.org/ont/SUTURO.owl#Clothing"/>
        <rdfs:subClassOf>
            <owl:Restriction>
                <owl:onProperty rdf:resource="http://www.ease-crc.org/ont/SUTURO.owl#hasPredefinedName"/>
                <owl:hasValue>tie</owl:hasValue>
            </owl:Restriction>
        </rdfs:subClassOf>
        <rdfs:isDefinedBy rdf:resource="http://www.ease-crc.org/ont/SUTURO.owl"/>
    </owl:Class>
    


    <!-- http://www.ease-crc.org/ont/SUTURO.owl#TigerCup -->

    <owl:Class rdf:about="http://www.ease-crc.org/ont/SUTURO.owl#TigerCup">
        <rdfs:subClassOf rdf:resource="http://www.ease-crc.org/ont/SOMA.owl#Cup"/>
        <rdfs:subClassOf>
            <owl:Restriction>
                <owl:onProperty rdf:resource="http://www.ease-crc.org/ont/SUTURO.owl#hasPredefinedName"/>
                <owl:hasValue>tiger cup</owl:hasValue>
            </owl:Restriction>
        </rdfs:subClassOf>
        <rdfs:isDefinedBy rdf:resource="http://www.ease-crc.org/ont/SUTURO.owl"/>
    </owl:Class>
    


    <!-- http://www.ease-crc.org/ont/SUTURO.owl#Timer -->

    <owl:Class rdf:about="http://www.ease-crc.org/ont/SUTURO.owl#Timer">
        <rdfs:subClassOf rdf:resource="http://www.ease-crc.org/ont/SUTURO.owl#HouseholdHardware"/>
        <rdfs:subClassOf>
            <owl:Restriction>
                <owl:onProperty rdf:resource="http://www.ease-crc.org/ont/SUTURO.owl#hasPredefinedName"/>
                <owl:hasValue>timer</owl:hasValue>
            </owl:Restriction>
        </rdfs:subClassOf>
        <rdfs:comment>A timer is a device used to measure and indicate the passing of a set amount of time.</rdfs:comment>
        <rdfs:isDefinedBy rdf:resource="http://www.ease-crc.org/ont/SUTURO.owl"/>
    </owl:Class>
    


    <!-- http://www.ease-crc.org/ont/SUTURO.owl#Toast -->

    <owl:Class rdf:about="http://www.ease-crc.org/ont/SUTURO.owl#Toast">
        <rdfs:subClassOf rdf:resource="http://www.ease-crc.org/ont/SOMA.owl#Bread"/>
        <rdfs:subClassOf>
            <owl:Restriction>
                <owl:onProperty rdf:resource="http://www.ease-crc.org/ont/SUTURO.owl#hasPredefinedName"/>
                <owl:hasValue>toast</owl:hasValue>
            </owl:Restriction>
        </rdfs:subClassOf>
        <rdfs:isDefinedBy rdf:resource="http://www.ease-crc.org/ont/SUTURO.owl"/>
    </owl:Class>
    


    <!-- http://www.ease-crc.org/ont/SUTURO.owl#Tomato -->

    <owl:Class rdf:about="http://www.ease-crc.org/ont/SUTURO.owl#Tomato">
        <rdfs:subClassOf rdf:resource="http://www.ease-crc.org/ont/SUTURO.owl#Vegetable"/>
        <rdfs:subClassOf>
            <owl:Restriction>
                <owl:onProperty rdf:resource="http://www.ease-crc.org/ont/SUTURO.owl#hasPredefinedName"/>
                <owl:hasValue>tomato</owl:hasValue>
            </owl:Restriction>
        </rdfs:subClassOf>
        <rdfs:comment>A tomato is a fruit that is commonly used as a culinary vegetable and is known for its juicy flesh, bright color, and versatile flavor.</rdfs:comment>
        <rdfs:isDefinedBy rdf:resource="http://www.ease-crc.org/ont/SUTURO.owl"/>
    </owl:Class>
    


    <!-- http://www.ease-crc.org/ont/SUTURO.owl#TomatoSoup -->

    <owl:Class rdf:about="http://www.ease-crc.org/ont/SUTURO.owl#TomatoSoup">
        <rdfs:subClassOf rdf:resource="http://www.ease-crc.org/ont/SUTURO.owl#Soup"/>
        <rdfs:subClassOf>
            <owl:Restriction>
                <owl:onProperty rdf:resource="http://www.ease-crc.org/ont/SUTURO.owl#hasPredefinedName"/>
                <owl:hasValue>tomato soup</owl:hasValue>
            </owl:Restriction>
        </rdfs:subClassOf>
        <rdfs:comment>Tomato soup is a type of soup made from tomatoes, typically with additional ingredients such as broth, cream, and spices. It is a popular comfort food that is enjoyed around the world and can be served hot or cold.</rdfs:comment>
        <rdfs:isDefinedBy rdf:resource="http://www.ease-crc.org/ont/SUTURO.owl"/>
    </owl:Class>
    


    <!-- http://www.ease-crc.org/ont/SUTURO.owl#TomatoSoupCan -->

    <owl:Class rdf:about="http://www.ease-crc.org/ont/SUTURO.owl#TomatoSoupCan">
        <rdfs:subClassOf rdf:resource="http://www.ease-crc.org/ont/SUTURO.owl#RoboCupFood"/>
        <rdfs:subClassOf rdf:resource="http://www.ease-crc.org/ont/SUTURO.owl#SoupCan"/>
        <rdfs:subClassOf>
            <owl:Restriction>
                <owl:onProperty rdf:resource="http://www.ease-crc.org/ont/SUTURO.owl#hasPredefinedName"/>
                <owl:hasValue>tomato soup can</owl:hasValue>
            </owl:Restriction>
        </rdfs:subClassOf>
        <SUTURO:perceptionId rdf:datatype="http://www.w3.org/2001/XMLSchema#int">67</SUTURO:perceptionId>
        <rdfs:comment>Tomato soup can refers to a cylindrical metal container that holds condensed or ready-to-eat tomato soup.</rdfs:comment>
        <rdfs:isDefinedBy rdf:resource="http://www.ease-crc.org/ont/SUTURO.owl"/>
    </owl:Class>
    


    <!-- http://www.ease-crc.org/ont/SUTURO.owl#Toothpaste -->

    <owl:Class rdf:about="http://www.ease-crc.org/ont/SUTURO.owl#Toothpaste">
        <rdfs:subClassOf rdf:resource="http://www.ease-crc.org/ont/SUTURO.owl#HygieneProduct"/>
        <rdfs:subClassOf>
            <owl:Restriction>
                <owl:onProperty rdf:resource="http://www.ease-crc.org/ont/SUTURO.owl#hasPredefinedName"/>
                <owl:hasValue>toothpaste</owl:hasValue>
            </owl:Restriction>
        </rdfs:subClassOf>
        <SUTURO:perceptionId rdf:datatype="http://www.w3.org/2001/XMLSchema#int">64</SUTURO:perceptionId>
        <rdfs:comment>Toothpaste is a gel or paste used for cleaning teeth and maintaining oral hygiene. It typically contains abrasives, fluoride, and other active ingredients that help remove plaque, prevent tooth decay, and freshen breath.</rdfs:comment>
        <rdfs:isDefinedBy rdf:resource="http://www.ease-crc.org/ont/SUTURO.owl"/>
    </owl:Class>
    


    <!-- http://www.ease-crc.org/ont/SUTURO.owl#ToothpasteTube -->

    <owl:Class rdf:about="http://www.ease-crc.org/ont/SUTURO.owl#ToothpasteTube">
        <rdfs:subClassOf rdf:resource="http://www.ease-crc.org/ont/SUTURO.owl#Tube"/>
        <rdfs:comment>A toothpaste tube is a soft plastic or aluminum container that holds toothpaste for brushing teeth. The tube is typically sealed with a screw-on cap or flip-top lid and is squeezed to dispense the toothpaste.</rdfs:comment>
        <rdfs:isDefinedBy rdf:resource="http://www.ease-crc.org/ont/SUTURO.owl"/>
    </owl:Class>
    


    <!-- http://www.ease-crc.org/ont/SUTURO.owl#Towel -->

    <owl:Class rdf:about="http://www.ease-crc.org/ont/SUTURO.owl#Towel">
        <rdfs:subClassOf rdf:resource="http://www.ease-crc.org/ont/SUTURO.owl#DesignedFabric"/>
        <rdfs:subClassOf>
            <owl:Restriction>
                <owl:onProperty rdf:resource="http://www.ease-crc.org/ont/SUTURO.owl#hasPredefinedName"/>
                <owl:hasValue>towel</owl:hasValue>
            </owl:Restriction>
        </rdfs:subClassOf>
        <rdfs:isDefinedBy rdf:resource="http://www.ease-crc.org/ont/SUTURO.owl"/>
    </owl:Class>
    


    <!-- http://www.ease-crc.org/ont/SUTURO.owl#Toy -->

    <owl:Class rdf:about="http://www.ease-crc.org/ont/SUTURO.owl#Toy">
        <rdfs:subClassOf rdf:resource="http://www.ease-crc.org/ont/SOMA.owl#DesignedTool"/>
        <rdfs:comment>A toy is an object designed for children or adults to play with, often for amusement or education, and can range from simple objects to complex electronic devices.</rdfs:comment>
        <rdfs:isDefinedBy rdf:resource="http://www.ease-crc.org/ont/SUTURO.owl"/>
    </owl:Class>
    


    <!-- http://www.ease-crc.org/ont/SUTURO.owl#ToyAirplane -->

    <owl:Class rdf:about="http://www.ease-crc.org/ont/SUTURO.owl#ToyAirplane">
        <rdfs:subClassOf rdf:resource="http://www.ease-crc.org/ont/SUTURO.owl#Toy"/>
        <rdfs:subClassOf>
            <owl:Restriction>
                <owl:onProperty rdf:resource="http://www.ease-crc.org/ont/SUTURO.owl#hasPredefinedName"/>
                <owl:hasValue>toy airplane</owl:hasValue>
            </owl:Restriction>
        </rdfs:subClassOf>
        <rdfs:comment>A toy airplane is a miniature version of an airplane designed for children to play with.</rdfs:comment>
        <rdfs:isDefinedBy rdf:resource="http://www.ease-crc.org/ont/SUTURO.owl"/>
    </owl:Class>
    


    <!-- http://www.ease-crc.org/ont/SUTURO.owl#ToyotaHSR -->

    <owl:Class rdf:about="http://www.ease-crc.org/ont/SUTURO.owl#ToyotaHSR">
        <rdfs:subClassOf rdf:resource="http://knowrob.org/kb/urdf.owl#Robot"/>
        <rdfs:subClassOf>
            <owl:Restriction>
                <owl:onProperty rdf:resource="http://www.ease-crc.org/ont/SUTURO.owl#hasPredefinedName"/>
                <owl:hasValue>toyota HSR</owl:hasValue>
            </owl:Restriction>
        </rdfs:subClassOf>
        <SUTURO:perceptionId rdf:datatype="http://www.w3.org/2001/XMLSchema#int">61</SUTURO:perceptionId>
        <rdfs:comment>Toyota&apos;s HSR is a compact mobile cobot (collaborative robot) platform that can move around and fetch objects using a multi-DOF arm while avoiding obstacles. Operable by voice command or by tablet PC, HSR has a highly maneuverable, compact, and lightweight cylindrical body with a folding arm that enables it to pick up objects off the floor, suction up thin objects, retrieve objects from high locations, open curtains, and perform other household tasks.</rdfs:comment>
        <rdfs:isDefinedBy rdf:resource="http://www.ease-crc.org/ont/SUTURO.owl"/>
    </owl:Class>
    


    <!-- http://www.ease-crc.org/ont/SUTURO.owl#TrashBag -->

    <owl:Class rdf:about="http://www.ease-crc.org/ont/SUTURO.owl#TrashBag">
        <rdfs:subClassOf rdf:resource="http://www.ease-crc.org/ont/SOMA.owl#TrashContainer"/>
        <rdfs:comment>A bag made of plastic or other materials that is used to contain waste material.</rdfs:comment>
        <rdfs:isDefinedBy rdf:resource="http://www.ease-crc.org/ont/SUTURO.owl"/>
    </owl:Class>
    


    <!-- http://www.ease-crc.org/ont/SUTURO.owl#TrashBin -->

    <owl:Class rdf:about="http://www.ease-crc.org/ont/SUTURO.owl#TrashBin">
        <rdfs:subClassOf rdf:resource="http://www.ease-crc.org/ont/SOMA.owl#TrashContainer"/>
        <rdfs:subClassOf>
            <owl:Restriction>
                <owl:onProperty rdf:resource="http://www.ease-crc.org/ont/SUTURO.owl#hasPredefinedName"/>
                <owl:hasValue>trash bin</owl:hasValue>
            </owl:Restriction>
        </rdfs:subClassOf>
        <SUTURO:perceptionId rdf:datatype="http://www.w3.org/2001/XMLSchema#int">0</SUTURO:perceptionId>
        <rdfs:comment>A container for holding waste or garbage.</rdfs:comment>
        <rdfs:isDefinedBy rdf:resource="http://www.ease-crc.org/ont/SUTURO.owl"/>
    </owl:Class>
    


    <!-- http://www.ease-crc.org/ont/SUTURO.owl#Tray -->

    <owl:Class rdf:about="http://www.ease-crc.org/ont/SUTURO.owl#Tray">
        <rdfs:subClassOf rdf:resource="http://www.ease-crc.org/ont/SUTURO.owl#HouseholdHardware"/>
        <rdfs:subClassOf>
            <owl:Restriction>
                <owl:onProperty rdf:resource="http://www.ease-crc.org/ont/SUTURO.owl#hasPredefinedName"/>
                <owl:hasValue>tray</owl:hasValue>
            </owl:Restriction>
        </rdfs:subClassOf>
        <SUTURO:perceptionId rdf:datatype="http://www.w3.org/2001/XMLSchema#int">26</SUTURO:perceptionId>
        <rdfs:comment>A flat, shallow container with a raised rim, typically used for carrying food and drink, or for holding small items or loose material.</rdfs:comment>
        <rdfs:isDefinedBy rdf:resource="http://www.ease-crc.org/ont/SUTURO.owl"/>
    </owl:Class>
    


    <!-- http://www.ease-crc.org/ont/SUTURO.owl#TropicalJuice -->

    <owl:Class rdf:about="http://www.ease-crc.org/ont/SUTURO.owl#TropicalJuice">
        <rdfs:subClassOf rdf:resource="http://www.ease-crc.org/ont/SUTURO.owl#Juice"/>
        <rdfs:subClassOf>
            <owl:Restriction>
                <owl:onProperty rdf:resource="http://www.ease-crc.org/ont/SUTURO.owl#hasPredefinedName"/>
                <owl:hasValue>tropical juice</owl:hasValue>
            </owl:Restriction>
        </rdfs:subClassOf>
    </owl:Class>
    


    <!-- http://www.ease-crc.org/ont/SUTURO.owl#TropicalJuiceBottle -->

    <owl:Class rdf:about="http://www.ease-crc.org/ont/SUTURO.owl#TropicalJuiceBottle">
        <rdfs:subClassOf rdf:resource="http://www.ease-crc.org/ont/SUTURO.owl#JuiceBottle"/>
        <rdfs:subClassOf rdf:resource="http://www.ease-crc.org/ont/SUTURO.owl#RoboCupDrinks"/>
        <rdfs:subClassOf>
            <owl:Restriction>
                <owl:onProperty rdf:resource="http://www.ease-crc.org/ont/SUTURO.owl#hasPredefinedName"/>
                <owl:hasValue>tropical juice bottle</owl:hasValue>
            </owl:Restriction>
        </rdfs:subClassOf>
        <SUTURO:perceptionId rdf:datatype="http://www.w3.org/2001/XMLSchema#int">84</SUTURO:perceptionId>
        <rdfs:comment>A tropical juice bottle is a container, typically made of plastic or glass, specifically designed to store and dispense juices made from tropical fruits. It usually features a screw-top or snap cap for freshness and ease of use, and is popular for its portability, making it suitable for on-the-go consumption.</rdfs:comment>
        <rdfs:isDefinedBy rdf:resource="http://www.ease-crc.org/ont/SUTURO.owl"/>
    </owl:Class>
    


    <!-- http://www.ease-crc.org/ont/SUTURO.owl#Trousers -->

    <owl:Class rdf:about="http://www.ease-crc.org/ont/SUTURO.owl#Trousers">
        <rdfs:subClassOf rdf:resource="http://www.ease-crc.org/ont/SUTURO.owl#Clothing"/>
        <rdfs:subClassOf>
            <owl:Restriction>
                <owl:onProperty rdf:resource="http://www.ease-crc.org/ont/SUTURO.owl#hasPredefinedName"/>
                <owl:hasValue>trousers</owl:hasValue>
            </owl:Restriction>
        </rdfs:subClassOf>
        <rdfs:isDefinedBy rdf:resource="http://www.ease-crc.org/ont/SUTURO.owl"/>
    </owl:Class>
    


    <!-- http://www.ease-crc.org/ont/SUTURO.owl#Tshirt -->

    <owl:Class rdf:about="http://www.ease-crc.org/ont/SUTURO.owl#Tshirt">
        <rdfs:subClassOf rdf:resource="http://www.ease-crc.org/ont/SUTURO.owl#Clothing"/>
        <rdfs:subClassOf>
            <owl:Restriction>
                <owl:onProperty rdf:resource="http://www.ease-crc.org/ont/SUTURO.owl#hasPredefinedName"/>
                <owl:hasValue>t-shirt</owl:hasValue>
            </owl:Restriction>
        </rdfs:subClassOf>
        <rdfs:comment>A T-shirt is a type of unisex fabric shirt named after the T shape of its body and sleeves. It is typically made of cotton and features short sleeves and a round neckline. It is a casual and comfortable piece of clothing that is often worn for everyday activities.</rdfs:comment>
        <rdfs:isDefinedBy rdf:resource="http://www.ease-crc.org/ont/SUTURO.owl"/>
    </owl:Class>
    


    <!-- http://www.ease-crc.org/ont/SUTURO.owl#Tube -->

    <owl:Class rdf:about="http://www.ease-crc.org/ont/SUTURO.owl#Tube">
        <rdfs:subClassOf rdf:resource="http://www.ease-crc.org/ont/SOMA.owl#DesignedContainer"/>
        <rdfs:comment>A tube is a cylindrical container made of plastic, metal, or other materials that is used to hold and dispense a product such as toothpaste, lotion, or paint. Tubes are typically sealed at one end and have an opening at the other end for dispensing the product.</rdfs:comment>
        <rdfs:isDefinedBy rdf:resource="http://www.ease-crc.org/ont/SUTURO.owl"/>
    </owl:Class>
    


    <!-- http://www.ease-crc.org/ont/SUTURO.owl#Tuna -->

    <owl:Class rdf:about="http://www.ease-crc.org/ont/SUTURO.owl#Tuna">
        <rdfs:subClassOf rdf:resource="http://www.ease-crc.org/ont/SUTURO.owl#Fish"/>
        <rdfs:subClassOf>
            <owl:Restriction>
                <owl:onProperty rdf:resource="http://www.ease-crc.org/ont/SUTURO.owl#hasPredefinedName"/>
                <owl:hasValue>tuna</owl:hasValue>
            </owl:Restriction>
        </rdfs:subClassOf>
        <rdfs:comment>Tuna is a saltwater fish that belongs to the mackerel family. It is a popular seafood item and is commonly used in a variety of dishes such as sushi, salads, and sandwiches.</rdfs:comment>
        <rdfs:isDefinedBy rdf:resource="http://www.ease-crc.org/ont/SUTURO.owl"/>
    </owl:Class>
    


    <!-- http://www.ease-crc.org/ont/SUTURO.owl#TunaFishCan -->

    <owl:Class rdf:about="http://www.ease-crc.org/ont/SUTURO.owl#TunaFishCan">
        <rdfs:subClassOf rdf:resource="http://www.ease-crc.org/ont/SUTURO.owl#Can"/>
        <rdfs:subClassOf rdf:resource="http://www.ease-crc.org/ont/SUTURO.owl#RoboCupFood"/>
        <rdfs:subClassOf>
            <owl:Restriction>
                <owl:onProperty rdf:resource="http://www.ease-crc.org/ont/SUTURO.owl#hasPredefinedName"/>
                <owl:hasValue>tuna fish can</owl:hasValue>
            </owl:Restriction>
        </rdfs:subClassOf>
        <SUTURO:perceptionId rdf:datatype="http://www.w3.org/2001/XMLSchema#int">68</SUTURO:perceptionId>
        <rdfs:comment>Tuna fish can refers to a metal container used to store and preserve tuna fish.</rdfs:comment>
        <rdfs:isDefinedBy rdf:resource="http://www.ease-crc.org/ont/SUTURO.owl"/>
    </owl:Class>
    


    <!-- http://www.ease-crc.org/ont/SUTURO.owl#Vegetable -->

    <owl:Class rdf:about="http://www.ease-crc.org/ont/SUTURO.owl#Vegetable">
        <rdfs:subClassOf rdf:resource="http://www.ease-crc.org/ont/SUTURO.owl#Food"/>
        <rdfs:subClassOf>
            <owl:Restriction>
                <owl:onProperty rdf:resource="http://www.ease-crc.org/ont/SUTURO.owl#hasPredefinedName"/>
                <owl:hasValue>vegetable</owl:hasValue>
            </owl:Restriction>
        </rdfs:subClassOf>
        <rdfs:comment>A vegetable is a plant or part of a plant that is typically eaten as food and is not classified as a fruit, seed, or spice.</rdfs:comment>
        <rdfs:isDefinedBy rdf:resource="http://www.ease-crc.org/ont/SUTURO.owl"/>
    </owl:Class>
    


    <!-- http://www.ease-crc.org/ont/SUTURO.owl#Vest -->

    <owl:Class rdf:about="http://www.ease-crc.org/ont/SUTURO.owl#Vest">
        <rdfs:subClassOf rdf:resource="http://www.ease-crc.org/ont/SUTURO.owl#Clothing"/>
        <rdfs:subClassOf>
            <owl:Restriction>
                <owl:onProperty rdf:resource="http://www.ease-crc.org/ont/SUTURO.owl#hasPredefinedName"/>
                <owl:hasValue>vest</owl:hasValue>
            </owl:Restriction>
        </rdfs:subClassOf>
        <rdfs:isDefinedBy rdf:resource="http://www.ease-crc.org/ont/SUTURO.owl"/>
    </owl:Class>
    


    <!-- http://www.ease-crc.org/ont/SUTURO.owl#WashCloth -->

    <owl:Class rdf:about="http://www.ease-crc.org/ont/SUTURO.owl#WashCloth">
        <rdfs:subClassOf rdf:resource="http://www.ease-crc.org/ont/SUTURO.owl#CleaningTool"/>
        <rdfs:subClassOf rdf:resource="http://www.ease-crc.org/ont/SUTURO.owl#RoboCupCleaningSupplies"/>
        <rdfs:subClassOf>
            <owl:Restriction>
                <owl:onProperty rdf:resource="http://www.ease-crc.org/ont/SUTURO.owl#hasPredefinedName"/>
                <owl:hasValue>washcloth</owl:hasValue>
            </owl:Restriction>
        </rdfs:subClassOf>
        <SUTURO:perceptionId rdf:datatype="http://www.w3.org/2001/XMLSchema#decimal">108</SUTURO:perceptionId>
        <rdfs:isDefinedBy rdf:resource="http://www.ease-crc.org/ont/SUTURO.owl"/>
    </owl:Class>
    


    <!-- http://www.ease-crc.org/ont/SUTURO.owl#Washer -->

    <owl:Class rdf:about="http://www.ease-crc.org/ont/SUTURO.owl#Washer">
        <rdfs:subClassOf rdf:resource="http://www.ease-crc.org/ont/SUTURO.owl#MetalHardware"/>
        <rdfs:subClassOf>
            <owl:Restriction>
                <owl:onProperty rdf:resource="http://www.ease-crc.org/ont/SUTURO.owl#hasPredefinedName"/>
                <owl:hasValue>washer</owl:hasValue>
            </owl:Restriction>
        </rdfs:subClassOf>
        <SUTURO:perceptionId rdf:datatype="http://www.w3.org/2001/XMLSchema#int">14</SUTURO:perceptionId>
        <rdfs:comment>A washer is a thin, flat ring-shaped object, typically made of metal, rubber, or plastic, used to distribute the load of a threaded fastener such as a screw or bolt, or as a spacer, seal, or locking device.</rdfs:comment>
        <rdfs:isDefinedBy rdf:resource="http://www.ease-crc.org/ont/SUTURO.owl"/>
    </owl:Class>
    


    <!-- http://www.ease-crc.org/ont/SUTURO.owl#Water -->

    <owl:Class rdf:about="http://www.ease-crc.org/ont/SUTURO.owl#Water">
        <rdfs:subClassOf rdf:resource="http://www.ease-crc.org/ont/SUTURO.owl#Drink"/>
        <rdfs:subClassOf rdf:resource="http://www.ease-crc.org/ont/SUTURO.owl#RoboCupDrinks"/>
    </owl:Class>
    


    <!-- http://www.ease-crc.org/ont/SUTURO.owl#WaterBottle -->

    <owl:Class rdf:about="http://www.ease-crc.org/ont/SUTURO.owl#WaterBottle">
        <rdfs:subClassOf rdf:resource="http://www.ease-crc.org/ont/SUTURO.owl#Drink"/>
        <rdfs:subClassOf rdf:resource="http://www.ease-crc.org/ont/SUTURO.owl#RoboCupDrinks"/>
        <rdfs:subClassOf rdf:resource="http://www.ease-crc.org/ont/SUTURO.owl#Water"/>
        <rdfs:subClassOf>
            <owl:Restriction>
                <owl:onProperty rdf:resource="http://www.ease-crc.org/ont/SUTURO.owl#hasPredefinedName"/>
                <owl:hasValue>water</owl:hasValue>
            </owl:Restriction>
        </rdfs:subClassOf>
        <SUTURO:perceptionId rdf:datatype="http://www.w3.org/2001/XMLSchema#decimal">113</SUTURO:perceptionId>
        <rdfs:isDefinedBy rdf:resource="http://www.ease-crc.org/ont/SUTURO.owl"/>
    </owl:Class>
    


    <!-- http://www.ease-crc.org/ont/SUTURO.owl#Weight -->

    <owl:Class rdf:about="http://www.ease-crc.org/ont/SUTURO.owl#Weight">
        <rdfs:subClassOf rdf:resource="http://www.ease-crc.org/ont/SOMA.owl#Intrinsic"/>
        <rdfs:comment>Weight refers to the amount of force exerted on an object due to gravity, usually measured in units such as pounds or kilograms. It is a physical property that can change based on the location of the object and the gravitational force acting upon it.</rdfs:comment>
        <rdfs:isDefinedBy rdf:resource="http://www.ease-crc.org/ont/SUTURO.owl"/>
    </owl:Class>
    


    <!-- http://www.ease-crc.org/ont/SUTURO.owl#WoodBlock -->

    <owl:Class rdf:about="http://www.ease-crc.org/ont/SUTURO.owl#WoodBlock">
        <rdfs:subClassOf rdf:resource="http://www.ease-crc.org/ont/SUTURO.owl#Block"/>
        <rdfs:subClassOf>
            <owl:Restriction>
                <owl:onProperty rdf:resource="http://www.ease-crc.org/ont/SUTURO.owl#hasPredefinedName"/>
                <owl:hasValue>wood block</owl:hasValue>
            </owl:Restriction>
        </rdfs:subClassOf>
        <SUTURO:perceptionId rdf:datatype="http://www.w3.org/2001/XMLSchema#decimal">105</SUTURO:perceptionId>
        <rdfs:comment>A wood block is a solid piece of wood cut into a rectangular or square shape, used for carving, chopping, or as a decorative item.</rdfs:comment>
        <rdfs:isDefinedBy rdf:resource="http://www.ease-crc.org/ont/SUTURO.owl"/>
    </owl:Class>
    


    <!-- http://www.ease-crc.org/ont/SUTURO.owl#Wrench -->

    <owl:Class rdf:about="http://www.ease-crc.org/ont/SUTURO.owl#Wrench">
        <rdfs:subClassOf rdf:resource="http://www.ease-crc.org/ont/SUTURO.owl#ForceConcentratingTool"/>
        <rdfs:subClassOf>
            <owl:Restriction>
                <owl:onProperty rdf:resource="http://www.ease-crc.org/ont/SOMA.owl#hasPhysicalComponent"/>
                <owl:someValuesFrom rdf:resource="http://www.ease-crc.org/ont/SOMA.owl#DesignedHandle"/>
            </owl:Restriction>
        </rdfs:subClassOf>
        <rdfs:comment>A wrench is a hand tool with a handle and adjustable jaws or a fixed socket used for gripping and turning nuts, bolts, and other fasteners.</rdfs:comment>
        <rdfs:isDefinedBy rdf:resource="http://www.ease-crc.org/ont/SUTURO.owl"/>
    </owl:Class>
    


    <!-- http://www.ease-crc.org/ont/SUTURO.owl#WritingTool -->

    <owl:Class rdf:about="http://www.ease-crc.org/ont/SUTURO.owl#WritingTool">
        <rdfs:subClassOf rdf:resource="http://www.ease-crc.org/ont/SOMA.owl#DesignedTool"/>
        <rdfs:subClassOf>
            <owl:Restriction>
                <owl:onProperty rdf:resource="http://www.ease-crc.org/ont/SUTURO.owl#hasPredefinedName"/>
                <owl:hasValue>writing tool</owl:hasValue>
            </owl:Restriction>
        </rdfs:subClassOf>
        <rdfs:comment>A writing tool is a device used to inscribe characters onto a surface, such as paper or digital media, and can include pens, pencils, markers, styluses, and digital pens.</rdfs:comment>
        <rdfs:isDefinedBy rdf:resource="http://www.ease-crc.org/ont/SUTURO.owl"/>
    </owl:Class>
    


    <!-- http://www.ease-crc.org/ont/SUTURO.owl#hasFavouriteDrink -->

    <owl:Class rdf:about="http://www.ease-crc.org/ont/SUTURO.owl#hasFavouriteDrink">
        <rdfs:subClassOf rdf:resource="http://www.ease-crc.org/ont/SOMA.owl#Preference"/>
        <rdfs:comment> A preferred drink by a customer </rdfs:comment>
        <rdfs:isDefinedBy rdf:resource="http://www.ease-crc.org/ont/SUTURO.owl"/>
    </owl:Class>
    


    <!-- http://www.ontologydesignpatterns.org/ont/dul/DUL.owl#BiologicalObject -->

    <owl:Class rdf:about="http://www.ontologydesignpatterns.org/ont/dul/DUL.owl#BiologicalObject">
        <rdfs:comment>A biological object refers to any living entity, organism, or part thereof that is associated with biological systems or processes. It encompasses a wide range of living things, including plants, animals, microorganisms, cells, tissues, organs, and biological molecules, and is a fundamental concept in the field of biology.</rdfs:comment>
    </owl:Class>
    


    <!-- http://www.ontologydesignpatterns.org/ont/dul/DUL.owl#Collection -->

    <owl:Class rdf:about="http://www.ontologydesignpatterns.org/ont/dul/DUL.owl#Collection"/>
    


    <!-- http://www.ontologydesignpatterns.org/ont/dul/DUL.owl#DesignedArtifact -->

    <owl:Class rdf:about="http://www.ontologydesignpatterns.org/ont/dul/DUL.owl#DesignedArtifact"/>
    


    <!-- http://www.ontologydesignpatterns.org/ont/dul/DUL.owl#DesignedSubstance -->

    <owl:Class rdf:about="http://www.ontologydesignpatterns.org/ont/dul/DUL.owl#DesignedSubstance"/>
    


    <!-- http://www.ontologydesignpatterns.org/ont/dul/DUL.owl#Entity -->

    <owl:Class rdf:about="http://www.ontologydesignpatterns.org/ont/dul/DUL.owl#Entity"/>
    


    <!-- http://www.ontologydesignpatterns.org/ont/dul/DUL.owl#NaturalPerson -->

    <owl:Class rdf:about="http://www.ontologydesignpatterns.org/ont/dul/DUL.owl#NaturalPerson">
        <rdfs:subClassOf>
            <owl:Restriction>
                <owl:onProperty rdf:resource="http://www.ease-crc.org/ont/SUTURO.owl#hasPredefinedName"/>
                <owl:hasValue>Adel</owl:hasValue>
            </owl:Restriction>
        </rdfs:subClassOf>
        <rdfs:subClassOf>
            <owl:Restriction>
                <owl:onProperty rdf:resource="http://www.ease-crc.org/ont/SUTURO.owl#hasPredefinedName"/>
                <owl:hasValue>Alice</owl:hasValue>
            </owl:Restriction>
        </rdfs:subClassOf>
        <rdfs:subClassOf>
            <owl:Restriction>
                <owl:onProperty rdf:resource="http://www.ease-crc.org/ont/SUTURO.owl#hasPredefinedName"/>
                <owl:hasValue>Amanda</owl:hasValue>
            </owl:Restriction>
        </rdfs:subClassOf>
        <rdfs:subClassOf>
            <owl:Restriction>
                <owl:onProperty rdf:resource="http://www.ease-crc.org/ont/SUTURO.owl#hasPredefinedName"/>
                <owl:hasValue>Andrew</owl:hasValue>
            </owl:Restriction>
        </rdfs:subClassOf>
        <rdfs:subClassOf>
            <owl:Restriction>
                <owl:onProperty rdf:resource="http://www.ease-crc.org/ont/SUTURO.owl#hasPredefinedName"/>
                <owl:hasValue>Angel</owl:hasValue>
            </owl:Restriction>
        </rdfs:subClassOf>
        <rdfs:subClassOf>
            <owl:Restriction>
                <owl:onProperty rdf:resource="http://www.ease-crc.org/ont/SUTURO.owl#hasPredefinedName"/>
                <owl:hasValue>Ashley</owl:hasValue>
            </owl:Restriction>
        </rdfs:subClassOf>
        <rdfs:subClassOf>
            <owl:Restriction>
                <owl:onProperty rdf:resource="http://www.ease-crc.org/ont/SUTURO.owl#hasPredefinedName"/>
                <owl:hasValue>Axel</owl:hasValue>
            </owl:Restriction>
        </rdfs:subClassOf>
        <rdfs:subClassOf>
            <owl:Restriction>
                <owl:onProperty rdf:resource="http://www.ease-crc.org/ont/SUTURO.owl#hasPredefinedName"/>
                <owl:hasValue>Bob</owl:hasValue>
            </owl:Restriction>
        </rdfs:subClassOf>
        <rdfs:subClassOf>
            <owl:Restriction>
                <owl:onProperty rdf:resource="http://www.ease-crc.org/ont/SUTURO.owl#hasPredefinedName"/>
                <owl:hasValue>Brittany</owl:hasValue>
            </owl:Restriction>
        </rdfs:subClassOf>
        <rdfs:subClassOf>
            <owl:Restriction>
                <owl:onProperty rdf:resource="http://www.ease-crc.org/ont/SUTURO.owl#hasPredefinedName"/>
                <owl:hasValue>Charlie</owl:hasValue>
            </owl:Restriction>
        </rdfs:subClassOf>
        <rdfs:subClassOf>
            <owl:Restriction>
                <owl:onProperty rdf:resource="http://www.ease-crc.org/ont/SUTURO.owl#hasPredefinedName"/>
                <owl:hasValue>Christopher</owl:hasValue>
            </owl:Restriction>
        </rdfs:subClassOf>
        <rdfs:subClassOf>
            <owl:Restriction>
                <owl:onProperty rdf:resource="http://www.ease-crc.org/ont/SUTURO.owl#hasPredefinedName"/>
                <owl:hasValue>Daniel</owl:hasValue>
            </owl:Restriction>
        </rdfs:subClassOf>
        <rdfs:subClassOf>
            <owl:Restriction>
                <owl:onProperty rdf:resource="http://www.ease-crc.org/ont/SUTURO.owl#hasPredefinedName"/>
                <owl:hasValue>David</owl:hasValue>
            </owl:Restriction>
        </rdfs:subClassOf>
        <rdfs:subClassOf>
            <owl:Restriction>
                <owl:onProperty rdf:resource="http://www.ease-crc.org/ont/SUTURO.owl#hasPredefinedName"/>
                <owl:hasValue>Elizabeth</owl:hasValue>
            </owl:Restriction>
        </rdfs:subClassOf>
        <rdfs:subClassOf>
            <owl:Restriction>
                <owl:onProperty rdf:resource="http://www.ease-crc.org/ont/SUTURO.owl#hasPredefinedName"/>
                <owl:hasValue>Emma</owl:hasValue>
            </owl:Restriction>
        </rdfs:subClassOf>
        <rdfs:subClassOf>
            <owl:Restriction>
                <owl:onProperty rdf:resource="http://www.ease-crc.org/ont/SUTURO.owl#hasPredefinedName"/>
                <owl:hasValue>Fleur</owl:hasValue>
            </owl:Restriction>
        </rdfs:subClassOf>
        <rdfs:subClassOf>
            <owl:Restriction>
                <owl:onProperty rdf:resource="http://www.ease-crc.org/ont/SUTURO.owl#hasPredefinedName"/>
                <owl:hasValue>Gabrielle</owl:hasValue>
            </owl:Restriction>
        </rdfs:subClassOf>
        <rdfs:subClassOf>
            <owl:Restriction>
                <owl:onProperty rdf:resource="http://www.ease-crc.org/ont/SUTURO.owl#hasPredefinedName"/>
                <owl:hasValue>Harrie</owl:hasValue>
            </owl:Restriction>
        </rdfs:subClassOf>
        <rdfs:subClassOf>
            <owl:Restriction>
                <owl:onProperty rdf:resource="http://www.ease-crc.org/ont/SUTURO.owl#hasPredefinedName"/>
                <owl:hasValue>Hayley</owl:hasValue>
            </owl:Restriction>
        </rdfs:subClassOf>
        <rdfs:subClassOf>
            <owl:Restriction>
                <owl:onProperty rdf:resource="http://www.ease-crc.org/ont/SUTURO.owl#hasPredefinedName"/>
                <owl:hasValue>James</owl:hasValue>
            </owl:Restriction>
        </rdfs:subClassOf>
        <rdfs:subClassOf>
            <owl:Restriction>
                <owl:onProperty rdf:resource="http://www.ease-crc.org/ont/SUTURO.owl#hasPredefinedName"/>
                <owl:hasValue>Jane</owl:hasValue>
            </owl:Restriction>
        </rdfs:subClassOf>
        <rdfs:subClassOf>
            <owl:Restriction>
                <owl:onProperty rdf:resource="http://www.ease-crc.org/ont/SUTURO.owl#hasPredefinedName"/>
                <owl:hasValue>Jennifer</owl:hasValue>
            </owl:Restriction>
        </rdfs:subClassOf>
        <rdfs:subClassOf>
            <owl:Restriction>
                <owl:onProperty rdf:resource="http://www.ease-crc.org/ont/SUTURO.owl#hasPredefinedName"/>
                <owl:hasValue>Jesse</owl:hasValue>
            </owl:Restriction>
        </rdfs:subClassOf>
        <rdfs:subClassOf>
            <owl:Restriction>
                <owl:onProperty rdf:resource="http://www.ease-crc.org/ont/SUTURO.owl#hasPredefinedName"/>
                <owl:hasValue>Jessica</owl:hasValue>
            </owl:Restriction>
        </rdfs:subClassOf>
        <rdfs:subClassOf>
            <owl:Restriction>
                <owl:onProperty rdf:resource="http://www.ease-crc.org/ont/SUTURO.owl#hasPredefinedName"/>
                <owl:hasValue>John</owl:hasValue>
            </owl:Restriction>
        </rdfs:subClassOf>
        <rdfs:subClassOf>
            <owl:Restriction>
                <owl:onProperty rdf:resource="http://www.ease-crc.org/ont/SUTURO.owl#hasPredefinedName"/>
                <owl:hasValue>Joseph</owl:hasValue>
            </owl:Restriction>
        </rdfs:subClassOf>
        <rdfs:subClassOf>
            <owl:Restriction>
                <owl:onProperty rdf:resource="http://www.ease-crc.org/ont/SUTURO.owl#hasPredefinedName"/>
                <owl:hasValue>Joshua</owl:hasValue>
            </owl:Restriction>
        </rdfs:subClassOf>
        <rdfs:subClassOf>
            <owl:Restriction>
                <owl:onProperty rdf:resource="http://www.ease-crc.org/ont/SUTURO.owl#hasPredefinedName"/>
                <owl:hasValue>Jules</owl:hasValue>
            </owl:Restriction>
        </rdfs:subClassOf>
        <rdfs:subClassOf>
            <owl:Restriction>
                <owl:onProperty rdf:resource="http://www.ease-crc.org/ont/SUTURO.owl#hasPredefinedName"/>
                <owl:hasValue>Julia</owl:hasValue>
            </owl:Restriction>
        </rdfs:subClassOf>
        <rdfs:subClassOf>
            <owl:Restriction>
                <owl:onProperty rdf:resource="http://www.ease-crc.org/ont/SUTURO.owl#hasPredefinedName"/>
                <owl:hasValue>Justin</owl:hasValue>
            </owl:Restriction>
        </rdfs:subClassOf>
        <rdfs:subClassOf>
            <owl:Restriction>
                <owl:onProperty rdf:resource="http://www.ease-crc.org/ont/SUTURO.owl#hasPredefinedName"/>
                <owl:hasValue>Kevin</owl:hasValue>
            </owl:Restriction>
        </rdfs:subClassOf>
        <rdfs:subClassOf>
            <owl:Restriction>
                <owl:onProperty rdf:resource="http://www.ease-crc.org/ont/SUTURO.owl#hasPredefinedName"/>
                <owl:hasValue>Laura</owl:hasValue>
            </owl:Restriction>
        </rdfs:subClassOf>
        <rdfs:subClassOf>
            <owl:Restriction>
                <owl:onProperty rdf:resource="http://www.ease-crc.org/ont/SUTURO.owl#hasPredefinedName"/>
                <owl:hasValue>Lauren</owl:hasValue>
            </owl:Restriction>
        </rdfs:subClassOf>
        <rdfs:subClassOf>
            <owl:Restriction>
                <owl:onProperty rdf:resource="http://www.ease-crc.org/ont/SUTURO.owl#hasPredefinedName"/>
                <owl:hasValue>Liam</owl:hasValue>
            </owl:Restriction>
        </rdfs:subClassOf>
        <rdfs:subClassOf>
            <owl:Restriction>
                <owl:onProperty rdf:resource="http://www.ease-crc.org/ont/SUTURO.owl#hasPredefinedName"/>
                <owl:hasValue>Lucas</owl:hasValue>
            </owl:Restriction>
        </rdfs:subClassOf>
        <rdfs:subClassOf>
            <owl:Restriction>
                <owl:onProperty rdf:resource="http://www.ease-crc.org/ont/SUTURO.owl#hasPredefinedName"/>
                <owl:hasValue>Matthew</owl:hasValue>
            </owl:Restriction>
        </rdfs:subClassOf>
        <rdfs:subClassOf>
            <owl:Restriction>
                <owl:onProperty rdf:resource="http://www.ease-crc.org/ont/SUTURO.owl#hasPredefinedName"/>
                <owl:hasValue>Michael</owl:hasValue>
            </owl:Restriction>
        </rdfs:subClassOf>
        <rdfs:subClassOf>
            <owl:Restriction>
                <owl:onProperty rdf:resource="http://www.ease-crc.org/ont/SUTURO.owl#hasPredefinedName"/>
                <owl:hasValue>Morgan</owl:hasValue>
            </owl:Restriction>
        </rdfs:subClassOf>
        <rdfs:subClassOf>
            <owl:Restriction>
                <owl:onProperty rdf:resource="http://www.ease-crc.org/ont/SUTURO.owl#hasPredefinedName"/>
                <owl:hasValue>Noah</owl:hasValue>
            </owl:Restriction>
        </rdfs:subClassOf>
        <rdfs:subClassOf>
            <owl:Restriction>
                <owl:onProperty rdf:resource="http://www.ease-crc.org/ont/SUTURO.owl#hasPredefinedName"/>
                <owl:hasValue>Paris</owl:hasValue>
            </owl:Restriction>
        </rdfs:subClassOf>
        <rdfs:subClassOf>
            <owl:Restriction>
                <owl:onProperty rdf:resource="http://www.ease-crc.org/ont/SUTURO.owl#hasPredefinedName"/>
                <owl:hasValue>Peter</owl:hasValue>
            </owl:Restriction>
        </rdfs:subClassOf>
        <rdfs:subClassOf>
            <owl:Restriction>
                <owl:onProperty rdf:resource="http://www.ease-crc.org/ont/SUTURO.owl#hasPredefinedName"/>
                <owl:hasValue>Robin</owl:hasValue>
            </owl:Restriction>
        </rdfs:subClassOf>
        <rdfs:subClassOf>
            <owl:Restriction>
                <owl:onProperty rdf:resource="http://www.ease-crc.org/ont/SUTURO.owl#hasPredefinedName"/>
                <owl:hasValue>Samantha</owl:hasValue>
            </owl:Restriction>
        </rdfs:subClassOf>
        <rdfs:subClassOf>
            <owl:Restriction>
                <owl:onProperty rdf:resource="http://www.ease-crc.org/ont/SUTURO.owl#hasPredefinedName"/>
                <owl:hasValue>Sara</owl:hasValue>
            </owl:Restriction>
        </rdfs:subClassOf>
        <rdfs:subClassOf>
            <owl:Restriction>
                <owl:onProperty rdf:resource="http://www.ease-crc.org/ont/SUTURO.owl#hasPredefinedName"/>
                <owl:hasValue>Sarah</owl:hasValue>
            </owl:Restriction>
        </rdfs:subClassOf>
        <rdfs:subClassOf>
            <owl:Restriction>
                <owl:onProperty rdf:resource="http://www.ease-crc.org/ont/SUTURO.owl#hasPredefinedName"/>
                <owl:hasValue>Simone</owl:hasValue>
            </owl:Restriction>
        </rdfs:subClassOf>
        <rdfs:subClassOf>
            <owl:Restriction>
                <owl:onProperty rdf:resource="http://www.ease-crc.org/ont/SUTURO.owl#hasPredefinedName"/>
                <owl:hasValue>Sophie</owl:hasValue>
            </owl:Restriction>
        </rdfs:subClassOf>
        <rdfs:subClassOf>
            <owl:Restriction>
                <owl:onProperty rdf:resource="http://www.ease-crc.org/ont/SUTURO.owl#hasPredefinedName"/>
                <owl:hasValue>Stephanie</owl:hasValue>
            </owl:Restriction>
        </rdfs:subClassOf>
        <rdfs:subClassOf>
            <owl:Restriction>
                <owl:onProperty rdf:resource="http://www.ease-crc.org/ont/SUTURO.owl#hasPredefinedName"/>
                <owl:hasValue>Susan</owl:hasValue>
            </owl:Restriction>
        </rdfs:subClassOf>
        <rdfs:subClassOf>
            <owl:Restriction>
                <owl:onProperty rdf:resource="http://www.ease-crc.org/ont/SUTURO.owl#hasPredefinedName"/>
                <owl:hasValue>William</owl:hasValue>
            </owl:Restriction>
        </rdfs:subClassOf>
        <rdfs:subClassOf>
            <owl:Restriction>
                <owl:onProperty rdf:resource="http://www.ease-crc.org/ont/SUTURO.owl#hasPredefinedName"/>
                <owl:hasValue>boy</owl:hasValue>
            </owl:Restriction>
        </rdfs:subClassOf>
        <rdfs:subClassOf>
            <owl:Restriction>
                <owl:onProperty rdf:resource="http://www.ease-crc.org/ont/SUTURO.owl#hasPredefinedName"/>
                <owl:hasValue>child</owl:hasValue>
            </owl:Restriction>
        </rdfs:subClassOf>
        <rdfs:subClassOf>
            <owl:Restriction>
                <owl:onProperty rdf:resource="http://www.ease-crc.org/ont/SUTURO.owl#hasPredefinedName"/>
                <owl:hasValue>dame</owl:hasValue>
            </owl:Restriction>
        </rdfs:subClassOf>
        <rdfs:subClassOf>
            <owl:Restriction>
                <owl:onProperty rdf:resource="http://www.ease-crc.org/ont/SUTURO.owl#hasPredefinedName"/>
                <owl:hasValue>damsel</owl:hasValue>
            </owl:Restriction>
        </rdfs:subClassOf>
        <rdfs:subClassOf>
            <owl:Restriction>
                <owl:onProperty rdf:resource="http://www.ease-crc.org/ont/SUTURO.owl#hasPredefinedName"/>
                <owl:hasValue>fellow</owl:hasValue>
            </owl:Restriction>
        </rdfs:subClassOf>
        <rdfs:subClassOf>
            <owl:Restriction>
                <owl:onProperty rdf:resource="http://www.ease-crc.org/ont/SUTURO.owl#hasPredefinedName"/>
                <owl:hasValue>gentleman</owl:hasValue>
            </owl:Restriction>
        </rdfs:subClassOf>
        <rdfs:subClassOf>
            <owl:Restriction>
                <owl:onProperty rdf:resource="http://www.ease-crc.org/ont/SUTURO.owl#hasPredefinedName"/>
                <owl:hasValue>girl</owl:hasValue>
            </owl:Restriction>
        </rdfs:subClassOf>
        <rdfs:subClassOf>
            <owl:Restriction>
                <owl:onProperty rdf:resource="http://www.ease-crc.org/ont/SUTURO.owl#hasPredefinedName"/>
                <owl:hasValue>guy</owl:hasValue>
            </owl:Restriction>
        </rdfs:subClassOf>
        <rdfs:subClassOf>
            <owl:Restriction>
                <owl:onProperty rdf:resource="http://www.ease-crc.org/ont/SUTURO.owl#hasPredefinedName"/>
                <owl:hasValue>lady</owl:hasValue>
            </owl:Restriction>
        </rdfs:subClassOf>
        <rdfs:subClassOf>
            <owl:Restriction>
                <owl:onProperty rdf:resource="http://www.ease-crc.org/ont/SUTURO.owl#hasPredefinedName"/>
                <owl:hasValue>lord</owl:hasValue>
            </owl:Restriction>
        </rdfs:subClassOf>
        <rdfs:subClassOf>
            <owl:Restriction>
                <owl:onProperty rdf:resource="http://www.ease-crc.org/ont/SUTURO.owl#hasPredefinedName"/>
                <owl:hasValue>madam</owl:hasValue>
            </owl:Restriction>
        </rdfs:subClassOf>
        <rdfs:subClassOf>
            <owl:Restriction>
                <owl:onProperty rdf:resource="http://www.ease-crc.org/ont/SUTURO.owl#hasPredefinedName"/>
                <owl:hasValue>man</owl:hasValue>
            </owl:Restriction>
        </rdfs:subClassOf>
        <rdfs:subClassOf>
            <owl:Restriction>
                <owl:onProperty rdf:resource="http://www.ease-crc.org/ont/SUTURO.owl#hasPredefinedName"/>
                <owl:hasValue>miss</owl:hasValue>
            </owl:Restriction>
        </rdfs:subClassOf>
        <rdfs:subClassOf>
            <owl:Restriction>
                <owl:onProperty rdf:resource="http://www.ease-crc.org/ont/SUTURO.owl#hasPredefinedName"/>
                <owl:hasValue>missus</owl:hasValue>
            </owl:Restriction>
        </rdfs:subClassOf>
        <rdfs:subClassOf>
            <owl:Restriction>
                <owl:onProperty rdf:resource="http://www.ease-crc.org/ont/SUTURO.owl#hasPredefinedName"/>
                <owl:hasValue>mister</owl:hasValue>
            </owl:Restriction>
        </rdfs:subClassOf>
        <rdfs:subClassOf>
            <owl:Restriction>
                <owl:onProperty rdf:resource="http://www.ease-crc.org/ont/SUTURO.owl#hasPredefinedName"/>
                <owl:hasValue>mr</owl:hasValue>
            </owl:Restriction>
        </rdfs:subClassOf>
        <rdfs:subClassOf>
            <owl:Restriction>
                <owl:onProperty rdf:resource="http://www.ease-crc.org/ont/SUTURO.owl#hasPredefinedName"/>
                <owl:hasValue>mrs</owl:hasValue>
            </owl:Restriction>
        </rdfs:subClassOf>
        <rdfs:subClassOf>
            <owl:Restriction>
                <owl:onProperty rdf:resource="http://www.ease-crc.org/ont/SUTURO.owl#hasPredefinedName"/>
                <owl:hasValue>person</owl:hasValue>
            </owl:Restriction>
        </rdfs:subClassOf>
        <rdfs:subClassOf>
            <owl:Restriction>
                <owl:onProperty rdf:resource="http://www.ease-crc.org/ont/SUTURO.owl#hasPredefinedName"/>
                <owl:hasValue>woman</owl:hasValue>
            </owl:Restriction>
        </rdfs:subClassOf>
        <SUTURO:perceptionId rdf:datatype="http://www.w3.org/2001/XMLSchema#int">23</SUTURO:perceptionId>
    </owl:Class>
    


    <!-- http://www.ontologydesignpatterns.org/ont/dul/DUL.owl#Plan -->

    <owl:Class rdf:about="http://www.ontologydesignpatterns.org/ont/dul/DUL.owl#Plan"/>
    


    <!-- http://www.ontologydesignpatterns.org/ont/dul/DUL.owl#SocialObject -->

    <owl:Class rdf:about="http://www.ontologydesignpatterns.org/ont/dul/DUL.owl#SocialObject"/>
    


    <!-- http://www.ontologydesignpatterns.org/ont/dul/DUL.owl#Substance -->

    <owl:Class rdf:about="http://www.ontologydesignpatterns.org/ont/dul/DUL.owl#Substance"/>
    


    <!-- 
    ///////////////////////////////////////////////////////////////////////////////////////
    //
    // Annotations
    //
    ///////////////////////////////////////////////////////////////////////////////////////
     -->

    <rdf:Description rdf:about="http://www.ease-crc.org/ont/SOMA-HOME.owl#DesignedChair">
        <SUTURO:perceptionId rdf:datatype="http://www.w3.org/2001/XMLSchema#int">2</SUTURO:perceptionId>
    </rdf:Description>
    <rdf:Description rdf:about="http://www.ease-crc.org/ont/SOMA-HOME.owl#KitchenCabinet">
        <SUTURO:perceptionId rdf:datatype="http://www.w3.org/2001/XMLSchema#int">9</SUTURO:perceptionId>
    </rdf:Description>
    <rdf:Description rdf:about="http://www.ease-crc.org/ont/SOMA.owl#Compartment">
        <rdfs:comment>A compartment is a distinct, enclosed space within a larger structure or system, often used to separate or organize different components or elements. It helps to compartmentalize and manage complex systems by providing a segregated environment for specific functions or entities.</rdfs:comment>
    </rdf:Description>
    <rdf:Description rdf:about="http://www.ease-crc.org/ont/SOMA.owl#PancakeMix">
        <rdfs:comment>Pancake mix is a pre-made dry mixture of flour, baking powder, salt, and other ingredients that is used to make pancakes quickly and easily. It typically requires the addition of liquid ingredients such as milk, eggs, and oil, and can be customized with various flavors and additions such as chocolate chips or blueberries.</rdfs:comment>
    </rdf:Description>
    <rdf:Description rdf:about="http://www.ease-crc.org/ont/SOMA.owl#Tableware">
        <rdfs:comment>Tableware refers to the dishes, utensils, and other items used for serving and eating food. This can include plates, bowls, cups, silverware, and serving platters, among other things.</rdfs:comment>
    </rdf:Description>
</rdf:RDF>



<!-- Generated by the OWL API (version 4.5.29.2024-05-13T12:11:03Z) https://github.com/owlcs/owlapi -->

